<?xml version="1.0"?>
<rdf:RDF xmlns="https://w3id.org/hacid/onto/core/naming/"
     xml:base="https://w3id.org/hacid/onto/core/naming/"
     xmlns:top="https://w3id.org/hacid/onto/top-level/"
     xmlns:rdf="http://www.w3.org/1999/02/22-rdf-syntax-ns#"
     xmlns:owl="http://www.w3.org/2002/07/owl#"
     xmlns:xml="http://www.w3.org/XML/1998/namespace"
     xmlns:xsd="http://www.w3.org/2001/XMLSchema#"
     xmlns:rdfs="http://www.w3.org/2000/01/rdf-schema#">
    <owl:Ontology rdf:about="https://w3id.org/hacid/onto/core/naming">
        <owl:imports rdf:resource="https://w3id.org/hacid/onto/top-level"/>
    </owl:Ontology>
    


    <!-- 
    ///////////////////////////////////////////////////////////////////////////////////////
    //
    // Object Properties
    //
    ///////////////////////////////////////////////////////////////////////////////////////
     -->

    


    <!-- https://w3id.org/hacid/onto/core/naming/hasAlternativeName -->

    <owl:ObjectProperty rdf:about="https://w3id.org/hacid/onto/core/naming/hasAlternativeName">
        <rdfs:subPropertyOf rdf:resource="https://w3id.org/hacid/onto/core/naming/hasName"/>
        <owl:inverseOf rdf:resource="https://w3id.org/hacid/onto/core/naming/isAlternativeNameOf"/>
        <rdfs:domain rdf:resource="https://w3id.org/hacid/onto/top-level/Entity"/>
        <rdfs:range rdf:resource="https://w3id.org/hacid/onto/core/naming/Name"/>
        <rdfs:comment xml:lang="it">La proprietà per associare un nome alternativo all&apos;entità da nominare.</rdfs:comment>
        <rdfs:comment xml:lang="en">The property to associate an alternative name with the entity being named.</rdfs:comment>
        <rdfs:label xml:lang="it">ha nome alternativo</rdfs:label>
        <rdfs:label xml:lang="en">has alternative name</rdfs:label>
    </owl:ObjectProperty>
    


    <!-- https://w3id.org/hacid/onto/core/naming/hasName -->

    <owl:ObjectProperty rdf:about="https://w3id.org/hacid/onto/core/naming/hasName">
        <rdfs:subPropertyOf rdf:resource="https://w3id.org/hacid/onto/top-level/associatedWith"/>
        <owl:inverseOf rdf:resource="https://w3id.org/hacid/onto/core/naming/isNameOf"/>
        <rdfs:domain rdf:resource="https://w3id.org/hacid/onto/top-level/Entity"/>
        <rdfs:range rdf:resource="https://w3id.org/hacid/onto/core/naming/Name"/>
        <rdfs:comment xml:lang="it">La proprietà che associa un&apos;entità al nome corrispondente.</rdfs:comment>
        <rdfs:comment xml:lang="en">The property that associates an entity with its corresponding name.</rdfs:comment>
        <rdfs:isDefinedBy rdf:resource="https://w3id.org/hacid/onto/core/naming"/>
        <rdfs:label xml:lang="it">ha nome</rdfs:label>
        <rdfs:label xml:lang="en">has name</rdfs:label>
    </owl:ObjectProperty>
    


    <!-- https://w3id.org/hacid/onto/core/naming/hasNameType -->

    <owl:ObjectProperty rdf:about="https://w3id.org/hacid/onto/core/naming/hasNameType">
        <rdfs:subPropertyOf rdf:resource="https://w3id.org/hacid/onto/top-level/isClassifiedBy"/>
        <owl:inverseOf rdf:resource="https://w3id.org/hacid/onto/core/naming/isNameTypeOf"/>
        <rdfs:domain rdf:resource="https://w3id.org/hacid/onto/core/naming/Naming"/>
        <rdfs:range rdf:resource="https://w3id.org/hacid/onto/core/naming/NameType"/>
        <rdfs:comment xml:lang="it">La proprietà che serve a classificare una denominazione con un tipo di nome.</rdfs:comment>
        <rdfs:comment xml:lang="en">The property that serves to classify a denomination with a name type.</rdfs:comment>
        <rdfs:isDefinedBy rdf:resource="https://w3id.org/hacid/onto/core/naming"/>
        <rdfs:label xml:lang="it">ha tipo di nome</rdfs:label>
        <rdfs:label xml:lang="en">has name type</rdfs:label>
    </owl:ObjectProperty>
    


    <!-- https://w3id.org/hacid/onto/core/naming/hasNaming -->

    <owl:ObjectProperty rdf:about="https://w3id.org/hacid/onto/core/naming/hasNaming">
        <rdfs:subPropertyOf rdf:resource="https://w3id.org/hacid/onto/top-level/isInvolvedIn"/>
        <owl:inverseOf rdf:resource="https://w3id.org/hacid/onto/core/naming/isNamingOf"/>
        <rdfs:domain rdf:resource="https://w3id.org/hacid/onto/top-level/Entity"/>
        <rdfs:range rdf:resource="https://w3id.org/hacid/onto/core/naming/Naming"/>
        <rdfs:comment xml:lang="it">La proprietà per collegare un&apos;entità alla sua denominazione.</rdfs:comment>
        <rdfs:comment xml:lang="en">The property to link an entity to its naming.</rdfs:comment>
        <rdfs:isDefinedBy rdf:resource="https://w3id.org/hacid/onto/core/naming"/>
        <rdfs:label xml:lang="it">ha denominazione</rdfs:label>
        <rdfs:label xml:lang="en">has naming</rdfs:label>
    </owl:ObjectProperty>
    


    <!-- https://w3id.org/hacid/onto/core/naming/hasPreferredName -->

    <owl:ObjectProperty rdf:about="https://w3id.org/hacid/onto/core/naming/hasPreferredName">
        <rdfs:subPropertyOf rdf:resource="https://w3id.org/hacid/onto/core/naming/hasName"/>
        <owl:inverseOf rdf:resource="https://w3id.org/hacid/onto/core/naming/isPreferredNameOf"/>
        <rdfs:domain rdf:resource="https://w3id.org/hacid/onto/top-level/Entity"/>
        <rdfs:range rdf:resource="https://w3id.org/hacid/onto/core/naming/Name"/>
        <rdfs:comment xml:lang="it">La specializzazione di &quot;ha nome&quot; per riferirsi a un nome preferito.</rdfs:comment>
        <rdfs:comment xml:lang="en">The specialisation of &quot;has name&quot; for referring to a preferred name.</rdfs:comment>
        <rdfs:isDefinedBy rdf:resource="https://w3id.org/hacid/onto/core/naming"/>
        <rdfs:label xml:lang="it">ha nome preferito</rdfs:label>
        <rdfs:label xml:lang="en">has preferred name</rdfs:label>
    </owl:ObjectProperty>
    


    <!-- https://w3id.org/hacid/onto/core/naming/isAlternativeNameOf -->

    <owl:ObjectProperty rdf:about="https://w3id.org/hacid/onto/core/naming/isAlternativeNameOf">
        <rdfs:subPropertyOf rdf:resource="https://w3id.org/hacid/onto/core/naming/isNameOf"/>
        <rdfs:domain rdf:resource="https://w3id.org/hacid/onto/core/naming/Name"/>
        <rdfs:range rdf:resource="https://w3id.org/hacid/onto/top-level/Entity"/>
        <rdfs:comment xml:lang="it">La proprietà per associare un nome qualificato come alternativo all&apos;entità che viene nominata.</rdfs:comment>
        <rdfs:comment xml:lang="en">The property to associate an alternative name with the entity being named.</rdfs:comment>
        <rdfs:isDefinedBy rdf:resource="https://w3id.org/hacid/onto/core/naming"/>
        <rdfs:label xml:lang="en">is alternative name of</rdfs:label>
        <rdfs:label xml:lang="it">è nome alternativo di</rdfs:label>
    </owl:ObjectProperty>
    


    <!-- https://w3id.org/hacid/onto/core/naming/isNameOf -->

    <owl:ObjectProperty rdf:about="https://w3id.org/hacid/onto/core/naming/isNameOf">
        <rdfs:subPropertyOf rdf:resource="https://w3id.org/hacid/onto/top-level/associatedWith"/>
        <rdfs:domain rdf:resource="https://w3id.org/hacid/onto/core/naming/Name"/>
        <rdfs:range rdf:resource="https://w3id.org/hacid/onto/top-level/Entity"/>
        <rdfs:comment xml:lang="it">La proprietà che collega un nome a un&apos;entità.</rdfs:comment>
        <rdfs:comment xml:lang="en">The property that links a name to an entity.</rdfs:comment>
        <rdfs:isDefinedBy rdf:resource="https://w3id.org/hacid/onto/core/naming"/>
        <rdfs:label xml:lang="en">is name of</rdfs:label>
        <rdfs:label xml:lang="it">è nome di</rdfs:label>
    </owl:ObjectProperty>
    


    <!-- https://w3id.org/hacid/onto/core/naming/isNameTypeOf -->

    <owl:ObjectProperty rdf:about="https://w3id.org/hacid/onto/core/naming/isNameTypeOf">
        <rdfs:subPropertyOf rdf:resource="https://w3id.org/hacid/onto/top-level/classifies"/>
        <rdfs:domain rdf:resource="https://w3id.org/hacid/onto/core/naming/NameType"/>
        <rdfs:range rdf:resource="https://w3id.org/hacid/onto/core/naming/Naming"/>
        <rdfs:comment xml:lang="it">La proprietà che collega un tipo di nome ad una denominazione.</rdfs:comment>
        <rdfs:comment xml:lang="en">The property that links a name type to a naming.</rdfs:comment>
        <rdfs:isDefinedBy rdf:resource="https://w3id.org/hacid/onto/core/naming"/>
        <rdfs:label xml:lang="en">is name type of</rdfs:label>
        <rdfs:label xml:lang="it">è tipo di nome di</rdfs:label>
    </owl:ObjectProperty>
    


    <!-- https://w3id.org/hacid/onto/core/naming/isNamingOf -->

    <owl:ObjectProperty rdf:about="https://w3id.org/hacid/onto/core/naming/isNamingOf">
        <rdfs:subPropertyOf rdf:resource="https://w3id.org/hacid/onto/top-level/involves"/>
        <rdfs:domain rdf:resource="https://w3id.org/hacid/onto/core/naming/Naming"/>
        <rdfs:range rdf:resource="https://w3id.org/hacid/onto/top-level/Entity"/>
        <rdfs:comment xml:lang="it">La relazione di coinvolgimento limitata alla sola situazione di denominazione.</rdfs:comment>
        <rdfs:comment xml:lang="en">The involves relation which is narrowed to naming situation only.</rdfs:comment>
        <rdfs:isDefinedBy rdf:resource="https://w3id.org/hacid/onto/core/naming"/>
        <rdfs:label xml:lang="en">is naming of</rdfs:label>
        <rdfs:label xml:lang="it">è denominazione di</rdfs:label>
    </owl:ObjectProperty>
    


    <!-- https://w3id.org/hacid/onto/core/naming/isPreferredNameOf -->

    <owl:ObjectProperty rdf:about="https://w3id.org/hacid/onto/core/naming/isPreferredNameOf">
        <rdfs:subPropertyOf rdf:resource="https://w3id.org/hacid/onto/core/naming/isNameOf"/>
        <rdfs:domain rdf:resource="https://w3id.org/hacid/onto/core/naming/Name"/>
        <rdfs:range rdf:resource="https://w3id.org/hacid/onto/top-level/Entity"/>
        <rdfs:comment xml:lang="it">La proprietà per associare un nome qualificato come preferito all&apos;entità che viene nominata.</rdfs:comment>
        <rdfs:comment xml:lang="en">The property to associate a preferred name with the entity being named.</rdfs:comment>
        <rdfs:isDefinedBy rdf:resource="https://w3id.org/hacid/onto/core/naming"/>
        <rdfs:label xml:lang="en">is preferred name of</rdfs:label>
        <rdfs:label xml:lang="it">è nome preferito di</rdfs:label>
    </owl:ObjectProperty>
    


    <!-- 
    ///////////////////////////////////////////////////////////////////////////////////////
    //
    // Data properties
    //
    ///////////////////////////////////////////////////////////////////////////////////////
     -->

    


    <!-- https://w3id.org/hacid/onto/core/naming/lexicalItem -->

    <owl:DatatypeProperty rdf:about="https://w3id.org/hacid/onto/core/naming/lexicalItem">
        <rdfs:subPropertyOf rdf:resource="https://w3id.org/hacid/onto/top-level/name"/>
        <rdfs:domain rdf:resource="https://w3id.org/hacid/onto/core/naming/Name"/>
        <rdfs:range rdf:resource="http://www.w3.org/2000/01/rdf-schema#Literal"/>
        <rdfs:comment xml:lang="it">La proprietà datatype per associare un nome alla sua espressione lessicale.</rdfs:comment>
        <rdfs:comment xml:lang="en">The datatype property for associating a name with its lexical item.</rdfs:comment>
        <rdfs:isDefinedBy rdf:resource="https://w3id.org/hacid/onto/core/naming"/>
        <rdfs:label xml:lang="it">elemento lessicale</rdfs:label>
        <rdfs:label xml:lang="en">lexical item</rdfs:label>
    </owl:DatatypeProperty>
    


    <!-- 
    ///////////////////////////////////////////////////////////////////////////////////////
    //
    // Classes
    //
    ///////////////////////////////////////////////////////////////////////////////////////
     -->

    


    <!-- https://w3id.org/hacid/onto/core/naming/Name -->

    <owl:Class rdf:about="https://w3id.org/hacid/onto/core/naming/Name">
        <rdfs:subClassOf rdf:resource="https://w3id.org/hacid/onto/top-level/Value"/>
        <rdfs:subClassOf>
            <owl:Restriction>
                <owl:onProperty rdf:resource="https://w3id.org/hacid/onto/core/naming/lexicalItem"/>
                <owl:someValuesFrom rdf:resource="http://www.w3.org/2000/01/rdf-schema#Literal"/>
            </owl:Restriction>
        </rdfs:subClassOf>
        <rdfs:comment xml:lang="it">Nome di un&apos;entità inteso come suo elemento lessicale, cioè una singola parola, una parte di una parola o una catena di parole che forma sintatticamente un nome.</rdfs:comment>
        <rdfs:comment xml:lang="en">The name of an entity meant as its lexical item, i.e., a single word, a part of a word, or a chain of words that forms a name syntactically.</rdfs:comment>
        <rdfs:isDefinedBy rdf:resource="https://w3id.org/hacid/onto/core/naming"/>
        <rdfs:label xml:lang="en">Name</rdfs:label>
        <rdfs:label xml:lang="it">Nome</rdfs:label>
    </owl:Class>
    


    <!-- https://w3id.org/hacid/onto/core/naming/NameType -->

    <owl:Class rdf:about="https://w3id.org/hacid/onto/core/naming/NameType">
        <rdfs:subClassOf rdf:resource="https://w3id.org/hacid/onto/top-level/Concept"/>
        <rdfs:subClassOf>
            <owl:Restriction>
                <owl:onProperty rdf:resource="https://w3id.org/hacid/onto/top-level/classifies"/>
                <owl:allValuesFrom rdf:resource="https://w3id.org/hacid/onto/core/naming/Naming"/>
            </owl:Restriction>
        </rdfs:subClassOf>
        <rdfs:comment xml:lang="en">A kind of name. Possible examples are: &quot;Peferred name&quot;, &quot;Alternative name&quot;, etc...</rdfs:comment>
        <rdfs:comment xml:lang="it">Un tipo di nome. Possibili esempi sono: &quot;Nome prefito&quot;, &quot;Nome alternativo&quot;, ecc...</rdfs:comment>
        <rdfs:isDefinedBy rdf:resource="https://w3id.org/hacid/onto/core/naming"/>
        <rdfs:label xml:lang="en">Name type</rdfs:label>
        <rdfs:label xml:lang="it">Tipo di nome</rdfs:label>
    </owl:Class>
    


    <!-- https://w3id.org/hacid/onto/core/naming/Naming -->

    <owl:Class rdf:about="https://w3id.org/hacid/onto/core/naming/Naming">
        <rdfs:subClassOf rdf:resource="https://w3id.org/hacid/onto/top-level/Situation"/>
        <rdfs:subClassOf>
            <owl:Restriction>
                <owl:onProperty rdf:resource="https://w3id.org/hacid/onto/core/naming/hasName"/>
                <owl:someValuesFrom rdf:resource="https://w3id.org/hacid/onto/core/naming/Name"/>
            </owl:Restriction>
        </rdfs:subClassOf>
        <rdfs:subClassOf>
            <owl:Restriction>
                <owl:onProperty rdf:resource="https://w3id.org/hacid/onto/core/naming/hasNameType"/>
                <owl:someValuesFrom rdf:resource="https://w3id.org/hacid/onto/core/naming/NameType"/>
            </owl:Restriction>
        </rdfs:subClassOf>
        <rdfs:subClassOf>
            <owl:Restriction>
                <owl:onProperty rdf:resource="https://w3id.org/hacid/onto/core/naming/isNamingOf"/>
                <owl:someValuesFrom rdf:resource="https://w3id.org/hacid/onto/top-level/Entity"/>
            </owl:Restriction>
        </rdfs:subClassOf>
        <owl:hasKey rdf:parseType="Collection">
            <rdf:Description rdf:about="https://w3id.org/hacid/onto/core/naming/hasName"/>
            <rdf:Description rdf:about="https://w3id.org/hacid/onto/core/naming/hasNameType"/>
            <rdf:Description rdf:about="https://w3id.org/hacid/onto/core/naming/isNamingOf"/>
        </owl:hasKey>
        <rdfs:comment xml:lang="it">L&apos;atto di associare un nome ad un&apos;entità.</rdfs:comment>
        <rdfs:comment xml:lang="en">The act of associating a name to an entity.</rdfs:comment>
        <rdfs:isDefinedBy rdf:resource="https://w3id.org/hacid/onto/core/naming"/>
        <rdfs:label xml:lang="it">Denominazione</rdfs:label>
        <rdfs:label xml:lang="en">Naming</rdfs:label>
    </owl:Class>
    


    <!-- https://w3id.org/hacid/onto/core/naming/SynonymSet -->

    <owl:Class rdf:about="https://w3id.org/hacid/onto/core/naming/SynonymSet">
        <rdfs:subClassOf rdf:resource="https://w3id.org/hacid/onto/top-level/Collection"/>
        <rdfs:subClassOf>
            <owl:Restriction>
                <owl:onProperty rdf:resource="https://w3id.org/hacid/onto/top-level/hasMember"/>
                <owl:someValuesFrom rdf:resource="https://w3id.org/hacid/onto/core/naming/Naming"/>
            </owl:Restriction>
        </rdfs:subClassOf>
        <rdfs:subClassOf>
            <owl:Restriction>
                <owl:onProperty rdf:resource="https://w3id.org/hacid/onto/top-level/hasMember"/>
                <owl:allValuesFrom rdf:resource="https://w3id.org/hacid/onto/core/naming/Naming"/>
            </owl:Restriction>
        </rdfs:subClassOf>
    </owl:Class>
    


    <!-- 
    ///////////////////////////////////////////////////////////////////////////////////////
    //
    // Individuals
    //
    ///////////////////////////////////////////////////////////////////////////////////////
     -->

    


    <!-- https://w3id.org/hacid/onto/core/naming/alternative-name -->

    <owl:NamedIndividual rdf:about="https://w3id.org/hacid/onto/core/naming/alternative-name">
        <rdf:type rdf:resource="https://w3id.org/hacid/onto/core/naming/NameType"/>
        <rdfs:comment xml:lang="it">L&apos;individuo che rappresenta il concetto di nome che è un&apos;espressione alternativa per denominare una determinata entità.</rdfs:comment>
        <rdfs:comment xml:lang="en">The individual representing the concept of a name which is an alternative expression for naming a certain entity.</rdfs:comment>
        <rdfs:label rdf:resource="https://w3id.org/hacid/onto/core/naming"/>
        <rdfs:label xml:lang="en">alternative name</rdfs:label>
        <rdfs:label xml:lang="it">nome alternativo</rdfs:label>
    </owl:NamedIndividual>
    


    <!-- https://w3id.org/hacid/onto/core/naming/preferred-name -->

    <owl:NamedIndividual rdf:about="https://w3id.org/hacid/onto/core/naming/preferred-name">
        <rdf:type rdf:resource="https://w3id.org/hacid/onto/core/naming/NameType"/>
        <rdfs:comment xml:lang="it">L&apos;individuo che rappresenta il concetto di nome preferito per denominare una determinata entità.</rdfs:comment>
        <rdfs:comment xml:lang="en">The individual representing the concept of a name which is preferred for naming a certain entity.</rdfs:comment>
        <rdfs:isDefinedBy rdf:resource="https://w3id.org/hacid/onto/core/naming"/>
        <rdfs:label xml:lang="it">Nome preferito</rdfs:label>
        <rdfs:label xml:lang="en">Preferred name</rdfs:label>
    </owl:NamedIndividual>
</rdf:RDF>



<!-- Generated by the OWL API (version 4.2.8.20170104-2310) https://github.com/owlcs/owlapi -->

