<rdf:RDF xmlns:rdf="http://www.w3.org/1999/02/22-rdf-syntax-ns#" xmlns:rdfs="http://www.w3.org/2000/01/rdf-schema#" xmlns:owl="http://www.w3.org/2002/07/owl#" xml:base="https://w3id.org/hacid/onto/top-level">
    <owl:Ontology rdf:about="https://w3id.org/hacid/onto/top-level"/>
    


    <!-- 
    ///////////////////////////////////////////////////////////////////////////////////////
    //
    // Datatypes
    //
    ///////////////////////////////////////////////////////////////////////////////////////
     -->

    


    <!-- http://www.w3.org/2001/XMLSchema#date -->

    <rdfs:Datatype rdf:about="http://www.w3.org/2001/XMLSchema#date"/>
    


    <!-- http://www.w3.org/2001/XMLSchema#gYear -->

    <rdfs:Datatype rdf:about="http://www.w3.org/2001/XMLSchema#gYear"/>
    


    <!-- http://www.w3.org/2001/XMLSchema#time -->

    <rdfs:Datatype rdf:about="http://www.w3.org/2001/XMLSchema#time"/>
    


    <!-- 
    ///////////////////////////////////////////////////////////////////////////////////////
    //
    // Object Properties
    //
    ///////////////////////////////////////////////////////////////////////////////////////
     -->

    


    <!-- http://www.w3.org/2000/01/rdf-schema#domain -->

    <owl:ObjectProperty rdf:about="http://www.w3.org/2000/01/rdf-schema#domain"/>
    


    <!-- https://w3id.org/hacid/onto/top-level/associatedWith -->

    <owl:ObjectProperty rdf:about="https://w3id.org/hacid/onto/top-level/associatedWith">
        <rdfs:comment xml:lang="en">A catch-all object property, useful for alignment and querying purposes.
It is declared as both transitive and symmetric, in order to reason an a maximal closure of associations between individuals.</rdfs:comment>
        <rdfs:isDefinedBy rdf:resource="https://w3id.org/hacid/onto/top-level"/>
        <rdfs:label xml:lang="en">associated with</rdfs:label>
        <rdfs:label xml:lang="it">associato a</rdfs:label>
    </owl:ObjectProperty>
    


    <!-- https://w3id.org/hacid/onto/top-level/atTime -->

    <owl:ObjectProperty rdf:about="https://w3id.org/hacid/onto/top-level/atTime">
        <rdfs:subPropertyOf rdf:resource="https://w3id.org/hacid/onto/top-level/associatedWith"/>
        <owl:inverseOf rdf:resource="https://w3id.org/hacid/onto/top-level/isTimeOf"/>
        <rdfs:domain rdf:resource="https://w3id.org/hacid/onto/top-level/Entity"/>
        <rdfs:range rdf:resource="https://w3id.org/hacid/onto/top-level/TemporalEntity"/>
        <rdfs:comment xml:lang="it">La relazione esistente tra una qualsiasi entità ed un'entità temporale.</rdfs:comment>
        <rdfs:comment xml:lang="en">The relation holding between an entity ad a temporal entity.</rdfs:comment>
        <rdfs:isDefinedBy rdf:resource="https://w3id.org/hacid/onto/top-level"/>
        <rdfs:label xml:lang="it">al tempo</rdfs:label>
        <rdfs:label xml:lang="en">at time</rdfs:label>
    </owl:ObjectProperty>
    


    <!-- https://w3id.org/hacid/onto/top-level/classifies -->

    <owl:ObjectProperty rdf:about="https://w3id.org/hacid/onto/top-level/classifies">
        <rdfs:subPropertyOf rdf:resource="https://w3id.org/hacid/onto/top-level/associatedWith"/>
        <owl:inverseOf rdf:resource="https://w3id.org/hacid/onto/top-level/isClassifiedBy"/>
        <rdfs:domain rdf:resource="https://w3id.org/hacid/onto/top-level/Concept"/>
        <rdfs:range rdf:resource="https://w3id.org/hacid/onto/top-level/Entity"/>
        <rdfs:comment xml:lang="it">La proprietà utilizzata per affermare che un concetto classificava una certa entità.</rdfs:comment>
        <rdfs:comment xml:lang="en">The property used to state that a concept classified a certain entity.</rdfs:comment>
        <rdfs:isDefinedBy rdf:resource="https://w3id.org/hacid/onto/top-level"/>
        <rdfs:label xml:lang="it">classifica</rdfs:label>
        <rdfs:label xml:lang="en">classifies</rdfs:label>
    </owl:ObjectProperty>
    


    <!-- https://w3id.org/hacid/onto/top-level/defines -->

    <owl:ObjectProperty rdf:about="https://w3id.org/hacid/onto/top-level/defines">
        <rdfs:subPropertyOf rdf:resource="https://w3id.org/hacid/onto/top-level/usesConcept"/>
        <owl:inverseOf rdf:resource="https://w3id.org/hacid/onto/top-level/isDefinedIn"/>
        <rdfs:domain rdf:resource="https://w3id.org/hacid/onto/top-level/Description"/>
        <rdfs:range rdf:resource="https://w3id.org/hacid/onto/top-level/Concept"/>
        <rdfs:comment xml:lang="en">A relation between a Description and a Concept, e.g. a Workflow for a governmental Organization defines the Role 'officer', or 'the Italian Traffic Law defines the role Vehicle'.</rdfs:comment>
        <rdfs:isDefinedBy rdf:resource="https://w3id.org/hacid/onto/top-level"/>
        <rdfs:label xml:lang="en">defines</rdfs:label>
        <rdfs:label xml:lang="it">definisce</rdfs:label>
    </owl:ObjectProperty>
    


    <!-- https://w3id.org/hacid/onto/top-level/definesRole -->

    <owl:ObjectProperty rdf:about="https://w3id.org/hacid/onto/top-level/definesRole">
        <rdfs:subPropertyOf rdf:resource="https://w3id.org/hacid/onto/top-level/defines"/>
        <owl:inverseOf rdf:resource="https://w3id.org/hacid/onto/top-level/isRoleDefinedIn"/>
        <rdfs:domain rdf:resource="https://w3id.org/hacid/onto/top-level/Description"/>
        <rdfs:range rdf:resource="https://w3id.org/hacid/onto/top-level/Role"/>
        <rdfs:comment xml:lang="en">A relation between a description and a role, e.g. the recipe for a cake defines the role 'ingredient'.</rdfs:comment>
        <rdfs:isDefinedBy rdf:resource="https://w3id.org/hacid/onto/top-level"/>
        <rdfs:label xml:lang="en">defines role</rdfs:label>
        <rdfs:label xml:lang="it">definisce il ruolo</rdfs:label>
    </owl:ObjectProperty>
    


    <!-- https://w3id.org/hacid/onto/top-level/definesTask -->

    <owl:ObjectProperty rdf:about="https://w3id.org/hacid/onto/top-level/definesTask">
        <rdfs:subPropertyOf rdf:resource="https://w3id.org/hacid/onto/top-level/defines"/>
        <owl:inverseOf rdf:resource="https://w3id.org/hacid/onto/top-level/isTaskDefinedIn"/>
        <rdfs:domain rdf:resource="https://w3id.org/hacid/onto/top-level/Description"/>
        <rdfs:range rdf:resource="https://w3id.org/hacid/onto/top-level/Task"/>
        <rdfs:comment xml:lang="en">A relation between a description and a task, e.g. the recipe for a cake defines the task 'boil'.</rdfs:comment>
        <rdfs:isDefinedBy rdf:resource="https://w3id.org/hacid/onto/top-level"/>
        <rdfs:label xml:lang="en">defines task</rdfs:label>
        <rdfs:label xml:lang="it">definisce il task</rdfs:label>
    </owl:ObjectProperty>
    


    <!-- https://w3id.org/hacid/onto/top-level/describes -->

    <owl:ObjectProperty rdf:about="https://w3id.org/hacid/onto/top-level/describes">
        <rdfs:subPropertyOf rdf:resource="https://w3id.org/hacid/onto/top-level/associatedWith"/>
        <owl:inverseOf rdf:resource="https://w3id.org/hacid/onto/top-level/isDescribedBy"/>
        <rdfs:domain rdf:resource="https://w3id.org/hacid/onto/top-level/Description"/>
        <rdfs:range rdf:resource="https://w3id.org/hacid/onto/top-level/Entity"/>
        <rdfs:comment xml:lang="it">La realazione per associare una descrizione all'entità oggetto di tale descrizione.</rdfs:comment>
        <rdfs:comment xml:lang="en">The relation for associating a description with the entity being described.</rdfs:comment>
        <rdfs:isDefinedBy rdf:resource="https://w3id.org/hacid/onto/top-level"/>
        <rdfs:label xml:lang="it">describe</rdfs:label>
        <rdfs:label xml:lang="en">describes</rdfs:label>
    </owl:ObjectProperty>
    


    <!-- https://w3id.org/hacid/onto/top-level/directlyFollows -->

    <owl:ObjectProperty rdf:about="https://w3id.org/hacid/onto/top-level/directlyFollows">
        <rdfs:subPropertyOf rdf:resource="https://w3id.org/hacid/onto/top-level/follows"/>
        <owl:inverseOf rdf:resource="https://w3id.org/hacid/onto/top-level/directlyPrecedes"/>
        <rdfs:domain rdf:resource="https://w3id.org/hacid/onto/top-level/Entity"/>
        <rdfs:range rdf:resource="https://w3id.org/hacid/onto/top-level/Entity"/>
        <rdfs:comment xml:lang="it">L'intransitivo segue la relazione. Ad esempio, il martedì segue direttamente il lunedì. L'immediatezza della precedenza dipende dalla concettualizzazione del progettista.</rdfs:comment>
        <rdfs:comment xml:lang="en">The intransitive follows relation. For example, Tuesday directly follows Monday. Directness of precedence depends on the designer conceptualization.</rdfs:comment>
        <rdfs:isDefinedBy rdf:resource="https://w3id.org/hacid/onto/top-level"/>
        <rdfs:label xml:lang="en">directly follows</rdfs:label>
        <rdfs:label xml:lang="it">segue direttamente</rdfs:label>
    </owl:ObjectProperty>
    


    <!-- https://w3id.org/hacid/onto/top-level/directlyPrecedes -->

    <owl:ObjectProperty rdf:about="https://w3id.org/hacid/onto/top-level/directlyPrecedes">
        <rdfs:subPropertyOf rdf:resource="https://w3id.org/hacid/onto/top-level/precedes"/>
        <rdfs:domain rdf:resource="https://w3id.org/hacid/onto/top-level/Entity"/>
        <rdfs:range rdf:resource="https://w3id.org/hacid/onto/top-level/Entity"/>
        <rdfs:comment xml:lang="it">L'intransitivo precede la relazione. Ad esempio, il lunedì precede direttamente il martedì. L'immediatezza della precedenza dipende dalla concettualizzazione del progettista.</rdfs:comment>
        <rdfs:comment xml:lang="en">The intransitive precedes relation. For example, Monday directly precedes Tuesday. Directness of precedence depends on the designer conceptualization.</rdfs:comment>
        <rdfs:isDefinedBy rdf:resource="https://w3id.org/hacid/onto/top-level"/>
        <rdfs:label xml:lang="en">directly precedes</rdfs:label>
        <rdfs:label xml:lang="it">precede direttamente</rdfs:label>
    </owl:ObjectProperty>
    


    <!-- https://w3id.org/hacid/onto/top-level/executesTask -->

    <owl:ObjectProperty rdf:about="https://w3id.org/hacid/onto/top-level/executesTask">
        <rdfs:subPropertyOf rdf:resource="https://w3id.org/hacid/onto/top-level/isClassifiedBy"/>
        <owl:inverseOf rdf:resource="https://w3id.org/hacid/onto/top-level/isExecutedIn"/>
        <rdfs:domain rdf:resource="https://w3id.org/hacid/onto/top-level/Action"/>
        <rdfs:range rdf:resource="https://w3id.org/hacid/onto/top-level/Task"/>
        <rdfs:comment xml:lang="en">A relation between an action and a task, e.g. 'putting some water in a pot and putting the pot on a fire until the water starts bubbling' executes the task 'boiling'.</rdfs:comment>
        <rdfs:isDefinedBy rdf:resource="https://w3id.org/hacid/onto/top-level"/>
        <rdfs:label xml:lang="it">esegue il task</rdfs:label>
        <rdfs:label xml:lang="en">executes task</rdfs:label>
    </owl:ObjectProperty>
    


    <!-- https://w3id.org/hacid/onto/top-level/follows -->

    <owl:ObjectProperty rdf:about="https://w3id.org/hacid/onto/top-level/follows">
        <rdfs:subPropertyOf rdf:resource="https://w3id.org/hacid/onto/top-level/associatedWith"/>
        <owl:inverseOf rdf:resource="https://w3id.org/hacid/onto/top-level/precedes"/>
        <rdf:type rdf:resource="http://www.w3.org/2002/07/owl#TransitiveProperty"/>
        <rdfs:domain rdf:resource="https://w3id.org/hacid/onto/top-level/Entity"/>
        <rdfs:range rdf:resource="https://w3id.org/hacid/onto/top-level/Entity"/>
        <rdfs:comment xml:lang="en">A relation between entities, expressing a 'sequence' schema.</rdfs:comment>
        <rdfs:comment xml:lang="it">Una relazione tra entità, che esprime uno schema di 'sequenza'.</rdfs:comment>
        <rdfs:isDefinedBy rdf:resource="https://w3id.org/hacid/onto/top-level"/>
        <rdfs:label xml:lang="en">follows</rdfs:label>
        <rdfs:label xml:lang="it">segue</rdfs:label>
    </owl:ObjectProperty>
    


    <!-- https://w3id.org/hacid/onto/top-level/hasAssignedRole -->

    <owl:ObjectProperty rdf:about="https://w3id.org/hacid/onto/top-level/hasAssignedRole">
        <rdfs:subPropertyOf rdf:resource="https://w3id.org/hacid/onto/top-level/associatedWith"/>
        <owl:inverseOf rdf:resource="https://w3id.org/hacid/onto/top-level/isAssignedRoleIn"/>
        <rdfs:domain rdf:resource="https://w3id.org/hacid/onto/top-level/ObjectRoleAssignment"/>
        <rdfs:range rdf:resource="https://w3id.org/hacid/onto/top-level/Role"/>
        <rdfs:isDefinedBy rdf:resource="https://w3id.org/hacid/onto/top-level"/>
        <rdfs:label xml:lang="en">has assigned role</rdfs:label>
        <rdfs:comment xml:lang="en">Associates the assignment with the assigned role.</rdfs:comment>
    </owl:ObjectProperty>
    


    <!-- https://w3id.org/hacid/onto/top-level/hasAssigneeObject -->

    <owl:ObjectProperty rdf:about="https://w3id.org/hacid/onto/top-level/hasAssigneeObject">
        <rdfs:subPropertyOf rdf:resource="https://w3id.org/hacid/onto/top-level/associatedWith"/>
        <owl:inverseOf rdf:resource="https://w3id.org/hacid/onto/top-level/isAssigneeObjectIn"/>
        <rdfs:domain rdf:resource="https://w3id.org/hacid/onto/top-level/ObjectRoleAssignment"/>
        <rdfs:range rdf:resource="https://w3id.org/hacid/onto/top-level/Object"/>
        <rdfs:isDefinedBy rdf:resource="https://w3id.org/hacid/onto/top-level"/>
        <rdfs:label xml:lang="en">has assignee object</rdfs:label>
        <rdfs:comment xml:lang="en">Associates the assignment with the object to which the corresponding role is assigned.</rdfs:comment>
    </owl:ObjectProperty>
    


    <!-- https://w3id.org/hacid/onto/top-level/hasBroader -->

    <owl:ObjectProperty rdf:about="https://w3id.org/hacid/onto/top-level/hasBroader">
        <rdfs:subPropertyOf rdf:resource="https://w3id.org/hacid/onto/top-level/associatedWith"/>
        <owl:inverseOf rdf:resource="https://w3id.org/hacid/onto/top-level/hasNarrower"/>
        <rdf:type rdf:resource="http://www.w3.org/2002/07/owl#TransitiveProperty"/>
        <rdfs:domain rdf:resource="https://w3id.org/hacid/onto/top-level/Concept"/>
        <rdfs:range rdf:resource="https://w3id.org/hacid/onto/top-level/Concept"/>
        <rdfs:comment xml:lang="it">La relazione per creare tassonomie di concetti dal più specifico al più generale.</rdfs:comment>
        <rdfs:comment xml:lang="en">The relation for creating hierarchies of concepts from the most specific to the most general.</rdfs:comment>
        <rdfs:isDefinedBy rdf:resource="https://w3id.org/hacid/onto/top-level"/>
        <rdfs:label xml:lang="it">ha più generale</rdfs:label>
        <rdfs:label xml:lang="en">has broader</rdfs:label>
    </owl:ObjectProperty>
    


    <!-- https://w3id.org/hacid/onto/top-level/hasCharacteristic -->

    <owl:ObjectProperty rdf:about="https://w3id.org/hacid/onto/top-level/hasCharacteristic">
        <rdfs:subPropertyOf rdf:resource="https://w3id.org/hacid/onto/top-level/associatedWith"/>
        <owl:inverseOf rdf:resource="https://w3id.org/hacid/onto/top-level/isCharacteristicOf"/>
        <rdfs:domain rdf:resource="https://w3id.org/hacid/onto/top-level/Entity"/>
        <rdfs:range rdf:resource="https://w3id.org/hacid/onto/top-level/Characteristic"/>
        <rdfs:comment xml:lang="it">La relazione di primo livello che intercorre tra un'entità e una delle sue caratteristiche.</rdfs:comment>
        <rdfs:comment xml:lang="en">The top-level relation holding between an entity and one of its characteristics.</rdfs:comment>
        <rdfs:isDefinedBy rdf:resource="https://w3id.org/hacid/onto/top-level"/>
        <rdfs:label xml:lang="it">ha caratteristica</rdfs:label>
        <rdfs:label xml:lang="en">has characteristic</rdfs:label>
    </owl:ObjectProperty>
    


    <!-- https://w3id.org/hacid/onto/top-level/hasCollection -->

    <owl:ObjectProperty rdf:about="https://w3id.org/hacid/onto/top-level/hasCollection">
        <rdfs:subPropertyOf rdf:resource="https://w3id.org/hacid/onto/top-level/associatedWith"/>
        <owl:inverseOf rdf:resource="https://w3id.org/hacid/onto/top-level/isCollectionOf"/>
        <rdfs:domain rdf:resource="https://w3id.org/hacid/onto/top-level/Entity"/>
        <rdfs:range rdf:resource="https://w3id.org/hacid/onto/top-level/Collection"/>
        <rdfs:comment xml:lang="it">La relazione esistente tra un'entità ed una collezione.</rdfs:comment>
        <rdfs:comment xml:lang="en">The relation holding between an entity and a collection.</rdfs:comment>
        <rdfs:isDefinedBy rdf:resource="https://w3id.org/hacid/onto/top-level"/>
        <rdfs:label xml:lang="it">ha collezione</rdfs:label>
        <rdfs:label xml:lang="en">has collection</rdfs:label>
    </owl:ObjectProperty>
    


    <!-- https://w3id.org/hacid/onto/top-level/hasCreator -->

    <owl:ObjectProperty rdf:about="https://w3id.org/hacid/onto/top-level/hasCreator">
        <rdfs:subPropertyOf rdf:resource="https://w3id.org/hacid/onto/top-level/associatedWith"/>
        <owl:inverseOf rdf:resource="https://w3id.org/hacid/onto/top-level/isCreatorOf"/>
        <rdfs:domain rdf:resource="https://w3id.org/hacid/onto/top-level/Entity"/>
        <rdfs:comment xml:lang="it">Relazione per associare ad un'entità un agente creatore.</rdfs:comment>
        <rdfs:comment xml:lang="en">The relation for associating an entity to an agent being the creator.</rdfs:comment>
        <rdfs:isDefinedBy rdf:resource="https://w3id.org/hacid/onto/top-level"/>
        <rdfs:label xml:lang="it">ha creatore</rdfs:label>
        <rdfs:label xml:lang="en">has creator</rdfs:label>
    </owl:ObjectProperty>
    


    <!-- https://w3id.org/hacid/onto/top-level/hasDataSchema -->

    <owl:ObjectProperty rdf:about="https://w3id.org/hacid/onto/top-level/hasDataSchema">
        <rdfs:subPropertyOf rdf:resource="https://w3id.org/hacid/onto/top-level/hasDescription"/>
        <owl:inverseOf rdf:resource="https://w3id.org/hacid/onto/top-level/isDataSchemaOf"/>
        <rdfs:domain rdf:resource="https://w3id.org/hacid/onto/top-level/Media"/>
        <rdfs:range rdf:resource="https://w3id.org/hacid/onto/top-level/DataSchema"/>
        <rdfs:comment xml:lang="it">La relazione che sussiste tra un media e il suo schema di dati.</rdfs:comment>
        <rdfs:comment xml:lang="en">The relation holding between a media and its data schema.</rdfs:comment>
        <rdfs:isDefinedBy rdf:resource="https://w3id.org/hacid/onto/top-level"/>
        <rdfs:label xml:lang="it">ha schema di dati</rdfs:label>
        <rdfs:label xml:lang="en">has data schema</rdfs:label>
    </owl:ObjectProperty>
    


    <!-- https://w3id.org/hacid/onto/top-level/hasDescription -->

    <owl:ObjectProperty rdf:about="https://w3id.org/hacid/onto/top-level/hasDescription">
        <rdfs:subPropertyOf rdf:resource="https://w3id.org/hacid/onto/top-level/associatedWith"/>
        <owl:inverseOf rdf:resource="https://w3id.org/hacid/onto/top-level/isDescriptionOf"/>
        <rdfs:domain rdf:resource="https://w3id.org/hacid/onto/top-level/Entity"/>
        <rdfs:range rdf:resource="https://w3id.org/hacid/onto/top-level/Description"/>
        <rdfs:comment xml:lang="en">Property that associates an entity with its description.</rdfs:comment>
        <rdfs:comment xml:lang="it">Proprietà che associa un'entità alla sua descrizione.</rdfs:comment>
        <rdfs:isDefinedBy rdf:resource="https://w3id.org/hacid/onto/top-level"/>
        <rdfs:label xml:lang="it">ha descrizione</rdfs:label>
        <rdfs:label xml:lang="en">has description</rdfs:label>
    </owl:ObjectProperty>
    


    <!-- https://w3id.org/hacid/onto/top-level/hasDownloadURL -->

    <owl:ObjectProperty rdf:about="https://w3id.org/hacid/onto/top-level/hasDownloadURL">
        <rdfs:subPropertyOf rdf:resource="https://w3id.org/hacid/onto/top-level/associatedWith"/>
        <rdfs:domain rdf:resource="https://w3id.org/hacid/onto/top-level/Media"/>
        <rdfs:comment xml:lang="it">Questo è un link diretto al file scaricabile in un dato formato. E.g. un file CSV o un file RDF. Il formato è descritto dal dct:format e/o dal dcat:mediaType della distribuzione.</rdfs:comment>
        <rdfs:comment xml:lang="en">The URL of the downloadable file in a given format. E.g. CSV file or RDF file. The format is indicated by the distribution's dct:format and/or dcat:mediaType.</rdfs:comment>
        <rdfs:isDefinedBy rdf:resource="https://w3id.org/hacid/onto/top-level"/>
        <rdfs:label xml:lang="it">ha URL di scaricamento</rdfs:label>
        <rdfs:label xml:lang="en">has download URL</rdfs:label>
    </owl:ObjectProperty>
    


    <!-- https://w3id.org/hacid/onto/top-level/hasEventuality -->

    <owl:ObjectProperty rdf:about="https://w3id.org/hacid/onto/top-level/hasEventuality">
        <rdfs:subPropertyOf rdf:resource="https://w3id.org/hacid/onto/top-level/associatedWith"/>
        <owl:inverseOf rdf:resource="https://w3id.org/hacid/onto/top-level/isEventualityOf"/>
        <rdfs:domain rdf:resource="https://w3id.org/hacid/onto/top-level/Entity"/>
        <rdfs:range rdf:resource="https://w3id.org/hacid/onto/top-level/Situation"/>
        <rdfs:comment xml:lang="it">La relazione esistente tra una qualsiasi entità ed una di tipo Eventualità.</rdfs:comment>
        <rdfs:comment xml:lang="en">The relationship existing between any entity and another typed as Eventuality.</rdfs:comment>
        <rdfs:isDefinedBy rdf:resource="https://w3id.org/hacid/onto/top-level"/>
        <rdfs:label xml:lang="it">ha eventualità</rdfs:label>
        <rdfs:label xml:lang="en">has eventuality</rdfs:label>
    </owl:ObjectProperty>
    


    <!-- https://w3id.org/hacid/onto/top-level/hasIdentifierSchema -->

    <owl:ObjectProperty rdf:about="https://w3id.org/hacid/onto/top-level/hasIdentifierSchema">
        <rdfs:subPropertyOf rdf:resource="https://w3id.org/hacid/onto/top-level/hasDescription"/>
        <owl:inverseOf rdf:resource="https://w3id.org/hacid/onto/top-level/isIdentifierSchemaOf"/>
        <rdfs:range rdf:resource="https://w3id.org/hacid/onto/top-level/IdentifierSchema"/>
        <rdfs:comment xml:lang="it">La relazione che lega un identificativo unico al suo schema di definizione.</rdfs:comment>
        <rdfs:comment xml:lang="en">The relation that associates a unique identifier to its defining schema.</rdfs:comment>
        <rdfs:isDefinedBy rdf:resource="https://w3id.org/hacid/onto/top-level"/>
        <rdfs:label xml:lang="it">ha schema di identificazione</rdfs:label>
        <rdfs:label xml:lang="en">has identifier schema</rdfs:label>
    </owl:ObjectProperty>
    


    <!-- https://w3id.org/hacid/onto/top-level/hasInputRole -->

    <owl:ObjectProperty rdf:about="https://w3id.org/hacid/onto/top-level/hasInputRole">
        <rdfs:subPropertyOf rdf:resource="https://w3id.org/hacid/onto/top-level/associatedWith"/>
        <owl:inverseOf rdf:resource="https://w3id.org/hacid/onto/top-level/isInputRoleOf"/>
        <rdfs:domain rdf:resource="https://w3id.org/hacid/onto/top-level/Task"/>
        <rdfs:range rdf:resource="https://w3id.org/hacid/onto/top-level/Role"/>
        <rdfs:comment xml:lang="en">Associates a task with roles that are expected to be fulfilled by objects consumed by any action executing the task.</rdfs:comment>
        <rdfs:isDefinedBy rdf:resource="https://w3id.org/hacid/onto/top-level"/>
        <rdfs:label xml:lang="en">has input role</rdfs:label>
    </owl:ObjectProperty>
    


    <!-- https://w3id.org/hacid/onto/top-level/hasLocation -->

    <owl:ObjectProperty rdf:about="https://w3id.org/hacid/onto/top-level/hasLocation">
        <rdfs:subPropertyOf rdf:resource="https://w3id.org/hacid/onto/top-level/associatedWith"/>
        <owl:inverseOf rdf:resource="https://w3id.org/hacid/onto/top-level/isLocationOf"/>
        <rdfs:domain rdf:resource="https://w3id.org/hacid/onto/top-level/Entity"/>
        <rdfs:range rdf:resource="https://w3id.org/hacid/onto/top-level/Location"/>
        <rdfs:comment xml:lang="it">La relazione esistente tra un qualsiasi tipo di entità ed un luogo.</rdfs:comment>
        <rdfs:comment xml:lang="en">The relation holding between any kind of entity and a place.</rdfs:comment>
        <rdfs:isDefinedBy rdf:resource="https://w3id.org/hacid/onto/top-level"/>
        <rdfs:label xml:lang="it">ha luogo</rdfs:label>
        <rdfs:label xml:lang="en">has place</rdfs:label>
    </owl:ObjectProperty>
    


    <!-- https://w3id.org/hacid/onto/top-level/hasMedia -->

    <owl:ObjectProperty rdf:about="https://w3id.org/hacid/onto/top-level/hasMedia">
        <rdfs:subPropertyOf rdf:resource="https://w3id.org/hacid/onto/top-level/associatedWith"/>
        <owl:inverseOf rdf:resource="https://w3id.org/hacid/onto/top-level/isMediaOf"/>
        <rdfs:domain rdf:resource="https://w3id.org/hacid/onto/top-level/Entity"/>
        <rdfs:range rdf:resource="https://w3id.org/hacid/onto/top-level/Media"/>
        <rdfs:comment xml:lang="it">La relazione tra un'entità ed un'istanza della classe Media.</rdfs:comment>
        <rdfs:comment xml:lang="en">The relationship between an entity and an instance of the middle class.</rdfs:comment>
        <rdfs:isDefinedBy rdf:resource="https://w3id.org/hacid/onto/top-level"/>
        <rdfs:label xml:lang="it">ha media</rdfs:label>
        <rdfs:label xml:lang="en">has media</rdfs:label>
    </owl:ObjectProperty>
    


    <!-- https://w3id.org/hacid/onto/top-level/hasMember -->

    <owl:ObjectProperty rdf:about="https://w3id.org/hacid/onto/top-level/hasMember">
        <rdfs:subPropertyOf rdf:resource="https://w3id.org/hacid/onto/top-level/associatedWith"/>
        <owl:inverseOf rdf:resource="https://w3id.org/hacid/onto/top-level/isMemberOf"/>
        <rdfs:domain rdf:resource="https://w3id.org/hacid/onto/top-level/Collection"/>
        <rdfs:range rdf:resource="https://w3id.org/hacid/onto/top-level/Entity"/>
        <rdfs:comment xml:lang="it">La relazione di membership.</rdfs:comment>
        <rdfs:comment xml:lang="en">The membership relation.</rdfs:comment>
        <rdfs:isDefinedBy rdf:resource="https://w3id.org/hacid/onto/top-level"/>
        <rdfs:label xml:lang="it">ha membro</rdfs:label>
        <rdfs:label xml:lang="en">has member</rdfs:label>
    </owl:ObjectProperty>
    


    <!-- https://w3id.org/hacid/onto/top-level/hasNarrower -->

    <owl:ObjectProperty rdf:about="https://w3id.org/hacid/onto/top-level/hasNarrower">
        <rdfs:subPropertyOf rdf:resource="https://w3id.org/hacid/onto/top-level/associatedWith"/>
        <rdf:type rdf:resource="http://www.w3.org/2002/07/owl#TransitiveProperty"/>
        <rdfs:domain rdf:resource="https://w3id.org/hacid/onto/top-level/Concept"/>
        <rdfs:range rdf:resource="https://w3id.org/hacid/onto/top-level/Concept"/>
        <rdfs:comment xml:lang="it">La relazione per creare tassonomie di concetti dal più generale al più specifico.</rdfs:comment>
        <rdfs:comment xml:lang="en">The relation for generating taxonomies of concepts from the most general to the most specific.</rdfs:comment>
        <rdfs:isDefinedBy rdf:resource="https://w3id.org/hacid/onto/top-level"/>
        <rdfs:label xml:lang="it">ha più specifico</rdfs:label>
        <rdfs:label xml:lang="en">has narrower</rdfs:label>
    </owl:ObjectProperty>
    


    <!-- https://w3id.org/hacid/onto/top-level/hasOutput -->

    <owl:ObjectProperty rdf:about="https://w3id.org/hacid/onto/top-level/hasOutput">
        <rdfs:isDefinedBy rdf:resource="https://w3id.org/hacid/onto/top-level"/>
        <rdfs:domain rdf:resource="https://w3id.org/hacid/onto/top-level/Action"/>
        <rdfs:range rdf:resource="https://w3id.org/hacid/onto/top-level/Object"/>
        <rdfs:label xml:lang="en">has output</rdfs:label>
        <rdfs:comment xml:lang="en">Associates an action with a produced object. The object typically fulfills one the output roles of the executed task.</rdfs:comment>
    </owl:ObjectProperty>
    


    <!-- https://w3id.org/hacid/onto/top-level/hasOutputRole -->

    <owl:ObjectProperty rdf:about="https://w3id.org/hacid/onto/top-level/hasOutputRole">
        <rdfs:subPropertyOf rdf:resource="https://w3id.org/hacid/onto/top-level/associatedWith"/>
        <owl:inverseOf rdf:resource="https://w3id.org/hacid/onto/top-level/isOutputRoleOf"/>
        <rdfs:domain rdf:resource="https://w3id.org/hacid/onto/top-level/Task"/>
        <rdfs:range rdf:resource="https://w3id.org/hacid/onto/top-level/Role"/>
        <rdfs:comment xml:lang="en">Associates a task with roles that are expected to be fulfilled by objects produced by any action executing the task.</rdfs:comment>
        <rdfs:isDefinedBy rdf:resource="https://w3id.org/hacid/onto/top-level"/>
        <rdfs:label xml:lang="en">has output role</rdfs:label>
    </owl:ObjectProperty>
    


    <!-- https://w3id.org/hacid/onto/top-level/hasPart -->

    <owl:ObjectProperty rdf:about="https://w3id.org/hacid/onto/top-level/hasPart">
        <rdfs:subPropertyOf rdf:resource="https://w3id.org/hacid/onto/top-level/associatedWith"/>
        <owl:inverseOf rdf:resource="https://w3id.org/hacid/onto/top-level/isPartOf"/>
        <rdf:type rdf:resource="http://www.w3.org/2002/07/owl#TransitiveProperty"/>
        <rdf:type rdf:resource="http://www.w3.org/2002/07/owl#ReflexiveProperty"/>
        <rdfs:domain rdf:resource="https://w3id.org/hacid/onto/top-level/Entity"/>
        <rdfs:range rdf:resource="https://w3id.org/hacid/onto/top-level/Entity"/>
        <rdfs:comment xml:lang="it">La relazione di parte definita come proprietà transitiva e riflessiva.</rdfs:comment>
        <rdfs:comment xml:lang="en">The parthood relation defined as a transitive and reflexive property.</rdfs:comment>
        <rdfs:isDefinedBy rdf:resource="https://w3id.org/hacid/onto/top-level"/>
        <rdfs:label xml:lang="it">ha parte</rdfs:label>
        <rdfs:label xml:lang="en">has part</rdfs:label>
    </owl:ObjectProperty>
    


    <!-- https://w3id.org/hacid/onto/top-level/hasParticipant -->

    <owl:ObjectProperty rdf:about="https://w3id.org/hacid/onto/top-level/hasParticipant">
        <rdfs:subPropertyOf rdf:resource="https://w3id.org/hacid/onto/top-level/associatedWith"/>
        <owl:inverseOf rdf:resource="https://w3id.org/hacid/onto/top-level/isParticipantIn"/>
        <rdfs:domain rdf:resource="https://w3id.org/hacid/onto/top-level/Event"/>
        <rdfs:range rdf:resource="https://w3id.org/hacid/onto/top-level/Object"/>
        <rdfs:comment xml:lang="en">A relation between an object and a process, e.g. 'John took part in the discussion', 'a large mass of snow fell during the avalanche', or 'a cook, some sugar, flour, etc. are all present in the cooking of a cake'.</rdfs:comment>
        <rdfs:isDefinedBy rdf:resource="https://w3id.org/hacid/onto/top-level"/>
        <rdfs:label xml:lang="it">ha come partecipante</rdfs:label>
        <rdfs:label xml:lang="en">has participant</rdfs:label>
    </owl:ObjectProperty>
    


    <!-- https://w3id.org/hacid/onto/top-level/hasProperPart -->

    <owl:ObjectProperty rdf:about="https://w3id.org/hacid/onto/top-level/hasProperPart">
        <rdfs:subPropertyOf rdf:resource="https://w3id.org/hacid/onto/top-level/hasPart"/>
        <owl:inverseOf rdf:resource="https://w3id.org/hacid/onto/top-level/isProperPartOf"/>
        <rdf:type rdf:resource="http://www.w3.org/2002/07/owl#AsymmetricProperty"/>
        <rdfs:domain rdf:resource="https://w3id.org/hacid/onto/top-level/Entity"/>
        <rdfs:range rdf:resource="https://w3id.org/hacid/onto/top-level/Entity"/>
        <rdfs:comment xml:lang="it">La proprietà per rappresentare la relazione di composizionalità tra un oggetto ed i suoi componenti diretti.</rdfs:comment>
        <rdfs:comment xml:lang="en">The property for representing compositionality between objects and their direct components.</rdfs:comment>
        <rdfs:isDefinedBy rdf:resource="https://w3id.org/hacid/onto/top-level"/>
        <rdfs:label xml:lang="it">ha parte propria</rdfs:label>
        <rdfs:label xml:lang="en">has proper part</rdfs:label>
    </owl:ObjectProperty>
    


    <!-- https://w3id.org/hacid/onto/top-level/hasRegion -->

    <owl:ObjectProperty rdf:about="https://w3id.org/hacid/onto/top-level/hasRegion">
        <rdfs:subPropertyOf rdf:resource="https://w3id.org/hacid/onto/top-level/associatedWith"/>
        <owl:inverseOf rdf:resource="https://w3id.org/hacid/onto/top-level/isRegionFor"/>
        <rdfs:domain rdf:resource="https://w3id.org/hacid/onto/top-level/Entity"/>
        <rdfs:range rdf:resource="https://w3id.org/hacid/onto/top-level/Region"/>
        <rdfs:comment xml:lang="en">A relation between entities and regions, e.g. 'the number of wheels of that truck is 12', 'the time of the experiment is August 9th, 2004', 'the whale has been localized at 34 degrees E, 20 degrees S'.</rdfs:comment>
        <rdfs:comment xml:lang="it">Una relazione tra entità e regioni, ad es. 'il numero di ruote di quel camion è 12', 'l'ora dell'esperimento è il 9 agosto 2004', 'la balena è stata localizzata a 34 gradi E, 20 gradi S'</rdfs:comment>
        <rdfs:isDefinedBy rdf:resource="https://w3id.org/hacid/onto/top-level"/>
        <rdfs:label xml:lang="it">ha attributo</rdfs:label>
        <rdfs:label xml:lang="en">has region</rdfs:label>
    </owl:ObjectProperty>
    


    <!-- https://w3id.org/hacid/onto/top-level/hasRole -->

    <owl:ObjectProperty rdf:about="https://w3id.org/hacid/onto/top-level/hasRole">
        <rdfs:subPropertyOf rdf:resource="https://w3id.org/hacid/onto/top-level/isClassifiedBy"/>
        <owl:inverseOf rdf:resource="https://w3id.org/hacid/onto/top-level/isRoleOf"/>
        <rdfs:domain rdf:resource="https://w3id.org/hacid/onto/top-level/Entity"/>
        <rdfs:range rdf:resource="https://w3id.org/hacid/onto/top-level/Role"/>
        <rdfs:comment xml:lang="it">La relazione che permette di classificare un'entità in base al ruolo che essa ricopre.</rdfs:comment>
        <rdfs:comment xml:lang="en">The relationship that allows you to classify an entity based on the role it holds.</rdfs:comment>
        <rdfs:isDefinedBy rdf:resource="https://w3id.org/hacid/onto/top-level"/>
        <rdfs:label xml:lang="it">ha il ruolo</rdfs:label>
        <rdfs:label xml:lang="en">has role</rdfs:label>
    </owl:ObjectProperty>
    


    <!-- https://w3id.org/hacid/onto/top-level/hasSchemaAttribute -->

    <owl:ObjectProperty rdf:about="https://w3id.org/hacid/onto/top-level/hasSchemaAttribute">
        <rdfs:subPropertyOf rdf:resource="https://w3id.org/hacid/onto/top-level/hasCharacteristic"/>
        <owl:inverseOf rdf:resource="https://w3id.org/hacid/onto/top-level/isSchemaAttributeOf"/>
        <rdfs:domain rdf:resource="https://w3id.org/hacid/onto/top-level/DataSchema"/>
        <rdfs:range rdf:resource="https://w3id.org/hacid/onto/top-level/SchemaAttribute"/>
        <rdfs:comment xml:lang="it">La relazione che consente di associare uno schema di dati ai suoi attributi dello schema.</rdfs:comment>
        <rdfs:comment xml:lang="en">The relation that allows one to associate a data schema with its schema attributes.</rdfs:comment>
        <rdfs:isDefinedBy rdf:resource="https://w3id.org/hacid/onto/top-level"/>
        <rdfs:label xml:lang="it">ha attributo di schema di dati</rdfs:label>
        <rdfs:label xml:lang="en">has data schema attribute</rdfs:label>
    </owl:ObjectProperty>
    


    <!-- https://w3id.org/hacid/onto/top-level/hasSetting -->

    <owl:ObjectProperty rdf:about="https://w3id.org/hacid/onto/top-level/hasSetting">
        <rdfs:subPropertyOf rdf:resource="https://w3id.org/hacid/onto/top-level/associatedWith"/>
        <owl:inverseOf rdf:resource="https://w3id.org/hacid/onto/top-level/isSettingFor"/>
        <rdfs:domain rdf:resource="https://w3id.org/hacid/onto/top-level/Entity"/>
        <rdfs:range rdf:resource="https://w3id.org/hacid/onto/top-level/Situation"/>
        <rdfs:comment xml:lang="en">A relation between entities and situations, e.g. 'this morning I've prepared my coffee with a new fantastic Arabica', i.e.: (an amount of) a new fantastic Arabica hasSetting the preparation of my coffee this morning.</rdfs:comment>
        <rdfs:isDefinedBy rdf:resource="https://w3id.org/hacid/onto/top-level"/>
        <rdfs:label xml:lang="en">has setting</rdfs:label>
        <rdfs:label xml:lang="it">è nel contesto di</rdfs:label>
    </owl:ObjectProperty>
    


    <!-- https://w3id.org/hacid/onto/top-level/hasSource -->

    <owl:ObjectProperty rdf:about="https://w3id.org/hacid/onto/top-level/hasSource">
        <rdfs:subPropertyOf rdf:resource="https://w3id.org/hacid/onto/top-level/associatedWith"/>
        <owl:inverseOf rdf:resource="https://w3id.org/hacid/onto/top-level/isSouceOf"/>
        <rdfs:domain rdf:resource="https://w3id.org/hacid/onto/top-level/Entity"/>
        <rdfs:range rdf:resource="https://w3id.org/hacid/onto/top-level/Entity"/>
        <rdfs:comment xml:lang="it">La relazione che permette di stabilire che una certa entità è sorgente di un'altra.</rdfs:comment>
        <rdfs:comment xml:lang="en">The relation that allows one that a certain entity is the source of another.</rdfs:comment>
        <rdfs:isDefinedBy rdf:resource="https://w3id.org/hacid/onto/top-level"/>
        <rdfs:label xml:lang="it">ha sorgente</rdfs:label>
        <rdfs:label xml:lang="en">has source</rdfs:label>
    </owl:ObjectProperty>
    


    <!-- https://w3id.org/hacid/onto/top-level/hasSystem -->

    <owl:ObjectProperty rdf:about="https://w3id.org/hacid/onto/top-level/hasSystem">
        <rdfs:subPropertyOf rdf:resource="https://w3id.org/hacid/onto/top-level/associatedWith"/>
        <owl:inverseOf rdf:resource="https://w3id.org/hacid/onto/top-level/isSystemOf"/>
        <rdfs:domain rdf:resource="https://w3id.org/hacid/onto/top-level/Entity"/>
        <rdfs:range rdf:resource="https://w3id.org/hacid/onto/top-level/System"/>
        <rdfs:comment xml:lang="it">La relazione che sussiste tra una qualsiasi entità ed un sistema.</rdfs:comment>
        <rdfs:comment xml:lang="en">The relation holding between any entity and a system.</rdfs:comment>
        <rdfs:isDefinedBy rdf:resource="https://w3id.org/hacid/onto/top-level"/>
        <rdfs:label xml:lang="en">has system</rdfs:label>
    </owl:ObjectProperty>
    


    <!-- https://w3id.org/hacid/onto/top-level/hasTask -->

    <owl:ObjectProperty rdf:about="https://w3id.org/hacid/onto/top-level/hasTask">
        <rdfs:subPropertyOf rdf:resource="https://w3id.org/hacid/onto/top-level/isRelatedToConcept"/>
        <owl:inverseOf rdf:resource="https://w3id.org/hacid/onto/top-level/isTaskOf"/>
        <rdfs:domain rdf:resource="https://w3id.org/hacid/onto/top-level/Role"/>
        <rdfs:range rdf:resource="https://w3id.org/hacid/onto/top-level/Task"/>
        <rdfs:comment xml:lang="en">A relation between roles and tasks, e.g. 'students have the duty of giving exams' (i.e. the Role 'student' hasTask the Task 'giving exams').</rdfs:comment>
        <rdfs:isDefinedBy rdf:resource="https://w3id.org/hacid/onto/top-level"/>
        <rdfs:label xml:lang="it">ha come obiettivo</rdfs:label>
        <rdfs:label xml:lang="en">has task</rdfs:label>
    </owl:ObjectProperty>
    


    <!-- https://w3id.org/hacid/onto/top-level/hasTimeInterval -->

    <owl:ObjectProperty rdf:about="https://w3id.org/hacid/onto/top-level/hasTimeInterval">
        <rdfs:subPropertyOf rdf:resource="https://w3id.org/hacid/onto/top-level/hasRegion"/>
        <owl:inverseOf rdf:resource="https://w3id.org/hacid/onto/top-level/isTimeIntervalOf"/>
        <rdfs:domain rdf:resource="https://w3id.org/hacid/onto/top-level/Event"/>
        <rdfs:range rdf:resource="https://w3id.org/hacid/onto/top-level/TimeInterval"/>
        <rdfs:comment xml:lang="it">La relazione generica tra eventi e intervalli di tempo.</rdfs:comment>
        <rdfs:comment xml:lang="en">The generic relation between events and time intervals.</rdfs:comment>
        <rdfs:isDefinedBy rdf:resource="https://w3id.org/hacid/onto/top-level"/>
        <rdfs:label xml:lang="it">ha intervallo temporale</rdfs:label>
        <rdfs:label xml:lang="en">has time interval</rdfs:label>
    </owl:ObjectProperty>
    


    <!-- https://w3id.org/hacid/onto/top-level/hasUniqueIdentifier -->

    <owl:ObjectProperty rdf:about="https://w3id.org/hacid/onto/top-level/hasUniqueIdentifier">
        <rdfs:subPropertyOf rdf:resource="https://w3id.org/hacid/onto/top-level/hasCharacteristic"/>
        <owl:inverseOf rdf:resource="https://w3id.org/hacid/onto/top-level/isUniqueIdentifierOf"/>
        <rdfs:domain rdf:resource="https://w3id.org/hacid/onto/top-level/Entity"/>
        <rdfs:comment xml:lang="it">La relazione esistente tra un'entità e il suo identificatore univoco.</rdfs:comment>
        <rdfs:comment xml:lang="en">The relation holding between an entity and its unique identifier.</rdfs:comment>
        <rdfs:isDefinedBy rdf:resource="https://w3id.org/hacid/onto/top-level"/>
        <rdfs:label xml:lang="it">ha identificativo univoco</rdfs:label>
        <rdfs:label xml:lang="en">has unique identifier</rdfs:label>
    </owl:ObjectProperty>
    


    <!-- https://w3id.org/hacid/onto/top-level/hasUnitOfMeasure -->

    <owl:ObjectProperty rdf:about="https://w3id.org/hacid/onto/top-level/hasUnitOfMeasure">
        <rdfs:subPropertyOf rdf:resource="https://w3id.org/hacid/onto/top-level/hasCharacteristic"/>
        <owl:inverseOf rdf:resource="https://w3id.org/hacid/onto/top-level/isUnitOfMeasureOf"/>
        <rdfs:domain rdf:resource="https://w3id.org/hacid/onto/top-level/Entity"/>
        <rdfs:range rdf:resource="https://w3id.org/hacid/onto/top-level/UnitOfMeasure"/>
        <rdfs:comment xml:lang="en">Property that links an object that can be measured to its corresponding unit of measure.</rdfs:comment>
        <rdfs:comment xml:lang="it">Proprietà che collega un oggetto misurabile alla sua unità di misura corrispondente.</rdfs:comment>
        <rdfs:isDefinedBy rdf:resource="https://w3id.org/hacid/onto/top-level"/>
        <rdfs:label xml:lang="it">ha unità di misura</rdfs:label>
        <rdfs:label xml:lang="en">has unit of measure</rdfs:label>
    </owl:ObjectProperty>
    


    <!-- https://w3id.org/hacid/onto/top-level/hasValue -->

    <owl:ObjectProperty rdf:about="https://w3id.org/hacid/onto/top-level/hasValue">
        <rdfs:subPropertyOf rdf:resource="https://w3id.org/hacid/onto/top-level/hasCharacteristic"/>
        <owl:inverseOf rdf:resource="https://w3id.org/hacid/onto/top-level/isValueOf"/>
        <rdfs:domain rdf:resource="https://w3id.org/hacid/onto/top-level/Entity"/>
        <rdfs:range rdf:resource="https://w3id.org/hacid/onto/top-level/Value"/>
        <rdfs:comment xml:lang="it">La relazione esistente tra un'entità ed il valore ad essa associata.</rdfs:comment>
        <rdfs:comment xml:lang="en">The relationship between an entity and the value it is associated with.</rdfs:comment>
        <rdfs:isDefinedBy rdf:resource="https://w3id.org/hacid/onto/top-level"/>
        <rdfs:label xml:lang="it">ha valore</rdfs:label>
        <rdfs:label xml:lang="en">has value</rdfs:label>
    </owl:ObjectProperty>
    


    <!-- https://w3id.org/hacid/onto/top-level/includesEvent -->

    <owl:ObjectProperty rdf:about="https://w3id.org/hacid/onto/top-level/includesEvent">
        <rdfs:comment xml:lang="en">A relation between situations and events, e.g. 'this morning I've prepared my coffee and had my fingers burnt' (i.e.: the preparation of my coffee this morning included a burning of my fingers).</rdfs:comment>
        <rdfs:isDefinedBy rdf:resource="https://w3id.org/hacid/onto/top-level"/>
        <rdfs:label xml:lang="it">include l'evento</rdfs:label>
        <rdfs:label xml:lang="en">includes event</rdfs:label>
    </owl:ObjectProperty>
    


    <!-- https://w3id.org/hacid/onto/top-level/includesObject -->

    <owl:ObjectProperty rdf:about="https://w3id.org/hacid/onto/top-level/includesObject">
        <rdfs:comment xml:lang="en">A relation between situations and objects, e.g. 'this morning I've prepared my coffee and had my fingers burnt' (i.e.: the preparation of my coffee this morning included me).</rdfs:comment>
        <rdfs:isDefinedBy rdf:resource="https://w3id.org/hacid/onto/top-level"/>
        <rdfs:label xml:lang="it">include l'oggetto</rdfs:label>
        <rdfs:label xml:lang="en">includes object</rdfs:label>
    </owl:ObjectProperty>
    


    <!-- https://w3id.org/hacid/onto/top-level/involves -->

    <owl:ObjectProperty rdf:about="https://w3id.org/hacid/onto/top-level/involves">
        <rdfs:subPropertyOf rdf:resource="https://w3id.org/hacid/onto/top-level/associatedWith"/>
        <owl:inverseOf rdf:resource="https://w3id.org/hacid/onto/top-level/isInvolvedIn"/>
        <rdfs:domain rdf:resource="https://w3id.org/hacid/onto/top-level/Situation"/>
        <rdfs:range rdf:resource="https://w3id.org/hacid/onto/top-level/Entity"/>
        <rdfs:comment xml:lang="it">La proprietà per collegare una situazione con i suoi argomenti.</rdfs:comment>
        <rdfs:comment xml:lang="it">Questa proprietà permette di collegare una situazione con le entità che costituiscono i suoi argomenti.</rdfs:comment>
        <rdfs:comment xml:lang="en">The property for associating a situation with its arguments.</rdfs:comment>
        <rdfs:isDefinedBy rdf:resource="https://w3id.org/hacid/onto/top-level"/>
        <rdfs:label xml:lang="it">coinvolge</rdfs:label>
        <rdfs:label xml:lang="en">involves</rdfs:label>
    </owl:ObjectProperty>
    


    <!-- https://w3id.org/hacid/onto/top-level/isAssignedRoleIn -->

    <owl:ObjectProperty rdf:about="https://w3id.org/hacid/onto/top-level/isAssignedRoleIn">
        <rdfs:subPropertyOf rdf:resource="https://w3id.org/hacid/onto/top-level/associatedWith"/>
        <rdfs:domain rdf:resource="https://w3id.org/hacid/onto/top-level/Role"/>
        <rdfs:range rdf:resource="https://w3id.org/hacid/onto/top-level/ObjectRoleAssignment"/>
        <rdfs:isDefinedBy rdf:resource="https://w3id.org/hacid/onto/top-level"/>
        <rdfs:label xml:lang="en">is assigned role in</rdfs:label>
        <rdfs:comment xml:lang="en">Associates a role with an assignment of that role.</rdfs:comment>
    </owl:ObjectProperty>
    


    <!-- https://w3id.org/hacid/onto/top-level/isAssigneeObjectIn -->

    <owl:ObjectProperty rdf:about="https://w3id.org/hacid/onto/top-level/isAssigneeObjectIn">
        <rdfs:subPropertyOf rdf:resource="https://w3id.org/hacid/onto/top-level/associatedWith"/>
        <rdfs:domain rdf:resource="https://w3id.org/hacid/onto/top-level/Object"/>
        <rdfs:range rdf:resource="https://w3id.org/hacid/onto/top-level/ObjectRoleAssignment"/>
        <rdfs:isDefinedBy rdf:resource="https://w3id.org/hacid/onto/top-level"/>
        <rdfs:label xml:lang="en">is assignee object in</rdfs:label>
        <rdfs:comment xml:lang="en">Associates an object with an assignment of some role to such object.</rdfs:comment>
    </owl:ObjectProperty>
    


    <!-- https://w3id.org/hacid/onto/top-level/isCharacteristicOf -->

    <owl:ObjectProperty rdf:about="https://w3id.org/hacid/onto/top-level/isCharacteristicOf">
        <rdfs:subPropertyOf rdf:resource="https://w3id.org/hacid/onto/top-level/associatedWith"/>
        <rdfs:domain rdf:resource="https://w3id.org/hacid/onto/top-level/Characteristic"/>
        <rdfs:range rdf:resource="https://w3id.org/hacid/onto/top-level/Entity"/>
        <rdfs:comment xml:lang="it">La relazione che collega una caratteristica all'entità a cui essa può essere associata.</rdfs:comment>
        <rdfs:comment xml:lang="en">The relationship that links a characteristic to the entity it can be associated with.</rdfs:comment>
        <rdfs:isDefinedBy rdf:resource="https://w3id.org/hacid/onto/top-level"/>
        <rdfs:label xml:lang="en">is characteristic of</rdfs:label>
        <rdfs:label xml:lang="it">è caratteristica di</rdfs:label>
    </owl:ObjectProperty>
    


    <!-- https://w3id.org/hacid/onto/top-level/isClassifiedBy -->

    <owl:ObjectProperty rdf:about="https://w3id.org/hacid/onto/top-level/isClassifiedBy">
        <rdfs:subPropertyOf rdf:resource="https://w3id.org/hacid/onto/top-level/associatedWith"/>
        <rdfs:domain rdf:resource="https://w3id.org/hacid/onto/top-level/Entity"/>
        <rdfs:range rdf:resource="https://w3id.org/hacid/onto/top-level/Concept"/>
        <rdfs:comment xml:lang="it">La proprietà per stabilire che un certo concetto viene usato per classificare una certa entità.</rdfs:comment>
        <rdfs:comment xml:lang="en">The property to state that a certain concept is used to classify a certain entity.</rdfs:comment>
        <rdfs:isDefinedBy rdf:resource="https://w3id.org/hacid/onto/top-level"/>
        <rdfs:label xml:lang="en">is classified by</rdfs:label>
        <rdfs:label xml:lang="it">è classificato da</rdfs:label>
    </owl:ObjectProperty>
    


    <!-- https://w3id.org/hacid/onto/top-level/isCollectionOf -->

    <owl:ObjectProperty rdf:about="https://w3id.org/hacid/onto/top-level/isCollectionOf">
        <rdfs:subPropertyOf rdf:resource="https://w3id.org/hacid/onto/top-level/associatedWith"/>
        <rdfs:domain rdf:resource="https://w3id.org/hacid/onto/top-level/Collection"/>
        <rdfs:range rdf:resource="https://w3id.org/hacid/onto/top-level/Entity"/>
        <rdfs:comment xml:lang="it">La relazione esistente tra una collezione ed una qualsiasi entità.</rdfs:comment>
        <rdfs:comment xml:lang="en">The relation holding between a collection and any possible entity.</rdfs:comment>
        <rdfs:isDefinedBy rdf:resource="https://w3id.org/hacid/onto/top-level"/>
        <rdfs:label xml:lang="en">is collection of</rdfs:label>
        <rdfs:label xml:lang="it">è collezione di</rdfs:label>
    </owl:ObjectProperty>
    


    <!-- https://w3id.org/hacid/onto/top-level/isConceptUsedIn -->

    <owl:ObjectProperty rdf:about="https://w3id.org/hacid/onto/top-level/isConceptUsedIn">
        <rdfs:subPropertyOf rdf:resource="https://w3id.org/hacid/onto/top-level/associatedWith"/>
        <owl:inverseOf rdf:resource="https://w3id.org/hacid/onto/top-level/usesConcept"/>
        <rdfs:domain rdf:resource="https://w3id.org/hacid/onto/top-level/Concept"/>
        <rdfs:range rdf:resource="https://w3id.org/hacid/onto/top-level/Description"/>
        <rdfs:comment xml:lang="en">A more generic relation holding between a Description and a Concept. In order to be used, a Concept must be previously definedIn another Description</rdfs:comment>
        <rdfs:isDefinedBy rdf:resource="https://w3id.org/hacid/onto/top-level"/>
        <rdfs:label xml:lang="en">is concept used in</rdfs:label>
        <rdfs:label xml:lang="it">è un concetto usato in</rdfs:label>
    </owl:ObjectProperty>
    


    <!-- https://w3id.org/hacid/onto/top-level/isCreatorOf -->

    <owl:ObjectProperty rdf:about="https://w3id.org/hacid/onto/top-level/isCreatorOf">
        <rdfs:subPropertyOf rdf:resource="https://w3id.org/hacid/onto/top-level/associatedWith"/>
        <rdfs:range rdf:resource="https://w3id.org/hacid/onto/top-level/Entity"/>
        <rdfs:comment xml:lang="it">La relazione per associare un agente creatore ad un'entità creata.</rdfs:comment>
        <rdfs:comment xml:lang="en">The relation for asserting that a certain agent is the creator of an entity.</rdfs:comment>
        <rdfs:isDefinedBy rdf:resource="https://w3id.org/hacid/onto/top-level"/>
        <rdfs:label xml:lang="en">is creator of</rdfs:label>
        <rdfs:label xml:lang="it">è creatore di</rdfs:label>
    </owl:ObjectProperty>
    


    <!-- https://w3id.org/hacid/onto/top-level/isDataSchemaOf -->

    <owl:ObjectProperty rdf:about="https://w3id.org/hacid/onto/top-level/isDataSchemaOf">
        <rdfs:subPropertyOf rdf:resource="https://w3id.org/hacid/onto/top-level/isDescriptionOf"/>
        <rdfs:domain rdf:resource="https://w3id.org/hacid/onto/top-level/DataSchema"/>
        <rdfs:range rdf:resource="https://w3id.org/hacid/onto/top-level/Media"/>
        <rdfs:comment xml:lang="it">La relazione esistente tra uno schema di dati e il supporto.</rdfs:comment>
        <rdfs:comment xml:lang="en">The relation existing between a data schema and the media.</rdfs:comment>
        <rdfs:isDefinedBy rdf:resource="https://w3id.org/hacid/onto/top-level"/>
        <rdfs:label xml:lang="en">is data schema of</rdfs:label>
        <rdfs:label xml:lang="it">è schema di dati di</rdfs:label>
    </owl:ObjectProperty>
    


    <!-- https://w3id.org/hacid/onto/top-level/isDefinedIn -->

    <owl:ObjectProperty rdf:about="https://w3id.org/hacid/onto/top-level/isDefinedIn">
        <rdfs:subPropertyOf rdf:resource="https://w3id.org/hacid/onto/top-level/isConceptUsedIn"/>
        <rdfs:domain rdf:resource="https://w3id.org/hacid/onto/top-level/Concept"/>
        <rdfs:range rdf:resource="https://w3id.org/hacid/onto/top-level/Description"/>
        <rdfs:comment xml:lang="en">A relation between a Description and a Concept, e.g. a Workflow for a governmental Organization defines the Role 'officer', or 'the Italian Traffic Law defines the role Vehicle'.</rdfs:comment>
        <rdfs:isDefinedBy rdf:resource="https://w3id.org/hacid/onto/top-level"/>
        <rdfs:label xml:lang="en">is defined in</rdfs:label>
        <rdfs:label xml:lang="it">è definito in</rdfs:label>
    </owl:ObjectProperty>
    


    <!-- https://w3id.org/hacid/onto/top-level/isDescribedBy -->

    <owl:ObjectProperty rdf:about="https://w3id.org/hacid/onto/top-level/isDescribedBy">
        <rdfs:subPropertyOf rdf:resource="https://w3id.org/hacid/onto/top-level/associatedWith"/>
        <rdfs:comment xml:lang="it">La relazione per associare un'entità alla sua descrizione.</rdfs:comment>
        <rdfs:comment xml:lang="en">The relation to associate an entity with its description.</rdfs:comment>
        <rdfs:isDefinedBy rdf:resource="https://w3id.org/hacid/onto/top-level"/>
        <rdfs:label xml:lang="en">is described by</rdfs:label>
        <rdfs:label xml:lang="it">è descritto da</rdfs:label>
    </owl:ObjectProperty>
    


    <!-- https://w3id.org/hacid/onto/top-level/isDescriptionOf -->

    <owl:ObjectProperty rdf:about="https://w3id.org/hacid/onto/top-level/isDescriptionOf">
        <rdfs:subPropertyOf rdf:resource="https://w3id.org/hacid/onto/top-level/associatedWith"/>
        <rdfs:domain rdf:resource="https://w3id.org/hacid/onto/top-level/Description"/>
        <rdfs:range rdf:resource="https://w3id.org/hacid/onto/top-level/Entity"/>
        <rdfs:comment xml:lang="it">La relazione esistente tra una descrizione e l'entità descritta.</rdfs:comment>
        <rdfs:comment xml:lang="en">The relationship between a description and the entity described.</rdfs:comment>
        <rdfs:isDefinedBy rdf:resource="https://w3id.org/hacid/onto/top-level"/>
        <rdfs:label xml:lang="en">is description of</rdfs:label>
        <rdfs:label xml:lang="it">è descrizione di</rdfs:label>
    </owl:ObjectProperty>
    


    <!-- https://w3id.org/hacid/onto/top-level/isEventualityOf -->

    <owl:ObjectProperty rdf:about="https://w3id.org/hacid/onto/top-level/isEventualityOf">
        <rdfs:subPropertyOf rdf:resource="https://w3id.org/hacid/onto/top-level/associatedWith"/>
        <rdfs:domain rdf:resource="https://w3id.org/hacid/onto/top-level/Situation"/>
        <rdfs:range rdf:resource="https://w3id.org/hacid/onto/top-level/Entity"/>
        <rdfs:comment xml:lang="it">Il rapporto esistente tra un'eventualità e qualsiasi entità possibile.</rdfs:comment>
        <rdfs:comment xml:lang="en">The relationship existing between an eventuality and any possible entity.</rdfs:comment>
        <rdfs:isDefinedBy rdf:resource="https://w3id.org/hacid/onto/top-level"/>
        <rdfs:label xml:lang="en">is eventuality of</rdfs:label>
        <rdfs:label xml:lang="it">è eventualità di</rdfs:label>
    </owl:ObjectProperty>
    


    <!-- https://w3id.org/hacid/onto/top-level/isExecutedIn -->

    <owl:ObjectProperty rdf:about="https://w3id.org/hacid/onto/top-level/isExecutedIn">
        <rdfs:subPropertyOf rdf:resource="https://w3id.org/hacid/onto/top-level/classifies"/>
        <rdfs:domain rdf:resource="https://w3id.org/hacid/onto/top-level/Task"/>
        <rdfs:range rdf:resource="https://w3id.org/hacid/onto/top-level/Action"/>
        <rdfs:comment xml:lang="en">A relation between an action and a task, e.g. 'putting some water in a pot and putting the pot on a fire until the water starts bubbling' executes the task 'boiling'.</rdfs:comment>
        <rdfs:isDefinedBy rdf:resource="https://w3id.org/hacid/onto/top-level"/>
        <rdfs:label xml:lang="en">is executed in</rdfs:label>
        <rdfs:label xml:lang="it">è eseguito mediante</rdfs:label>
    </owl:ObjectProperty>
    


    <!-- https://w3id.org/hacid/onto/top-level/isIdentifierSchemaOf -->

    <owl:ObjectProperty rdf:about="https://w3id.org/hacid/onto/top-level/isIdentifierSchemaOf">
        <rdfs:subPropertyOf rdf:resource="https://w3id.org/hacid/onto/top-level/isDescriptionOf"/>
        <rdfs:domain rdf:resource="https://w3id.org/hacid/onto/top-level/IdentifierSchema"/>
        <rdfs:comment xml:lang="it">La relazione che lega uno schema di identificazione ad un identificativo unico.</rdfs:comment>
        <rdfs:comment xml:lang="en">The relation between an identifier schema and a unique identifier.</rdfs:comment>
        <rdfs:isDefinedBy rdf:resource="https://w3id.org/hacid/onto/top-level"/>
        <rdfs:label xml:lang="en">is identifier schema of</rdfs:label>
        <rdfs:label xml:lang="it">è schema identificativo di</rdfs:label>
    </owl:ObjectProperty>
    


    <!-- https://w3id.org/hacid/onto/top-level/isInputRoleOf -->

    <owl:ObjectProperty rdf:about="https://w3id.org/hacid/onto/top-level/isInputRoleOf">
        <rdfs:subPropertyOf rdf:resource="https://w3id.org/hacid/onto/top-level/associatedWith"/>
        <rdfs:domain rdf:resource="https://w3id.org/hacid/onto/top-level/Role"/>
        <rdfs:range rdf:resource="https://w3id.org/hacid/onto/top-level/Task"/>
        <rdfs:comment xml:lang="en">Inverse property of hasInputRole.</rdfs:comment>
        <rdfs:isDefinedBy rdf:resource="https://w3id.org/hacid/onto/top-level"/>
        <rdfs:label xml:lang="en">is input role of</rdfs:label>
    </owl:ObjectProperty>
    


    <!-- https://w3id.org/hacid/onto/top-level/isInvolvedIn -->

    <owl:ObjectProperty rdf:about="https://w3id.org/hacid/onto/top-level/isInvolvedIn">
        <rdfs:subPropertyOf rdf:resource="https://w3id.org/hacid/onto/top-level/associatedWith"/>
        <rdfs:domain rdf:resource="https://w3id.org/hacid/onto/top-level/Entity"/>
        <rdfs:range rdf:resource="https://w3id.org/hacid/onto/top-level/Situation"/>
        <rdfs:comment xml:lang="it">La proprietà per associare un'entità ad una situazione.</rdfs:comment>
        <rdfs:comment xml:lang="en">The property for associating an entity with a situation.</rdfs:comment>
        <rdfs:isDefinedBy rdf:resource="https://w3id.org/hacid/onto/top-level"/>
        <rdfs:label xml:lang="en">is involved in</rdfs:label>
        <rdfs:label xml:lang="it">è coinvolto in</rdfs:label>
    </owl:ObjectProperty>
    


    <!-- https://w3id.org/hacid/onto/top-level/isIssuedBy -->

    <owl:ObjectProperty rdf:about="https://w3id.org/hacid/onto/top-level/isIssuedBy">
        <rdfs:subPropertyOf rdf:resource="https://w3id.org/hacid/onto/top-level/associatedWith"/>
        <owl:inverseOf rdf:resource="https://w3id.org/hacid/onto/top-level/issues"/>
        <rdfs:domain rdf:resource="https://w3id.org/hacid/onto/top-level/Entity"/>
        <rdfs:comment xml:lang="it">La relazione che consente di affermare che un'entità è creata da un determinato agente.</rdfs:comment>
        <rdfs:comment xml:lang="en">The relation that allows one to state that an entity is created by a given agent.</rdfs:comment>
        <rdfs:isDefinedBy rdf:resource="https://w3id.org/hacid/onto/top-level"/>
        <rdfs:label xml:lang="it">ha creatore</rdfs:label>
        <rdfs:label xml:lang="en">has creator</rdfs:label>
    </owl:ObjectProperty>
    


    <!-- https://w3id.org/hacid/onto/top-level/isLocationOf -->

    <owl:ObjectProperty rdf:about="https://w3id.org/hacid/onto/top-level/isLocationOf">
        <rdfs:subPropertyOf rdf:resource="https://w3id.org/hacid/onto/top-level/associatedWith"/>
        <rdfs:domain rdf:resource="https://w3id.org/hacid/onto/top-level/Location"/>
        <rdfs:range rdf:resource="https://w3id.org/hacid/onto/top-level/Entity"/>
        <rdfs:comment xml:lang="it">La proprietà che permette di dire che un determinato luogo è la posizione di un dato oggetto.</rdfs:comment>
        <rdfs:comment xml:lang="it">La relazione esistente tra un luogo ed un'entità di un qualsiasi tipo.</rdfs:comment>
        <rdfs:comment xml:lang="en">The property that allows to say that a certain place is the location of a given object.</rdfs:comment>
        <rdfs:comment xml:lang="en">The relation holding between a place and an entity of any possible type.</rdfs:comment>
        <rdfs:isDefinedBy rdf:resource="https://w3id.org/hacid/onto/top-level"/>
        <rdfs:label xml:lang="it">is location of</rdfs:label>
        <rdfs:label xml:lang="en">is place of</rdfs:label>
        <rdfs:label xml:lang="it">è luogo di</rdfs:label>
    </owl:ObjectProperty>
    


    <!-- https://w3id.org/hacid/onto/top-level/isMediaOf -->

    <owl:ObjectProperty rdf:about="https://w3id.org/hacid/onto/top-level/isMediaOf">
        <rdfs:subPropertyOf rdf:resource="https://w3id.org/hacid/onto/top-level/associatedWith"/>
        <rdfs:domain rdf:resource="https://w3id.org/hacid/onto/top-level/Media"/>
        <rdfs:range rdf:resource="https://w3id.org/hacid/onto/top-level/Entity"/>
        <rdfs:comment xml:lang="it">La relazione tra un'istanza di un'entità di classe Media e un'entità.</rdfs:comment>
        <rdfs:comment xml:lang="en">The relationship between an instance Media class entity and an entity.</rdfs:comment>
        <rdfs:isDefinedBy rdf:resource="https://w3id.org/hacid/onto/top-level"/>
        <rdfs:label xml:lang="en">is media of</rdfs:label>
        <rdfs:label xml:lang="it">è media di</rdfs:label>
    </owl:ObjectProperty>
    


    <!-- https://w3id.org/hacid/onto/top-level/isMemberOf -->

    <owl:ObjectProperty rdf:about="https://w3id.org/hacid/onto/top-level/isMemberOf">
        <rdfs:subPropertyOf rdf:resource="https://w3id.org/hacid/onto/top-level/associatedWith"/>
        <rdfs:domain rdf:resource="https://w3id.org/hacid/onto/top-level/Entity"/>
        <rdfs:range rdf:resource="https://w3id.org/hacid/onto/top-level/Collection"/>
        <rdfs:comment xml:lang="it">La relazione inversa di 'ha membro'. Come la sua inversa permette di stabilire relazione di memberhip tra un elemento ed la sua collezione.</rdfs:comment>
        <rdfs:comment xml:lang="en">The inverse relation of 'has member'. It allows to represent membership relations.</rdfs:comment>
        <rdfs:isDefinedBy rdf:resource="https://w3id.org/hacid/onto/top-level"/>
        <rdfs:label xml:lang="en">is member of</rdfs:label>
        <rdfs:label xml:lang="it">è membro di</rdfs:label>
    </owl:ObjectProperty>
    


    <!-- https://w3id.org/hacid/onto/top-level/isOutputRoleOf -->

    <owl:ObjectProperty rdf:about="https://w3id.org/hacid/onto/top-level/isOutputRoleOf">
        <rdfs:subPropertyOf rdf:resource="https://w3id.org/hacid/onto/top-level/associatedWith"/>
        <rdfs:domain rdf:resource="https://w3id.org/hacid/onto/top-level/Role"/>
        <rdfs:range rdf:resource="https://w3id.org/hacid/onto/top-level/Task"/>
        <rdfs:comment xml:lang="en">Inverse property of hasOutputRole.</rdfs:comment>
        <rdfs:isDefinedBy rdf:resource="https://w3id.org/hacid/onto/top-level"/>
        <rdfs:label xml:lang="en">is output role of</rdfs:label>
    </owl:ObjectProperty>
    


    <!-- https://w3id.org/hacid/onto/top-level/isParametrisedBy -->

    <owl:ObjectProperty rdf:about="https://w3id.org/hacid/onto/top-level/isParametrisedBy">
        <rdfs:subPropertyOf rdf:resource="https://w3id.org/hacid/onto/top-level/isClassifiedBy"/>
        <owl:inverseOf rdf:resource="https://w3id.org/hacid/onto/top-level/parametrises"/>
        <rdfs:domain rdf:resource="https://w3id.org/hacid/onto/top-level/Entity"/>
        <rdfs:range rdf:resource="https://w3id.org/hacid/onto/top-level/Parameter"/>
        <rdfs:comment xml:lang="it">La relazione che sussiste tra l'entità oggetto della parametrizzazione ed il parametro.</rdfs:comment>
        <rdfs:comment xml:lang="en">The relation holding between the entity being object of the parametrisation and a parameter.</rdfs:comment>
        <rdfs:isDefinedBy rdf:resource="https://w3id.org/hacid/onto/top-level"/>
        <rdfs:label xml:lang="en">is parametrised by</rdfs:label>
        <rdfs:label xml:lang="it">è parametrizzato da</rdfs:label>
    </owl:ObjectProperty>
    


    <!-- https://w3id.org/hacid/onto/top-level/isPartOf -->

    <owl:ObjectProperty rdf:about="https://w3id.org/hacid/onto/top-level/isPartOf">
        <rdfs:subPropertyOf rdf:resource="https://w3id.org/hacid/onto/top-level/associatedWith"/>
        <rdf:type rdf:resource="http://www.w3.org/2002/07/owl#TransitiveProperty"/>
        <rdf:type rdf:resource="http://www.w3.org/2002/07/owl#ReflexiveProperty"/>
        <rdfs:domain rdf:resource="https://w3id.org/hacid/onto/top-level/Entity"/>
        <rdfs:range rdf:resource="https://w3id.org/hacid/onto/top-level/Entity"/>
        <rdfs:comment xml:lang="it">L'inversa di 'ha parte' per rappresentare la relazione di parte dal punto di vista della parte. La proprietà è definita come riflessiva e transitiva.</rdfs:comment>
        <rdfs:comment xml:lang="en">The inverse of 'has part' for representing parthood from the perspective of the part. The property is defined as reflexive and transitive.</rdfs:comment>
        <rdfs:isDefinedBy rdf:resource="https://w3id.org/hacid/onto/top-level"/>
        <rdfs:label xml:lang="en">is part of</rdfs:label>
        <rdfs:label xml:lang="it">è parte di</rdfs:label>
    </owl:ObjectProperty>
    


    <!-- https://w3id.org/hacid/onto/top-level/isParticipantIn -->

    <owl:ObjectProperty rdf:about="https://w3id.org/hacid/onto/top-level/isParticipantIn">
        <rdfs:subPropertyOf rdf:resource="https://w3id.org/hacid/onto/top-level/associatedWith"/>
        <rdfs:domain rdf:resource="https://w3id.org/hacid/onto/top-level/Object"/>
        <rdfs:range rdf:resource="https://w3id.org/hacid/onto/top-level/Event"/>
        <rdfs:comment xml:lang="en">A relation between an object and a process, e.g. 'John took part in the discussion', 'a large mass of snow fell during the avalanche', or 'a cook, some sugar, flour, etc. are all present in the cooking of a cake'.</rdfs:comment>
        <rdfs:isDefinedBy rdf:resource="https://w3id.org/hacid/onto/top-level"/>
        <rdfs:label xml:lang="en">is participant in</rdfs:label>
        <rdfs:label xml:lang="it">è un partecipante a</rdfs:label>
    </owl:ObjectProperty>
    


    <!-- https://w3id.org/hacid/onto/top-level/isProperPartOf -->

    <owl:ObjectProperty rdf:about="https://w3id.org/hacid/onto/top-level/isProperPartOf">
        <rdfs:subPropertyOf rdf:resource="https://w3id.org/hacid/onto/top-level/isPartOf"/>
        <rdf:type rdf:resource="http://www.w3.org/2002/07/owl#AsymmetricProperty"/>
        <rdfs:domain rdf:resource="https://w3id.org/hacid/onto/top-level/Entity"/>
        <rdfs:range rdf:resource="https://w3id.org/hacid/onto/top-level/Entity"/>
        <rdfs:comment xml:lang="it">La proprietà per rappresentare la composizionalità tra un componente ed l'oggetto di cui fa parte.</rdfs:comment>
        <rdfs:comment xml:lang="en">The object property for representing the componency relation between a component and the object it is a component of.</rdfs:comment>
        <rdfs:isDefinedBy rdf:resource="https://w3id.org/hacid/onto/top-level"/>
        <rdfs:label xml:lang="en">is proper part of</rdfs:label>
        <rdfs:label xml:lang="it">è parte propria di</rdfs:label>
    </owl:ObjectProperty>
    


    <!-- https://w3id.org/hacid/onto/top-level/isRegionFor -->

    <owl:ObjectProperty rdf:about="https://w3id.org/hacid/onto/top-level/isRegionFor">
        <rdfs:subPropertyOf rdf:resource="https://w3id.org/hacid/onto/top-level/associatedWith"/>
        <rdfs:domain rdf:resource="https://w3id.org/hacid/onto/top-level/Region"/>
        <rdfs:range rdf:resource="https://w3id.org/hacid/onto/top-level/Entity"/>
        <rdfs:comment xml:lang="en">A relation between entities and regions, e.g. 'the color of my car is red'.</rdfs:comment>
        <rdfs:comment xml:lang="it">Una relazione tra entità e regioni, ad es. 'il colore della mia macchina è rosso'.</rdfs:comment>
        <rdfs:isDefinedBy rdf:resource="https://w3id.org/hacid/onto/top-level"/>
        <rdfs:label xml:lang="en">is region for</rdfs:label>
        <rdfs:label xml:lang="it">è una regione di</rdfs:label>
    </owl:ObjectProperty>
    


    <!-- https://w3id.org/hacid/onto/top-level/isRelatedToConcept -->

    <owl:ObjectProperty rdf:about="https://w3id.org/hacid/onto/top-level/isRelatedToConcept">
        <rdfs:subPropertyOf rdf:resource="https://w3id.org/hacid/onto/top-level/associatedWith"/>
        <rdfs:domain rdf:resource="https://w3id.org/hacid/onto/top-level/Concept"/>
        <rdfs:range rdf:resource="https://w3id.org/hacid/onto/top-level/Concept"/>
        <rdfs:comment xml:lang="en">Any relation between concepts, e.g. superordinated, conceptual parthood, having a parameter, having a task, superordination, etc.</rdfs:comment>
        <rdfs:isDefinedBy rdf:resource="https://w3id.org/hacid/onto/top-level"/>
        <rdfs:label xml:lang="en">is related to concept</rdfs:label>
        <rdfs:label xml:lang="it">è associato al concetto</rdfs:label>
    </owl:ObjectProperty>
    


    <!-- https://w3id.org/hacid/onto/top-level/isRoleDefinedIn -->

    <owl:ObjectProperty rdf:about="https://w3id.org/hacid/onto/top-level/isRoleDefinedIn">
        <rdfs:subPropertyOf rdf:resource="https://w3id.org/hacid/onto/top-level/isDefinedIn"/>
        <rdfs:domain rdf:resource="https://w3id.org/hacid/onto/top-level/Role"/>
        <rdfs:range rdf:resource="https://w3id.org/hacid/onto/top-level/Description"/>
        <rdfs:comment xml:lang="en">A relation between a description and a role, e.g. the role 'Ingredient' is defined in the recipe for a cake.</rdfs:comment>
        <rdfs:isDefinedBy rdf:resource="https://w3id.org/hacid/onto/top-level"/>
        <rdfs:label xml:lang="en">is role defined in</rdfs:label>
        <rdfs:label xml:lang="it">è un ruolo definito in</rdfs:label>
    </owl:ObjectProperty>
    


    <!-- https://w3id.org/hacid/onto/top-level/isRoleInvolvedIn -->

    <owl:ObjectProperty rdf:about="https://w3id.org/hacid/onto/top-level/isRoleInvolvedIn">
        <rdfs:subPropertyOf rdf:resource="https://w3id.org/hacid/onto/top-level/hasEventuality"/>
        <rdfs:domain rdf:resource="https://w3id.org/hacid/onto/top-level/Role"/>
        <rdfs:comment xml:lang="it">La relazione che collega un ruolo alla situazione ruolo-agente in cui esso partecipa.</rdfs:comment>
        <rdfs:comment xml:lang="en">The relationship that links a role to the agent-role situation it is involved in.</rdfs:comment>
        <rdfs:isDefinedBy rdf:resource="https://w3id.org/hacid/onto/top-level"/>
        <rdfs:label xml:lang="en">is role involved in</rdfs:label>
        <rdfs:label xml:lang="it">è il ruolo coinvolto in</rdfs:label>
    </owl:ObjectProperty>
    


    <!-- https://w3id.org/hacid/onto/top-level/isRoleOf -->

    <owl:ObjectProperty rdf:about="https://w3id.org/hacid/onto/top-level/isRoleOf">
        <rdfs:subPropertyOf rdf:resource="https://w3id.org/hacid/onto/top-level/classifies"/>
        <rdfs:domain rdf:resource="https://w3id.org/hacid/onto/top-level/Role"/>
        <rdfs:range rdf:resource="https://w3id.org/hacid/onto/top-level/Entity"/>
        <rdfs:comment xml:lang="it">La relazione che consente di utilizzare un ruolo per classificare una determinata entità.</rdfs:comment>
        <rdfs:comment xml:lang="en">The relation that allows you to use a role for classifying a certain entity.</rdfs:comment>
        <rdfs:isDefinedBy rdf:resource="https://w3id.org/hacid/onto/top-level"/>
        <rdfs:label xml:lang="en">is role of</rdfs:label>
        <rdfs:label xml:lang="it">è ruolo di</rdfs:label>
    </owl:ObjectProperty>
    


    <!-- https://w3id.org/hacid/onto/top-level/isSatisfiedBy -->

    <owl:ObjectProperty rdf:about="https://w3id.org/hacid/onto/top-level/isSatisfiedBy">
        <rdfs:subPropertyOf rdf:resource="https://w3id.org/hacid/onto/top-level/associatedWith"/>
        <owl:inverseOf rdf:resource="https://w3id.org/hacid/onto/top-level/satisfies"/>
        <rdfs:domain rdf:resource="https://w3id.org/hacid/onto/top-level/Description"/>
        <rdfs:range rdf:resource="https://w3id.org/hacid/onto/top-level/Situation"/>
        <rdfs:comment xml:lang="en">A relation between a Situation and a Description, e.g. the execution of a Plan satisfies that plan.</rdfs:comment>
        <rdfs:isDefinedBy rdf:resource="https://w3id.org/hacid/onto/top-level"/>
        <rdfs:label xml:lang="it">La relazione tra una descrizione ed un'eventualità.</rdfs:label>
        <rdfs:label xml:lang="en">The relation between a description and an eventuality.</rdfs:label>
        <rdfs:label xml:lang="en">is satisfied by</rdfs:label>
        <rdfs:label xml:lang="it">è soddisfatto da</rdfs:label>
    </owl:ObjectProperty>
    


    <!-- https://w3id.org/hacid/onto/top-level/isSchemaAttributeOf -->

    <owl:ObjectProperty rdf:about="https://w3id.org/hacid/onto/top-level/isSchemaAttributeOf">
        <rdfs:subPropertyOf rdf:resource="https://w3id.org/hacid/onto/top-level/isCharacteristicOf"/>
        <rdfs:domain rdf:resource="https://w3id.org/hacid/onto/top-level/SchemaAttribute"/>
        <rdfs:range rdf:resource="https://w3id.org/hacid/onto/top-level/DataSchema"/>
        <rdfs:comment xml:lang="it">La proprietà che permette di collegare un attributo allo schema di dati.</rdfs:comment>
        <rdfs:comment xml:lang="en">The property that allows you to link an attribute to the data schema.</rdfs:comment>
        <rdfs:isDefinedBy rdf:resource="https://w3id.org/hacid/onto/top-level"/>
        <rdfs:label xml:lang="en">is data schema attribute of</rdfs:label>
        <rdfs:label xml:lang="it">è attributo di schema di dati di</rdfs:label>
    </owl:ObjectProperty>
    


    <!-- https://w3id.org/hacid/onto/top-level/isSettingFor -->

    <owl:ObjectProperty rdf:about="https://w3id.org/hacid/onto/top-level/isSettingFor">
        <rdfs:subPropertyOf rdf:resource="https://w3id.org/hacid/onto/top-level/associatedWith"/>
        <rdfs:domain rdf:resource="https://w3id.org/hacid/onto/top-level/Situation"/>
        <rdfs:range rdf:resource="https://w3id.org/hacid/onto/top-level/Entity"/>
        <rdfs:comment xml:lang="en">A relation between situations and entities, e.g. 'this morning I've prepared my coffee with a new fantastic Arabica', i.e.: the preparation of my coffee this morning is the setting for (an amount of) a new fantastic Arabica.</rdfs:comment>
        <rdfs:isDefinedBy rdf:resource="https://w3id.org/hacid/onto/top-level"/>
        <rdfs:label xml:lang="it">include</rdfs:label>
        <rdfs:label xml:lang="en">is setting for</rdfs:label>
    </owl:ObjectProperty>
    


    <!-- https://w3id.org/hacid/onto/top-level/isSouceOf -->

    <owl:ObjectProperty rdf:about="https://w3id.org/hacid/onto/top-level/isSouceOf">
        <rdfs:subPropertyOf rdf:resource="https://w3id.org/hacid/onto/top-level/associatedWith"/>
        <rdfs:domain rdf:resource="https://w3id.org/hacid/onto/top-level/Entity"/>
        <rdfs:range rdf:resource="https://w3id.org/hacid/onto/top-level/Entity"/>
        <rdfs:comment xml:lang="en">Inverse object property of hasSource.</rdfs:comment>
        <rdfs:comment xml:lang="it">Object property inversa di hasSource.</rdfs:comment>
        <rdfs:isDefinedBy rdf:resource="https://w3id.org/hacid/onto/top-level"/>
        <rdfs:label xml:lang="en">is source of</rdfs:label>
        <rdfs:label xml:lang="it">è sorgente di</rdfs:label>
    </owl:ObjectProperty>
    


    <!-- https://w3id.org/hacid/onto/top-level/isSpecialisedBy -->

    <owl:ObjectProperty rdf:about="https://w3id.org/hacid/onto/top-level/isSpecialisedBy">
        <rdfs:subPropertyOf rdf:resource="https://w3id.org/hacid/onto/top-level/associatedWith"/>
        <owl:inverseOf rdf:resource="https://w3id.org/hacid/onto/top-level/specialises"/>
        <rdf:type rdf:resource="http://www.w3.org/2002/07/owl#TransitiveProperty"/>
        <rdfs:domain rdf:resource="https://w3id.org/hacid/onto/top-level/Entity"/>
        <rdfs:range rdf:resource="https://w3id.org/hacid/onto/top-level/Entity"/>
        <rdfs:comment xml:lang="it">La relazione inverse di 'specializza'.</rdfs:comment>
        <rdfs:comment xml:lang="en">The inverse releation of 'specialises'</rdfs:comment>
        <rdfs:isDefinedBy rdf:resource="https://w3id.org/hacid/onto/top-level"/>
        <rdfs:label xml:lang="en">is specialised by</rdfs:label>
        <rdfs:label xml:lang="it">è specializzato da</rdfs:label>
    </owl:ObjectProperty>
    


    <!-- https://w3id.org/hacid/onto/top-level/isSystemOf -->

    <owl:ObjectProperty rdf:about="https://w3id.org/hacid/onto/top-level/isSystemOf">
        <rdfs:subPropertyOf rdf:resource="https://w3id.org/hacid/onto/top-level/associatedWith"/>
        <rdfs:domain rdf:resource="https://w3id.org/hacid/onto/top-level/System"/>
        <rdfs:range rdf:resource="https://w3id.org/hacid/onto/top-level/Entity"/>
        <rdfs:comment xml:lang="it">La relazione che sussiste tra un sistema ed una qualsiasi entità.</rdfs:comment>
        <rdfs:comment xml:lang="en">The relationship holding between a system and any entity.</rdfs:comment>
        <rdfs:isDefinedBy rdf:resource="https://w3id.org/hacid/onto/top-level"/>
        <rdfs:label xml:lang="en">is system of</rdfs:label>
        <rdfs:label xml:lang="it">è sistema di</rdfs:label>
    </owl:ObjectProperty>
    


    <!-- https://w3id.org/hacid/onto/top-level/isTaskDefinedIn -->

    <owl:ObjectProperty rdf:about="https://w3id.org/hacid/onto/top-level/isTaskDefinedIn">
        <rdfs:subPropertyOf rdf:resource="https://w3id.org/hacid/onto/top-level/isDefinedIn"/>
        <rdfs:domain rdf:resource="https://w3id.org/hacid/onto/top-level/Task"/>
        <rdfs:range rdf:resource="https://w3id.org/hacid/onto/top-level/Description"/>
        <rdfs:comment xml:lang="en">A relation between a description and a task, e.g. the task 'boil' is defined in a recipe for a cake.</rdfs:comment>
        <rdfs:isDefinedBy rdf:resource="https://w3id.org/hacid/onto/top-level"/>
        <rdfs:label xml:lang="en">is task defined in</rdfs:label>
        <rdfs:label xml:lang="it">è un task definito in</rdfs:label>
    </owl:ObjectProperty>
    


    <!-- https://w3id.org/hacid/onto/top-level/isTaskOf -->

    <owl:ObjectProperty rdf:about="https://w3id.org/hacid/onto/top-level/isTaskOf">
        <rdfs:subPropertyOf rdf:resource="https://w3id.org/hacid/onto/top-level/isRelatedToConcept"/>
        <rdfs:domain rdf:resource="https://w3id.org/hacid/onto/top-level/Task"/>
        <rdfs:range rdf:resource="https://w3id.org/hacid/onto/top-level/Role"/>
        <rdfs:comment xml:lang="en">A relation between roles and tasks, e.g. 'students have the duty of giving exams' (i.e. the Role 'student' hasTask the Task 'giving exams').</rdfs:comment>
        <rdfs:isDefinedBy rdf:resource="https://w3id.org/hacid/onto/top-level"/>
        <rdfs:label xml:lang="en">is task of</rdfs:label>
        <rdfs:label xml:lang="it">è un obiettivo per</rdfs:label>
    </owl:ObjectProperty>
    


    <!-- https://w3id.org/hacid/onto/top-level/isTimeIntervalOf -->

    <owl:ObjectProperty rdf:about="https://w3id.org/hacid/onto/top-level/isTimeIntervalOf">
        <rdfs:subPropertyOf rdf:resource="https://w3id.org/hacid/onto/top-level/isRegionFor"/>
        <rdfs:domain rdf:resource="https://w3id.org/hacid/onto/top-level/TimeInterval"/>
        <rdfs:range rdf:resource="https://w3id.org/hacid/onto/top-level/Event"/>
        <rdfs:comment xml:lang="it">La relazione generica tra eventi e intervalli di tempo.</rdfs:comment>
        <rdfs:comment xml:lang="en">The generic relation between time intervals and events.</rdfs:comment>
        <rdfs:isDefinedBy rdf:resource="https://w3id.org/hacid/onto/top-level"/>
        <rdfs:label xml:lang="it">intervallo temporale di</rdfs:label>
        <rdfs:label xml:lang="en">is time interval of</rdfs:label>
    </owl:ObjectProperty>
    


    <!-- https://w3id.org/hacid/onto/top-level/isTimeOf -->

    <owl:ObjectProperty rdf:about="https://w3id.org/hacid/onto/top-level/isTimeOf">
        <rdfs:subPropertyOf rdf:resource="https://w3id.org/hacid/onto/top-level/associatedWith"/>
        <rdfs:domain rdf:resource="https://w3id.org/hacid/onto/top-level/TemporalEntity"/>
        <rdfs:range rdf:resource="https://w3id.org/hacid/onto/top-level/Entity"/>
        <rdfs:comment xml:lang="it">La relazione esistente tra un'entità temporale ed una qualsiasi altra entità.</rdfs:comment>
        <rdfs:comment xml:lang="en">The relationship existing between a time entity and any other entity.</rdfs:comment>
        <rdfs:isDefinedBy rdf:resource="https://w3id.org/hacid/onto/top-level"/>
        <rdfs:label xml:lang="en">is time of</rdfs:label>
        <rdfs:label xml:lang="it">è tempo di</rdfs:label>
    </owl:ObjectProperty>
    


    <!-- https://w3id.org/hacid/onto/top-level/isUniqueIdentifierOf -->

    <owl:ObjectProperty rdf:about="https://w3id.org/hacid/onto/top-level/isUniqueIdentifierOf">
        <rdfs:subPropertyOf rdf:resource="https://w3id.org/hacid/onto/top-level/isCharacteristicOf"/>
        <rdfs:comment xml:lang="en">La relazione che sussiste tra un identificatore univoco e l'entità che identifica.</rdfs:comment>
        <rdfs:comment xml:lang="en">The relation holding between a unique identifier and the entity it identifies.</rdfs:comment>
        <rdfs:isDefinedBy rdf:resource="https://w3id.org/hacid/onto/top-level"/>
        <rdfs:label xml:lang="en">is unique identifier of</rdfs:label>
        <rdfs:label xml:lang="it">è identificativo univoco di</rdfs:label>
    </owl:ObjectProperty>
    


    <!-- https://w3id.org/hacid/onto/top-level/isUnitOfMeasureOf -->

    <owl:ObjectProperty rdf:about="https://w3id.org/hacid/onto/top-level/isUnitOfMeasureOf">
        <rdfs:subPropertyOf rdf:resource="https://w3id.org/hacid/onto/top-level/isCharacteristicOf"/>
        <rdfs:domain rdf:resource="https://w3id.org/hacid/onto/top-level/UnitOfMeasure"/>
        <rdfs:range rdf:resource="https://w3id.org/hacid/onto/top-level/Entity"/>
        <rdfs:comment xml:lang="en">Property that links a unit of measure to the object or measured value.</rdfs:comment>
        <rdfs:comment xml:lang="it">Proprietà che collega un'unità di misura all'oggetto o al valore misurato.</rdfs:comment>
        <rdfs:isDefinedBy rdf:resource="https://w3id.org/hacid/onto/top-level"/>
        <rdfs:label xml:lang="en">is unit of measure of</rdfs:label>
        <rdfs:label xml:lang="it">è unità di misura di</rdfs:label>
    </owl:ObjectProperty>
    


    <!-- https://w3id.org/hacid/onto/top-level/isValueOf -->

    <owl:ObjectProperty rdf:about="https://w3id.org/hacid/onto/top-level/isValueOf">
        <rdfs:subPropertyOf rdf:resource="https://w3id.org/hacid/onto/top-level/isCharacteristicOf"/>
        <rdfs:domain rdf:resource="https://w3id.org/hacid/onto/top-level/Value"/>
        <rdfs:range rdf:resource="https://w3id.org/hacid/onto/top-level/Entity"/>
        <rdfs:comment xml:lang="it">La relazione esistente tra un valore ed un'entità a cui tale valore è associato.</rdfs:comment>
        <rdfs:comment xml:lang="en">The relationship between a value and an entity to which that value is associated.</rdfs:comment>
        <rdfs:isDefinedBy rdf:resource="https://w3id.org/hacid/onto/top-level"/>
        <rdfs:label xml:lang="en">is value of</rdfs:label>
        <rdfs:label xml:lang="it">è valore di</rdfs:label>
    </owl:ObjectProperty>
    


    <!-- https://w3id.org/hacid/onto/top-level/issues -->

    <owl:ObjectProperty rdf:about="https://w3id.org/hacid/onto/top-level/issues">
        <rdfs:subPropertyOf rdf:resource="https://w3id.org/hacid/onto/top-level/associatedWith"/>
        <rdfs:range rdf:resource="https://w3id.org/hacid/onto/top-level/Entity"/>
        <rdfs:comment xml:lang="it">La relazione che consente di affermare che un determinato agente è il creatore di una certa entità.</rdfs:comment>
        <rdfs:comment xml:lang="en">The property that allows us to state that a certain agent is the creator of a certain entity.</rdfs:comment>
        <rdfs:isDefinedBy rdf:resource="https://w3id.org/hacid/onto/top-level"/>
        <rdfs:label xml:lang="en">is creator of</rdfs:label>
        <rdfs:label xml:lang="it">è creatore di</rdfs:label>
    </owl:ObjectProperty>
    


    <!-- https://w3id.org/hacid/onto/top-level/parametrises -->

    <owl:ObjectProperty rdf:about="https://w3id.org/hacid/onto/top-level/parametrises">
        <rdfs:subPropertyOf rdf:resource="https://w3id.org/hacid/onto/top-level/classifies"/>
        <rdfs:domain rdf:resource="https://w3id.org/hacid/onto/top-level/Parameter"/>
        <rdfs:range rdf:resource="https://w3id.org/hacid/onto/top-level/Entity"/>
        <rdfs:comment xml:lang="it">La relazione che sussiste tra un parametro e l'entità oggetto della parametrizzazione.</rdfs:comment>
        <rdfs:comment xml:lang="en">The relation holding between a parameter and the entity being object of the parametrisation.</rdfs:comment>
        <rdfs:isDefinedBy rdf:resource="https://w3id.org/hacid/onto/top-level"/>
        <rdfs:label xml:lang="en">parametrises</rdfs:label>
        <rdfs:label xml:lang="it">parametrizza</rdfs:label>
    </owl:ObjectProperty>
    


    <!-- https://w3id.org/hacid/onto/top-level/precedes -->

    <owl:ObjectProperty rdf:about="https://w3id.org/hacid/onto/top-level/precedes">
        <rdfs:subPropertyOf rdf:resource="https://w3id.org/hacid/onto/top-level/associatedWith"/>
        <rdf:type rdf:resource="http://www.w3.org/2002/07/owl#TransitiveProperty"/>
        <rdfs:domain rdf:resource="https://w3id.org/hacid/onto/top-level/Entity"/>
        <rdfs:range rdf:resource="https://w3id.org/hacid/onto/top-level/Entity"/>
        <rdfs:comment xml:lang="en">A relation between entities, expressing a 'sequence' schema.</rdfs:comment>
        <rdfs:comment xml:lang="it">Una relazione tra entità, che esprime uno schema di 'sequenza'.</rdfs:comment>
        <rdfs:isDefinedBy rdf:resource="https://w3id.org/hacid/onto/top-level"/>
        <rdfs:label xml:lang="it">precede</rdfs:label>
        <rdfs:label xml:lang="en">precedes</rdfs:label>
    </owl:ObjectProperty>
    


    <!-- https://w3id.org/hacid/onto/top-level/satisfies -->

    <owl:ObjectProperty rdf:about="https://w3id.org/hacid/onto/top-level/satisfies">
        <rdfs:subPropertyOf rdf:resource="https://w3id.org/hacid/onto/top-level/associatedWith"/>
        <rdfs:domain rdf:resource="https://w3id.org/hacid/onto/top-level/Situation"/>
        <rdfs:range rdf:resource="https://w3id.org/hacid/onto/top-level/Description"/>
        <rdfs:comment xml:lang="it">La proprietà usata per asserire che un'eventualità soddisfa una certa descrizione.</rdfs:comment>
        <rdfs:comment xml:lang="en">The property for asserting that an eventuality satisfies a description.</rdfs:comment>
        <rdfs:isDefinedBy rdf:resource="https://w3id.org/hacid/onto/top-level"/>
        <rdfs:label xml:lang="en">satisfies</rdfs:label>
        <rdfs:label xml:lang="it">soddisfa</rdfs:label>
    </owl:ObjectProperty>
    


    <!-- https://w3id.org/hacid/onto/top-level/specialises -->

    <owl:ObjectProperty rdf:about="https://w3id.org/hacid/onto/top-level/specialises">
        <rdfs:subPropertyOf rdf:resource="https://w3id.org/hacid/onto/top-level/associatedWith"/>
        <rdf:type rdf:resource="http://www.w3.org/2002/07/owl#TransitiveProperty"/>
        <rdfs:domain rdf:resource="https://w3id.org/hacid/onto/top-level/Entity"/>
        <rdfs:range rdf:resource="https://w3id.org/hacid/onto/top-level/Entity"/>
        <rdfs:comment xml:lang="it">La proprietà per esprimere relazioni di specializzazione.</rdfs:comment>
        <rdfs:comment xml:lang="en">The property for expressing specialisation relations.</rdfs:comment>
        <rdfs:isDefinedBy rdf:resource="https://w3id.org/hacid/onto/top-level"/>
        <rdfs:label xml:lang="en">specialises</rdfs:label>
        <rdfs:label xml:lang="it">specializza</rdfs:label>
    </owl:ObjectProperty>
    


    <!-- https://w3id.org/hacid/onto/top-level/usesConcept -->

    <owl:ObjectProperty rdf:about="https://w3id.org/hacid/onto/top-level/usesConcept">
        <rdfs:subPropertyOf rdf:resource="https://w3id.org/hacid/onto/top-level/associatedWith"/>
        <rdfs:domain rdf:resource="https://w3id.org/hacid/onto/top-level/Description"/>
        <rdfs:range rdf:resource="https://w3id.org/hacid/onto/top-level/Concept"/>
        <rdfs:comment xml:lang="en">A generic relation holding between a Description and a Concept. In order to be used, a Concept must be previously definedIn another Description. This last condition cannot be encoded for object properties in OWL.</rdfs:comment>
        <rdfs:isDefinedBy rdf:resource="https://w3id.org/hacid/onto/top-level"/>
        <rdfs:label xml:lang="it">usa il concetto</rdfs:label>
        <rdfs:label xml:lang="en">uses concept</rdfs:label>
    </owl:ObjectProperty>
    


    <!-- 
    ///////////////////////////////////////////////////////////////////////////////////////
    //
    // Data properties
    //
    ///////////////////////////////////////////////////////////////////////////////////////
     -->

    


    <!-- https://w3id.org/hacid/onto/top-level/acronym -->

    <owl:DatatypeProperty rdf:about="https://w3id.org/hacid/onto/top-level/acronym">
        <rdfs:domain rdf:resource="https://w3id.org/hacid/onto/top-level/Entity"/>
        <rdfs:range rdf:resource="http://www.w3.org/2000/01/rdf-schema#Literal"/>
        <rdfs:comment xml:lang="en">A value for the acronym that is used for referring to an entity.</rdfs:comment>
        <rdfs:comment xml:lang="it">Un valore per l'acronimo utilizzato per fare riferimento a un'entità.</rdfs:comment>
        <rdfs:isDefinedBy rdf:resource="https://w3id.org/hacid/onto/top-level"/>
        <rdfs:label xml:lang="it">acronimo</rdfs:label>
        <rdfs:label xml:lang="en">acronym</rdfs:label>
    </owl:DatatypeProperty>
    


    <!-- https://w3id.org/hacid/onto/top-level/endTime -->

    <owl:DatatypeProperty rdf:about="https://w3id.org/hacid/onto/top-level/endTime">
        <rdfs:subPropertyOf rdf:resource="https://w3id.org/hacid/onto/top-level/time"/>
        <rdfs:domain rdf:resource="https://w3id.org/hacid/onto/top-level/TimeInterval"/>
        <rdfs:range>
            <rdfs:Datatype>
                <owl:unionOf rdf:parseType="Collection">
                    <rdf:Description rdf:about="http://www.w3.org/2001/XMLSchema#date"/>
                    <rdf:Description rdf:about="http://www.w3.org/2001/XMLSchema#dateTime"/>
                    <rdf:Description rdf:about="http://www.w3.org/2001/XMLSchema#time"/>
                </owl:unionOf>
            </rdfs:Datatype>
        </rdfs:range>
        <rdfs:isDefinedBy rdf:resource="https://w3id.org/hacid/onto/top-level"/>
        <rdfs:label xml:lang="en">end time</rdfs:label>
        <rdfs:label xml:lang="it">tempo di fine</rdfs:label>
    </owl:DatatypeProperty>
    


    <!-- https://w3id.org/hacid/onto/top-level/identifier -->

    <owl:DatatypeProperty rdf:about="https://w3id.org/hacid/onto/top-level/identifier">
        <rdfs:comment xml:lang="it">Il valore letterale di un identificativo, ex. il codice WMO '6100218'.</rdfs:comment>
        <rdfs:comment xml:lang="en">The literal value of an identifier, e.g. the WMO code '6100218'.</rdfs:comment>
        <rdfs:isDefinedBy rdf:resource="https://w3id.org/hacid/onto/top-level"/>
        <rdfs:label xml:lang="it">identificativo</rdfs:label>
        <rdfs:label xml:lang="en">identifier</rdfs:label>
    </owl:DatatypeProperty>
    


    <!-- https://w3id.org/hacid/onto/top-level/mediaType -->

    <owl:DatatypeProperty rdf:about="https://w3id.org/hacid/onto/top-level/mediaType">
        <rdfs:domain rdf:resource="https://w3id.org/hacid/onto/top-level/Media"/>
        <rdfs:range rdf:resource="http://www.w3.org/2000/01/rdf-schema#Literal"/>
        <rdfs:comment xml:lang="en">A value for the media type, e.g. text/csv, rdf/xml, etc.</rdfs:comment>
        <rdfs:comment xml:lang="it">Un valore per il tipo di supporto, ad es. text/csv, rdf/xml, ecc.</rdfs:comment>
        <rdfs:isDefinedBy rdf:resource="https://w3id.org/hacid/onto/top-level"/>
        <rdfs:label xml:lang="en">media type</rdfs:label>
        <rdfs:label xml:lang="it">tipo di supporto</rdfs:label>
    </owl:DatatypeProperty>
    


    <!-- https://w3id.org/hacid/onto/top-level/name -->

    <owl:DatatypeProperty rdf:about="https://w3id.org/hacid/onto/top-level/name">
        <rdfs:domain rdf:resource="https://w3id.org/hacid/onto/top-level/Entity"/>
        <rdfs:range rdf:resource="http://www.w3.org/2000/01/rdf-schema#Literal"/>
        <rdfs:comment xml:lang="it">Il letterale che rappresenta il nome di un'entità.</rdfs:comment>
        <rdfs:comment xml:lang="en">The literal representing the name of an entity.</rdfs:comment>
        <rdfs:isDefinedBy rdf:resource="https://w3id.org/hacid/onto/top-level"/>
        <rdfs:label xml:lang="en">name</rdfs:label>
        <rdfs:label xml:lang="it">nome</rdfs:label>
    </owl:DatatypeProperty>
    


    <!-- https://w3id.org/hacid/onto/top-level/startTime -->

    <owl:DatatypeProperty rdf:about="https://w3id.org/hacid/onto/top-level/startTime">
        <rdfs:subPropertyOf rdf:resource="https://w3id.org/hacid/onto/top-level/time"/>
        <rdfs:domain rdf:resource="https://w3id.org/hacid/onto/top-level/TimeInterval"/>
        <rdfs:range>
            <rdfs:Datatype>
                <owl:unionOf rdf:parseType="Collection">
                    <rdf:Description rdf:about="http://www.w3.org/2001/XMLSchema#date"/>
                    <rdf:Description rdf:about="http://www.w3.org/2001/XMLSchema#dateTime"/>
                    <rdf:Description rdf:about="http://www.w3.org/2001/XMLSchema#time"/>
                </owl:unionOf>
            </rdfs:Datatype>
        </rdfs:range>
        <rdfs:isDefinedBy rdf:resource="https://w3id.org/hacid/onto/top-level"/>
        <rdfs:label xml:lang="en">start time</rdfs:label>
        <rdfs:label xml:lang="it">tempo di inizio</rdfs:label>
    </owl:DatatypeProperty>
    


    <!-- https://w3id.org/hacid/onto/top-level/symbol -->

    <owl:DatatypeProperty rdf:about="https://w3id.org/hacid/onto/top-level/symbol">
        <rdfs:domain rdf:resource="https://w3id.org/hacid/onto/top-level/Entity"/>
        <rdfs:range rdf:resource="http://www.w3.org/1999/02/22-rdf-syntax-ns#PlainLiteral"/>
        <rdfs:comment xml:lang="en">Property used to specify a symbol. For instance the symbol of a unit of measure</rdfs:comment>
        <rdfs:comment xml:lang="it">Proprietà  utilizzata per specificare un simbolo. Ad esempio il simbolo dell'unità di misura</rdfs:comment>
        <rdfs:isDefinedBy rdf:resource="https://w3id.org/hacid/onto/top-level"/>
        <rdfs:label xml:lang="it">simbolo</rdfs:label>
        <rdfs:label xml:lang="en">symbol</rdfs:label>
        <owl:versionInfo xml:lang="it">stabile</owl:versionInfo>
        <owl:versionInfo xml:lang="en">stable</owl:versionInfo>
    </owl:DatatypeProperty>
    


    <!-- https://w3id.org/hacid/onto/top-level/time -->

    <owl:DatatypeProperty rdf:about="https://w3id.org/hacid/onto/top-level/time">
        <rdfs:domain rdf:resource="https://w3id.org/hacid/onto/top-level/Entity"/>
        <rdfs:range rdf:resource="http://www.w3.org/2000/01/rdf-schema#Literal"/>
        <rdfs:comment xml:lang="it">La proprietà per associare la rappresentazione letterale del tempo a un'entità.</rdfs:comment>
        <rdfs:comment xml:lang="en">The property for associating the literal representation of time to an entity.</rdfs:comment>
        <rdfs:isDefinedBy rdf:resource="https://w3id.org/hacid/onto/top-level"/>
        <rdfs:label xml:lang="it">tempo</rdfs:label>
        <rdfs:label xml:lang="en">time</rdfs:label>
    </owl:DatatypeProperty>
    


    <!-- https://w3id.org/hacid/onto/top-level/value -->

    <owl:DatatypeProperty rdf:about="https://w3id.org/hacid/onto/top-level/value">
        <rdfs:domain rdf:resource="https://w3id.org/hacid/onto/top-level/Entity"/>
        <rdfs:range rdf:resource="http://www.w3.org/2000/01/rdf-schema#Literal"/>
        <rdfs:comment xml:lang="it">La rappresentazione letterale di un valore.</rdfs:comment>
        <rdfs:comment xml:lang="en">The literal representation of a value.</rdfs:comment>
        <rdfs:isDefinedBy rdf:resource="https://w3id.org/hacid/onto/top-level"/>
        <rdfs:label xml:lang="it">valore</rdfs:label>
        <rdfs:label xml:lang="en">value</rdfs:label>
    </owl:DatatypeProperty>
    


    <!-- https://w3id.org/hacid/onto/top-level/year -->

    <owl:DatatypeProperty rdf:about="https://w3id.org/hacid/onto/top-level/year">
        <rdfs:subPropertyOf rdf:resource="https://w3id.org/hacid/onto/top-level/time"/>
        <rdfs:domain rdf:resource="https://w3id.org/hacid/onto/top-level/TemporalEntity"/>
        <rdfs:range rdf:resource="http://www.w3.org/2001/XMLSchema#gYear"/>
        <rdfs:comment xml:lang="it">La proprietà per collegare il valore in gYear ad un istanza della classe TemporalEntity.</rdfs:comment>
        <rdfs:comment xml:lang="en">The property that relates a valued expressed a gYear to an instance of the class TemporalEntity.</rdfs:comment>
        <rdfs:isDefinedBy rdf:resource="https://w3id.org/hacid/onto/top-level"/>
        <rdfs:label xml:lang="it">anno</rdfs:label>
        <rdfs:label xml:lang="en">year</rdfs:label>
    </owl:DatatypeProperty>
    


    <!-- 
    ///////////////////////////////////////////////////////////////////////////////////////
    //
    // Classes
    //
    ///////////////////////////////////////////////////////////////////////////////////////
     -->

    


    <!-- http://www.w3.org/2000/01/rdf-schema#Property -->

    <owl:Class rdf:about="http://www.w3.org/2000/01/rdf-schema#Property"/>
    


    <!-- https://w3id.org/hacid/onto/top-level/Action -->

    <owl:Class rdf:about="https://w3id.org/hacid/onto/top-level/Action">
        <rdfs:subClassOf rdf:resource="https://w3id.org/hacid/onto/top-level/Event"/>
        <rdfs:comment xml:lang="en">An Event with at least one Agent that isParticipantIn it, and that executes a Task that typically isDefinedIn a Plan, Workflow, Project, etc.</rdfs:comment>
        <rdfs:isDefinedBy rdf:resource="https://w3id.org/hacid/onto/top-level"/>
        <rdfs:label xml:lang="en">Action</rdfs:label>
        <rdfs:label xml:lang="it">Azione</rdfs:label>
    </owl:Class>
    


    <!-- https://w3id.org/hacid/onto/top-level/Agent -->

    <owl:Class rdf:about="https://w3id.org/hacid/onto/top-level/Agent">
        <rdfs:subClassOf rdf:resource="https://w3id.org/hacid/onto/top-level/Object"/>
        <rdfs:comment xml:lang="en">Additional comment: a computational agent can be considered as a PhysicalAgent that realizes a certain class of algorithms (that can be considered as instances of InformationObject) that allow to obtain some behaviors that are considered typical of agents in general. For an ontology of computational objects based on DOLCE see e.g. http://www.loa-cnr.it/COS/COS.owl, and http://www.loa-cnr.it/KCO/KCO.owl.</rdfs:comment>
        <rdfs:comment xml:lang="en">Any agentive Object , either physical (e.g. a whale, a robot, an oak), or social (e.g. a corporation, an institution, a community).</rdfs:comment>
        <rdfs:isDefinedBy rdf:resource="https://w3id.org/hacid/onto/top-level"/>
        <rdfs:label xml:lang="en">Agent</rdfs:label>
        <rdfs:label xml:lang="it">Agente</rdfs:label>
    </owl:Class>
    


    <!-- https://w3id.org/hacid/onto/top-level/Characteristic -->

    <owl:Class rdf:about="https://w3id.org/hacid/onto/top-level/Characteristic">
        <rdfs:subClassOf rdf:resource="https://w3id.org/hacid/onto/top-level/Entity"/>
        <rdfs:comment xml:lang="it">La classe delle caratteristiche, intese come aspetti, attributi o qualità di un'entità. Ex. una quantità, qualità estetica, colore, etc.</rdfs:comment>
        <rdfs:comment xml:lang="en">The class of characteristics, intended as any aspect, attribuite, or quality of an entity. E.g. a certain size, aesthetic quality, color, etc.</rdfs:comment>
        <rdfs:isDefinedBy rdf:resource="https://w3id.org/hacid/onto/top-level"/>
        <rdfs:label xml:lang="it">Caratteristica</rdfs:label>
        <rdfs:label xml:lang="en">Characteristic</rdfs:label>
    </owl:Class>
    


    <!-- https://w3id.org/hacid/onto/top-level/Collection -->

    <owl:Class rdf:about="https://w3id.org/hacid/onto/top-level/Collection">
        <rdfs:subClassOf rdf:resource="https://w3id.org/hacid/onto/top-level/SocialObject"/>
        <rdfs:subClassOf>
            <owl:Restriction>
                <owl:onProperty rdf:resource="https://w3id.org/hacid/onto/top-level/hasMember"/>
                <owl:someValuesFrom rdf:resource="https://w3id.org/hacid/onto/top-level/Entity"/>
            </owl:Restriction>
        </rdfs:subClassOf>
        <rdfs:subClassOf>
            <owl:Restriction>
                <owl:onProperty rdf:resource="https://w3id.org/hacid/onto/top-level/hasPart"/>
                <owl:allValuesFrom rdf:resource="https://w3id.org/hacid/onto/top-level/Collection"/>
            </owl:Restriction>
        </rdfs:subClassOf>
        <rdfs:comment xml:lang="it">La classe per rappresentare collezioni che rendono possibile l'aggregazione di oggetti.</rdfs:comment>
        <rdfs:comment xml:lang="en">The class for representing collections and aggregating objects into collections.</rdfs:comment>
        <rdfs:isDefinedBy rdf:resource="https://w3id.org/hacid/onto/top-level"/>
        <rdfs:label xml:lang="en">Collection</rdfs:label>
        <rdfs:label xml:lang="it">Collezione</rdfs:label>
    </owl:Class>
    


    <!-- https://w3id.org/hacid/onto/top-level/Concept -->

    <owl:Class rdf:about="https://w3id.org/hacid/onto/top-level/Concept">
        <rdfs:subClassOf rdf:resource="https://w3id.org/hacid/onto/top-level/SocialObject"/>
        <rdfs:comment xml:lang="en">It is an object that is defined in some description. Once defined it can be used in other descriptions</rdfs:comment>
        <rdfs:comment xml:lang="it">È un oggetto che è definito in qualche descrizione. Una volta definito può essere utilizzato in altre descrizioni</rdfs:comment>
        <rdfs:isDefinedBy rdf:resource="https://w3id.org/hacid/onto/top-level"/>
        <rdfs:label xml:lang="en">Concept</rdfs:label>
        <rdfs:label xml:lang="it">Concetto</rdfs:label>
    </owl:Class>
    


    <!-- https://w3id.org/hacid/onto/top-level/DataSchema -->

    <owl:Class rdf:about="https://w3id.org/hacid/onto/top-level/DataSchema">
        <rdfs:subClassOf rdf:resource="https://w3id.org/hacid/onto/top-level/Description"/>
        <rdfs:subClassOf>
            <owl:Restriction>
                <owl:onProperty rdf:resource="https://w3id.org/hacid/onto/top-level/hasSchemaAttribute"/>
                <owl:someValuesFrom rdf:resource="https://w3id.org/hacid/onto/top-level/SchemaAttribute"/>
            </owl:Restriction>
        </rdfs:subClassOf>
        <rdfs:subClassOf>
            <owl:Restriction>
                <owl:onProperty rdf:resource="https://w3id.org/hacid/onto/top-level/hasSchemaAttribute"/>
                <owl:allValuesFrom rdf:resource="https://w3id.org/hacid/onto/top-level/SchemaAttribute"/>
            </owl:Restriction>
        </rdfs:subClassOf>
        <owl:disjointWith rdf:resource="https://w3id.org/hacid/onto/top-level/IdentifierSchema"/>
        <rdfs:comment xml:lang="it">La classe per la rappresentazione di schemi di dati.</rdfs:comment>
        <rdfs:comment xml:lang="en">The class for representing data schemata.</rdfs:comment>
        <rdfs:isDefinedBy rdf:resource="https://w3id.org/hacid/onto/top-level"/>
        <rdfs:label xml:lang="en">Data schema</rdfs:label>
        <rdfs:label xml:lang="it">Schema di dati.</rdfs:label>
    </owl:Class>
    


    <!-- https://w3id.org/hacid/onto/top-level/Dataset -->

    <owl:Class rdf:about="https://w3id.org/hacid/onto/top-level/Dataset">
        <rdfs:subClassOf rdf:resource="https://w3id.org/hacid/onto/top-level/Collection"/>
        <rdfs:subClassOf>
            <owl:Restriction>
                <owl:onProperty rdf:resource="https://w3id.org/hacid/onto/top-level/hasPart"/>
                <owl:allValuesFrom rdf:resource="https://w3id.org/hacid/onto/top-level/Dataset"/>
            </owl:Restriction>
        </rdfs:subClassOf>
        <rdfs:comment xml:lang="en">A collection of data.</rdfs:comment>
        <rdfs:comment xml:lang="it">Una collezione di dati.</rdfs:comment>
        <rdfs:isDefinedBy rdf:resource="https://w3id.org/hacid/onto/top-level"/>
        <rdfs:label xml:lang="en">Dataset</rdfs:label>
        <rdfs:label xml:lang="it">Dataset</rdfs:label>
    </owl:Class>
    


    <!-- https://w3id.org/hacid/onto/top-level/Description -->

    <owl:Class rdf:about="https://w3id.org/hacid/onto/top-level/Description">
        <rdfs:subClassOf rdf:resource="https://w3id.org/hacid/onto/top-level/SocialObject"/>
        <owl:disjointWith rdf:resource="https://w3id.org/hacid/onto/top-level/Situation"/>
        <rdfs:comment xml:lang="it">La classe degli oggetti costruiti socialmente (testi, valori, categorie, relazioni, contesti) usati per descrivere qualcos'altro in modo structuratto. Gli esempi includono i piani (come descrizioni strutturate di azioni da eseguire ex. in un processo industriale), le diagnosi (come descrizioni strutturate di situazioni osservate ex. clinicamente), le spiegazioni (come testi strutturati per chiarire ex. un concetto in un sistema normativo), osservazioni oggettive (come insiemi di valori strutturati che identificano una situazione rilevante ex. da un sistema di sensori).</rdfs:comment>
        <rdfs:comment xml:lang="en">The class of socially-created objects (texts, values, categories, relations, contexts) used to describe something else in a structured way. Examples include plans (as structured descriptions of actions to be executed), diagnoses (as structured descriptions of observed situations, explanations (as structured texts clarifying e.g. a concept), objective observations (as structured sets of values that identify a relevant situation).</rdfs:comment>
        <rdfs:isDefinedBy rdf:resource="https://w3id.org/hacid/onto/top-level"/>
        <rdfs:label xml:lang="en">Description</rdfs:label>
        <rdfs:label xml:lang="it">Descrizione</rdfs:label>
    </owl:Class>
    


    <!-- https://w3id.org/hacid/onto/top-level/Entity -->

    <owl:Class rdf:about="https://w3id.org/hacid/onto/top-level/Entity">
        <rdfs:comment xml:lang="en">Anything: real, possible, or imaginary, which some modeller wants to talk about for some purpose.</rdfs:comment>
        <rdfs:isDefinedBy rdf:resource="https://w3id.org/hacid/onto/top-level"/>
        <rdfs:label xml:lang="en">Entity</rdfs:label>
        <rdfs:label xml:lang="it">Entità</rdfs:label>
    </owl:Class>
    


    <!-- https://w3id.org/hacid/onto/top-level/Event -->

    <owl:Class rdf:about="https://w3id.org/hacid/onto/top-level/Event">
        <rdfs:subClassOf rdf:resource="https://w3id.org/hacid/onto/top-level/Entity"/>
        <rdfs:subClassOf>
            <owl:Restriction>
                <owl:onProperty rdf:resource="https://w3id.org/hacid/onto/top-level/hasPart"/>
                <owl:someValuesFrom rdf:resource="https://w3id.org/hacid/onto/top-level/Event"/>
            </owl:Restriction>
        </rdfs:subClassOf>
        <rdfs:comment xml:lang="en">Any physical, social, or mental process, event, or state.</rdfs:comment>
        <rdfs:comment xml:lang="it">Qualsiasi processo, evento o stato fisico, sociale o mentale.</rdfs:comment>
        <rdfs:isDefinedBy rdf:resource="https://w3id.org/hacid/onto/top-level"/>
        <rdfs:label xml:lang="en">Event</rdfs:label>
        <rdfs:label xml:lang="it">Evento</rdfs:label>
    </owl:Class>
    


    <!-- https://w3id.org/hacid/onto/top-level/FormalEntity -->

    <owl:Class rdf:about="https://w3id.org/hacid/onto/top-level/FormalEntity">
        <rdfs:subClassOf rdf:resource="https://w3id.org/hacid/onto/top-level/Entity"/>
        <rdfs:comment xml:lang="en">Entities that are formally defined and are considered independent from the social context in which they are used. They cannot be localized in space or time. Also called 'Platonic entities'.
Mathematical and logical entities are included in this class: sets, categories, tuples, costants, variables, etc.</rdfs:comment>
        <rdfs:comment xml:lang="it">Entità formalmente definite e considerate indipendenti dal contesto sociale in cui vengono utilizzate. Non possono essere localizzati nello spazio o nel tempo. Chiamate anche "entità platoniche".
In questa classe sono incluse le entità matematiche e logiche: insiemi, categorie, tuple, costanti, variabili, ecc.</rdfs:comment>
        <rdfs:isDefinedBy rdf:resource="https://w3id.org/hacid/onto/top-level"/>
        <rdfs:label xml:lang="it">Entità formale astratta</rdfs:label>
        <rdfs:label xml:lang="en">Formal entity</rdfs:label>
    </owl:Class>
    


    <!-- https://w3id.org/hacid/onto/top-level/Goal -->

    <owl:Class rdf:about="https://w3id.org/hacid/onto/top-level/Goal">
        <rdfs:comment xml:lang="en">The Description of a Situation that is desired by an Agent, and usually associated to a Plan that describes how to actually achieve it</rdfs:comment>
        <rdfs:isDefinedBy rdf:resource="https://w3id.org/hacid/onto/top-level"/>
        <rdfs:label xml:lang="en">Goal</rdfs:label>
        <rdfs:label xml:lang="it">Scopo</rdfs:label>
    </owl:Class>
    


    <!-- https://w3id.org/hacid/onto/top-level/IdentifierSchema -->

    <owl:Class rdf:about="https://w3id.org/hacid/onto/top-level/IdentifierSchema">
        <rdfs:subClassOf rdf:resource="https://w3id.org/hacid/onto/top-level/Description"/>
        <rdfs:comment xml:lang="en">A schema for identifiers.</rdfs:comment>
        <rdfs:comment xml:lang="it">Uno schema di identificativi.</rdfs:comment>
        <rdfs:isDefinedBy rdf:resource="https://w3id.org/hacid/onto/top-level"/>
        <rdfs:label xml:lang="en">Identifier schema</rdfs:label>
        <rdfs:label xml:lang="it">Schema di identificatori</rdfs:label>
    </owl:Class>
    


    <!-- https://w3id.org/hacid/onto/top-level/InformationEntity -->

    <owl:Class rdf:about="https://w3id.org/hacid/onto/top-level/InformationEntity">
        <rdfs:subClassOf rdf:resource="https://w3id.org/hacid/onto/top-level/Entity"/>
        <rdfs:comment xml:lang="en">A piece of information, be it concretely realised or not. It is a catchall class, intended to bypass the ambiguities of many data or text that could denote either a an expression or a concrete realisation of that expression.
In a semiotic model, there is no special reason to distinguish between them, however we may want to distinguish between a pure information content (e.g. the 3rd Gymnopedie by Satie), and its possible concrete realisations as a music sheet, a piano execution, the reproduction of the execution, its publishing as a record, etc.).</rdfs:comment>
        <rdfs:comment xml:lang="it">Un'informazione, concretamente realizzata o meno. È una classe generica, intesa a superare le ambiguità di molti dati o testo che potrebbero denotare un'espressione o una realizzazione concreta di tale espressione.
In un modello semiotico non vi è alcuna ragione particolare per distinguerli, tuttavia potremmo voler distinguere tra un contenuto puramente informativo (ad esempio la 3a Gymnopedie di Satie) e le sue possibili realizzazioni concrete come uno spartito, un'esecuzione pianistica, il riproduzione dell'esecuzione, sua pubblicazione in forma verbale, ecc.).</rdfs:comment>
        <rdfs:isDefinedBy rdf:resource="https://w3id.org/hacid/onto/top-level"/>
        <rdfs:label xml:lang="it">Entità informativa</rdfs:label>
        <rdfs:label xml:lang="en">Information entity</rdfs:label>
    </owl:Class>
    


    <!-- https://w3id.org/hacid/onto/top-level/Judgement -->

    <owl:Class rdf:about="https://w3id.org/hacid/onto/top-level/Judgement">
        <rdfs:subClassOf rdf:resource="https://w3id.org/hacid/onto/top-level/Entity"/>
        <rdfs:comment xml:lang="it">Il processo di formazione di un'opinione o di valutazione attraverso il discernimento e il confronto.</rdfs:comment>
        <rdfs:comment xml:lang="en">The process of forming an opinion or evaluation by discerning and comparing.</rdfs:comment>
        <rdfs:isDefinedBy rdf:resource="https://w3id.org/hacid/onto/top-level"/>
        <rdfs:label xml:lang="it">Giudizio</rdfs:label>
        <rdfs:label xml:lang="en">Judgement</rdfs:label>
    </owl:Class>
    


    <!-- https://w3id.org/hacid/onto/top-level/Location -->

    <owl:Class rdf:about="https://w3id.org/hacid/onto/top-level/Location">
        <rdfs:subClassOf rdf:resource="https://w3id.org/hacid/onto/top-level/SocialObject"/>
        <rdfs:comment xml:lang="it">Il concetto più generico per rappresentare ad alto livello qualsiasi tipo di oggetto che possa essere identificato come luogo.</rdfs:comment>
        <rdfs:comment xml:lang="en">The most generic concept for any kind of location.</rdfs:comment>
        <rdfs:isDefinedBy rdf:resource="https://w3id.org/hacid/onto/top-level"/>
        <rdfs:label xml:lang="it">Luogo</rdfs:label>
        <rdfs:label xml:lang="en">Place</rdfs:label>
    </owl:Class>
    


    <!-- https://w3id.org/hacid/onto/top-level/Material -->

    <owl:Class rdf:about="https://w3id.org/hacid/onto/top-level/Material">
        <rdfs:subClassOf rdf:resource="https://w3id.org/hacid/onto/top-level/Characteristic"/>
        <rdfs:comment xml:lang="it">La classe dei materiali.</rdfs:comment>
        <rdfs:comment xml:lang="en">The material class</rdfs:comment>
        <rdfs:isDefinedBy rdf:resource="https://w3id.org/hacid/onto/top-level"/>
        <rdfs:label xml:lang="en">Material</rdfs:label>
        <rdfs:label xml:lang="it">Materiale</rdfs:label>
    </owl:Class>
    


    <!-- https://w3id.org/hacid/onto/top-level/Media -->

    <owl:Class rdf:about="https://w3id.org/hacid/onto/top-level/Media">
        <rdfs:subClassOf rdf:resource="https://w3id.org/hacid/onto/top-level/Entity"/>
        <rdfs:subClassOf>
            <owl:Restriction>
                <owl:onProperty rdf:resource="https://w3id.org/hacid/onto/top-level/isSouceOf"/>
                <owl:someValuesFrom rdf:resource="https://w3id.org/hacid/onto/top-level/Entity"/>
            </owl:Restriction>
        </rdfs:subClassOf>
        <rdfs:subClassOf>
            <owl:Restriction>
                <owl:onProperty rdf:resource="https://w3id.org/hacid/onto/top-level/hasDataSchema"/>
                <owl:qualifiedCardinality rdf:datatype="http://www.w3.org/2001/XMLSchema#nonNegativeInteger">1</owl:qualifiedCardinality>
                <owl:onClass rdf:resource="https://w3id.org/hacid/onto/top-level/DataSchema"/>
            </owl:Restriction>
        </rdfs:subClassOf>
        <rdfs:subClassOf>
            <owl:Restriction>
                <owl:onProperty rdf:resource="https://w3id.org/hacid/onto/top-level/hasDownloadURL"/>
                <owl:cardinality rdf:datatype="http://www.w3.org/2001/XMLSchema#nonNegativeInteger">1</owl:cardinality>
            </owl:Restriction>
        </rdfs:subClassOf>
        <rdfs:subClassOf>
            <owl:Restriction>
                <owl:onProperty rdf:resource="https://w3id.org/hacid/onto/top-level/mediaType"/>
                <owl:cardinality rdf:datatype="http://www.w3.org/2001/XMLSchema#nonNegativeInteger">1</owl:cardinality>
            </owl:Restriction>
        </rdfs:subClassOf>
        <rdfs:comment xml:lang="en">Any media encoding data in any format.</rdfs:comment>
        <rdfs:comment xml:lang="it">Qualsiasi supporto che codifica i dati in qualsiasi formato.</rdfs:comment>
        <rdfs:isDefinedBy rdf:resource="https://w3id.org/hacid/onto/top-level"/>
        <rdfs:label xml:lang="en">Media</rdfs:label>
        <rdfs:label xml:lang="it">Media</rdfs:label>
    </owl:Class>
    


    <!-- https://w3id.org/hacid/onto/top-level/Object -->

    <owl:Class rdf:about="https://w3id.org/hacid/onto/top-level/Object">
        <rdfs:subClassOf rdf:resource="https://w3id.org/hacid/onto/top-level/Entity"/>
        <rdfs:comment xml:lang="en">Any physical, social, or mental object, or a substance. Following DOLCE Full, objects are always participating in some event (at least their own life), and are spatially located.</rdfs:comment>
        <rdfs:isDefinedBy rdf:resource="https://w3id.org/hacid/onto/top-level"/>
        <rdfs:label xml:lang="en">Object</rdfs:label>
        <rdfs:label xml:lang="it">Oggetto</rdfs:label>
    </owl:Class>
    


    <!-- https://w3id.org/hacid/onto/top-level/ObjectRoleAssignment -->

    <owl:Class rdf:about="https://w3id.org/hacid/onto/top-level/ObjectRoleAssignment">
        <rdfs:subClassOf rdf:resource="https://w3id.org/hacid/onto/top-level/Situation"/>
        <rdfs:isDefinedBy rdf:resource="https://w3id.org/hacid/onto/top-level"/>
        <rdfs:label xml:lang="en">Object role assignement</rdfs:label>
        <rdfs:comment xml:lang="en">The assignement of an object to a role contextualized to a specific situation.</rdfs:comment>
    </owl:Class>
    


    <!-- https://w3id.org/hacid/onto/top-level/Organization -->

    <owl:Class rdf:about="https://w3id.org/hacid/onto/top-level/Organization">
        <rdfs:subClassOf rdf:resource="https://w3id.org/hacid/onto/top-level/Agent"/>
        <owl:disjointWith rdf:resource="https://w3id.org/hacid/onto/top-level/Person"/>
        <rdfs:comment xml:lang="en">An organisation.</rdfs:comment>
        <rdfs:comment xml:lang="it">Un'organizzazione.</rdfs:comment>
        <rdfs:isDefinedBy rdf:resource="https://w3id.org/hacid/onto/top-level"/>
        <rdfs:label xml:lang="en">Organisation</rdfs:label>
        <rdfs:label xml:lang="it">Organizzazione</rdfs:label>
    </owl:Class>
    


    <!-- https://w3id.org/hacid/onto/top-level/Parameter -->

    <owl:Class rdf:about="https://w3id.org/hacid/onto/top-level/Parameter">
        <rdfs:subClassOf rdf:resource="https://w3id.org/hacid/onto/top-level/Characteristic"/>
        <rdfs:subClassOf rdf:resource="https://w3id.org/hacid/onto/top-level/Concept"/>
        <rdfs:comment xml:lang="it">La classe dei parametri. Esempio, il parametro di un'osservazione.</rdfs:comment>
        <rdfs:comment xml:lang="en">The class of parameters. Example, the parameter of an observation.</rdfs:comment>
        <rdfs:isDefinedBy rdf:resource="https://w3id.org/hacid/onto/top-level"/>
        <rdfs:label xml:lang="en">Parameter</rdfs:label>
        <rdfs:label xml:lang="it">Parametro</rdfs:label>
        <owl:versionInfo xml:lang="it">stabile</owl:versionInfo>
        <owl:versionInfo xml:lang="en">stable</owl:versionInfo>
    </owl:Class>
    


    <!-- https://w3id.org/hacid/onto/top-level/Person -->

    <owl:Class rdf:about="https://w3id.org/hacid/onto/top-level/Person">
        <rdfs:subClassOf rdf:resource="https://w3id.org/hacid/onto/top-level/Agent"/>
        <rdfs:comment xml:lang="en">A person</rdfs:comment>
        <rdfs:comment xml:lang="it">Una persona.</rdfs:comment>
        <rdfs:isDefinedBy rdf:resource="https://w3id.org/hacid/onto/top-level"/>
        <rdfs:label xml:lang="en">Person</rdfs:label>
        <rdfs:label xml:lang="it">Persona</rdfs:label>
    </owl:Class>
    


    <!-- https://w3id.org/hacid/onto/top-level/PhysicalObject -->

    <owl:Class rdf:about="https://w3id.org/hacid/onto/top-level/PhysicalObject">
        <rdfs:subClassOf rdf:resource="https://w3id.org/hacid/onto/top-level/Object"/>
        <rdfs:comment xml:lang="en">Any Object that has a proper space region. The prototypical physical object has also an associated mass, but the nature of its mass can greatly vary based on the epistemological status of the object (scientifically measured, subjectively possible, imaginary).</rdfs:comment>
        <rdfs:comment xml:lang="it">Qualsiasi oggetto che abbia una propria regione spaziale. L'oggetto fisico prototipico ha anche una massa associata, ma la natura della sua massa può variare notevolmente in base allo status epistemologico dell'oggetto (scientificamente misurato, soggettivamente possibile, immaginario).</rdfs:comment>
        <rdfs:isDefinedBy rdf:resource="https://w3id.org/hacid/onto/top-level"/>
        <rdfs:label xml:lang="it">Oggetto fisico</rdfs:label>
        <rdfs:label xml:lang="en">Physical object</rdfs:label>
    </owl:Class>
    


    <!-- https://w3id.org/hacid/onto/top-level/Region -->

    <owl:Class rdf:about="https://w3id.org/hacid/onto/top-level/Region">
        <rdfs:subClassOf rdf:resource="https://w3id.org/hacid/onto/top-level/FormalEntity"/>
        <rdfs:comment xml:lang="en">Any region in a dimensional space (a dimensional space is a maximal Region), which can be used as a value for a quality of an Entity . For example, TimeInterval, SpaceRegion, PhysicalAttribute, Amount, SocialAttribute are all subclasses of Region.</rdfs:comment>
        <rdfs:comment xml:lang="it">Qualsiasi regione in uno spazio dimensionale (uno spazio dimensionale è una regione massimale), che può essere utilizzata come valore per una qualità di un'entità. Ad esempio, TimeInterval, SpaceRegion, PhysicalAttribute, Amount, SocialAttribute sono tutte sottoclassi di Region.</rdfs:comment>
        <rdfs:isDefinedBy rdf:resource="https://w3id.org/hacid/onto/top-level"/>
        <rdfs:label xml:lang="en">Region</rdfs:label>
        <rdfs:label xml:lang="it">Regione</rdfs:label>
    </owl:Class>
    


    <!-- https://w3id.org/hacid/onto/top-level/Role -->

    <owl:Class rdf:about="https://w3id.org/hacid/onto/top-level/Role">
        <rdfs:subClassOf rdf:resource="https://w3id.org/hacid/onto/top-level/Concept"/>
        <rdfs:comment xml:lang="it">La classe per rappresentare i ruoli.</rdfs:comment>
        <rdfs:comment xml:lang="en">The class for representing roles.</rdfs:comment>
        <rdfs:isDefinedBy rdf:resource="https://w3id.org/hacid/onto/top-level"/>
        <rdfs:label xml:lang="en">Role</rdfs:label>
        <rdfs:label xml:lang="it">Ruolo</rdfs:label>
    </owl:Class>
    


    <!-- https://w3id.org/hacid/onto/top-level/SchemaAttribute -->

    <owl:Class rdf:about="https://w3id.org/hacid/onto/top-level/SchemaAttribute">
        <rdfs:subClassOf rdf:resource="https://w3id.org/hacid/onto/top-level/Characteristic"/>
        <rdfs:subClassOf>
            <owl:Restriction>
                <owl:onProperty rdf:resource="https://w3id.org/hacid/onto/top-level/isClassifiedBy"/>
                <owl:someValuesFrom rdf:resource="https://w3id.org/hacid/onto/top-level/Concept"/>
            </owl:Restriction>
        </rdfs:subClassOf>
        <rdfs:comment xml:lang="it">La classe degli attributi di uno schema dati</rdfs:comment>
        <rdfs:comment xml:lang="en">The class of the attributes of a data schema.</rdfs:comment>
        <rdfs:isDefinedBy rdf:resource="https://w3id.org/hacid/onto/top-level"/>
        <rdfs:label xml:lang="it">Attributo dello Schema</rdfs:label>
        <rdfs:label xml:lang="en">Schema attribute</rdfs:label>
        <owl:versionInfo xml:lang="it">stabile</owl:versionInfo>
        <owl:versionInfo xml:lang="en">stable</owl:versionInfo>
    </owl:Class>
    


    <!-- https://w3id.org/hacid/onto/top-level/Situation -->

    <owl:Class rdf:about="https://w3id.org/hacid/onto/top-level/Situation">
        <rdfs:subClassOf rdf:resource="https://w3id.org/hacid/onto/top-level/Entity"/>
        <rdfs:subClassOf>
            <owl:Restriction>
                <owl:onProperty rdf:resource="https://w3id.org/hacid/onto/top-level/satisfies"/>
                <owl:someValuesFrom rdf:resource="https://w3id.org/hacid/onto/top-level/Description"/>
            </owl:Restriction>
        </rdfs:subClassOf>
        <rdfs:comment xml:lang="en">Any event, situation, activity, event type, etc. Used to abstract from formal criteria that distinguish between event occurrences, their types, and constructed objects (situations, tropes, qua-entities) that provide a setting for multiple entities.
This is a catch all class to make sense of ambiguous data that cannot be made more precise, e.g. at the lexical level.
This is the same concept as defined in http://www.ontologydesignpatterns.org/ont/d0.owl.</rdfs:comment>
        <rdfs:comment xml:lang="it">Qualsiasi evento, situazione, attività, tipo di evento, ecc. Utilizzato per astrarre da criteri formali che distinguono tra occorrenze di eventi, i loro tipi e oggetti costruiti (situazioni, tropi, qua-entità) che forniscono un'ambientazione per più entità.
Questa è una classe catch all per dare un senso a dati ambigui che non possono essere resi più precisi, ad es. a livello lessicale.
Questo è lo stesso concetto definito in http://www.ontologydesignpatterns.org/ont/d0.owl.</rdfs:comment>
        <rdfs:isDefinedBy rdf:resource="https://w3id.org/hacid/onto/top-level"/>
        <rdfs:label xml:lang="en">Situation</rdfs:label>
        <rdfs:label xml:lang="it">Situazione</rdfs:label>
    </owl:Class>
    


    <!-- https://w3id.org/hacid/onto/top-level/SocialObject -->

    <owl:Class rdf:about="https://w3id.org/hacid/onto/top-level/SocialObject">
        <rdfs:subClassOf rdf:resource="https://w3id.org/hacid/onto/top-level/Object"/>
        <rdfs:comment xml:lang="en">Any Object that exists only within some communication Event, in which at least one PhysicalObject participates in. 
In other words, all objects that have been or are created in the process of social communication: for the sake of communication (InformationObject), for incorporating new individuals (SocialAgent, Place), for contextualizing or intepreting existing entities (Description, Concept), or for collecting existing entities (Collection).
Being dependent on communication, all social objects need to be expressed by some information object (information objects are self-expressing).</rdfs:comment>
        <rdfs:isDefinedBy rdf:resource="https://w3id.org/hacid/onto/top-level"/>
        <rdfs:label xml:lang="it">Oggetto sociale</rdfs:label>
        <rdfs:label xml:lang="en">Social object</rdfs:label>
    </owl:Class>
    


    <!-- https://w3id.org/hacid/onto/top-level/System -->

    <owl:Class rdf:about="https://w3id.org/hacid/onto/top-level/System">
        <rdfs:subClassOf rdf:resource="https://w3id.org/hacid/onto/top-level/Entity"/>
        <rdfs:comment xml:lang="en">Any possible kind of system.</rdfs:comment>
        <rdfs:comment xml:lang="it">Ogni possibile tipo di sistema.</rdfs:comment>
        <rdfs:isDefinedBy rdf:resource="https://w3id.org/hacid/onto/top-level"/>
        <rdfs:label xml:lang="it">Sistema</rdfs:label>
        <rdfs:label xml:lang="en">System</rdfs:label>
    </owl:Class>
    


    <!-- https://w3id.org/hacid/onto/top-level/Task -->

    <owl:Class rdf:about="https://w3id.org/hacid/onto/top-level/Task">
        <rdfs:subClassOf rdf:resource="https://w3id.org/hacid/onto/top-level/Concept"/>
        <rdfs:comment xml:lang="en">An EventType that classifies an Action to be executed. 
For example, reaching a destination is a task that can be executed by performing certain actions, e.g. driving a car, buying a train ticket, etc. 
The actions to execute a task can also be organized according to a Plan that is not the same as the one that defines the task (if any). 
For example, reaching a destination could be defined by a plan to get on holidays, while the plan to execute the task can consist of putting some travels into a sequence.</rdfs:comment>
        <rdfs:isDefinedBy rdf:resource="https://w3id.org/hacid/onto/top-level"/>
        <rdfs:label xml:lang="en">Task</rdfs:label>
        <rdfs:label xml:lang="it">Task</rdfs:label>
    </owl:Class>
    


    <!-- https://w3id.org/hacid/onto/top-level/TemporalEntity -->

    <owl:Class rdf:about="https://w3id.org/hacid/onto/top-level/TemporalEntity">
        <rdfs:subClassOf rdf:resource="https://w3id.org/hacid/onto/top-level/Entity"/>
        <rdfs:subClassOf>
            <owl:Restriction>
                <owl:onProperty rdf:resource="https://w3id.org/hacid/onto/top-level/time"/>
                <owl:someValuesFrom rdf:resource="http://www.w3.org/2001/XMLSchema#dateTime"/>
            </owl:Restriction>
        </rdfs:subClassOf>
        <rdfs:subClassOf>
            <owl:Restriction>
                <owl:onProperty rdf:resource="https://w3id.org/hacid/onto/top-level/time"/>
                <owl:allValuesFrom rdf:resource="http://www.w3.org/2001/XMLSchema#dateTime"/>
            </owl:Restriction>
        </rdfs:subClassOf>
        <rdfs:comment xml:lang="it">Questa classe rappresenta qualsiasi tipo di entità temporale, ad es. intervalli di tempo, mesi, giorni, ecc...</rdfs:comment>
        <rdfs:comment xml:lang="en">This class represents a temporal entity.</rdfs:comment>
        <rdfs:isDefinedBy rdf:resource="https://w3id.org/hacid/onto/top-level"/>
        <rdfs:label xml:lang="it">Entità temporale</rdfs:label>
        <rdfs:label xml:lang="en">Temporal entity</rdfs:label>
    </owl:Class>
    


    <!-- https://w3id.org/hacid/onto/top-level/TimeInterval -->

    <owl:Class rdf:about="https://w3id.org/hacid/onto/top-level/TimeInterval">
        <rdfs:subClassOf rdf:resource="https://w3id.org/hacid/onto/top-level/TemporalEntity"/>
        <rdfs:subClassOf>
            <owl:Restriction>
                <owl:onProperty rdf:resource="https://w3id.org/hacid/onto/top-level/endTime"/>
                <owl:maxQualifiedCardinality rdf:datatype="http://www.w3.org/2001/XMLSchema#nonNegativeInteger">1</owl:maxQualifiedCardinality>
                <owl:onDataRange>
                    <rdfs:Datatype>
                        <owl:unionOf rdf:parseType="Collection">
                            <rdf:Description rdf:about="http://www.w3.org/2001/XMLSchema#date"/>
                            <rdf:Description rdf:about="http://www.w3.org/2001/XMLSchema#dateTime"/>
                            <rdf:Description rdf:about="http://www.w3.org/2001/XMLSchema#time"/>
                        </owl:unionOf>
                    </rdfs:Datatype>
                </owl:onDataRange>
            </owl:Restriction>
        </rdfs:subClassOf>
        <rdfs:subClassOf>
            <owl:Restriction>
                <owl:onProperty rdf:resource="https://w3id.org/hacid/onto/top-level/startTime"/>
                <owl:maxQualifiedCardinality rdf:datatype="http://www.w3.org/2001/XMLSchema#nonNegativeInteger">1</owl:maxQualifiedCardinality>
                <owl:onDataRange>
                    <rdfs:Datatype>
                        <owl:unionOf rdf:parseType="Collection">
                            <rdf:Description rdf:about="http://www.w3.org/2001/XMLSchema#date"/>
                            <rdf:Description rdf:about="http://www.w3.org/2001/XMLSchema#dateTime"/>
                            <rdf:Description rdf:about="http://www.w3.org/2001/XMLSchema#time"/>
                        </owl:unionOf>
                    </rdfs:Datatype>
                </owl:onDataRange>
            </owl:Restriction>
        </rdfs:subClassOf>
        <rdfs:comment xml:lang="it">La classe per rappresentare gli intervalli temporali aventi un inizio ed una fine.</rdfs:comment>
        <rdfs:comment xml:lang="en">The class for representing time intervals having a start and end time.</rdfs:comment>
        <rdfs:isDefinedBy rdf:resource="https://w3id.org/hacid/onto/top-level"/>
        <rdfs:label xml:lang="it">Intervallo di tempo</rdfs:label>
        <rdfs:label xml:lang="en">Time interval</rdfs:label>
    </owl:Class>
    


    <!-- https://w3id.org/hacid/onto/top-level/UnitOfMeasure -->

    <owl:Class rdf:about="https://w3id.org/hacid/onto/top-level/UnitOfMeasure">
        <rdfs:subClassOf rdf:resource="https://w3id.org/hacid/onto/top-level/Parameter"/>
        <rdfs:comment xml:lang="it">Questa classe viene utilizzata per modellare un'unità di misura, ad es. metro, chilometro, grammo, ecc...</rdfs:comment>
        <rdfs:comment xml:lang="en">This class is used to model a measurement unit, e.g. meter, kilometer, gram, etc.</rdfs:comment>
        <rdfs:isDefinedBy rdf:resource="https://w3id.org/hacid/onto/top-level"/>
        <rdfs:label xml:lang="en">Unit of measure</rdfs:label>
        <rdfs:label xml:lang="it">Unità di misura</rdfs:label>
    </owl:Class>
    


    <!-- https://w3id.org/hacid/onto/top-level/Value -->

    <owl:Class rdf:about="https://w3id.org/hacid/onto/top-level/Value">
        <rdfs:subClassOf rdf:resource="https://w3id.org/hacid/onto/top-level/Characteristic"/>
        <rdfs:subClassOf>
            <owl:Restriction>
                <owl:onProperty rdf:resource="https://w3id.org/hacid/onto/top-level/hasUnitOfMeasure"/>
                <owl:maxQualifiedCardinality rdf:datatype="http://www.w3.org/2001/XMLSchema#nonNegativeInteger">1</owl:maxQualifiedCardinality>
                <owl:onClass rdf:resource="https://w3id.org/hacid/onto/top-level/UnitOfMeasure"/>
            </owl:Restriction>
        </rdfs:subClassOf>
        <rdfs:subClassOf>
            <owl:Restriction>
                <owl:onProperty rdf:resource="https://w3id.org/hacid/onto/top-level/value"/>
                <owl:cardinality rdf:datatype="http://www.w3.org/2001/XMLSchema#nonNegativeInteger">1</owl:cardinality>
            </owl:Restriction>
        </rdfs:subClassOf>
        <owl:hasKey rdf:parseType="Collection">
            <rdf:Description rdf:about="https://w3id.org/hacid/onto/top-level/hasUnitOfMeasure"/>
            <rdf:Description rdf:about="https://w3id.org/hacid/onto/top-level/value"/>
        </owl:hasKey>
        <rdfs:comment xml:lang="it">La classe che modella generici valori che tipicamente hanno un'unità di misura e il valore stesso.</rdfs:comment>
        <rdfs:comment xml:lang="en">The generic class for the values that typically have the unit of measure and the value itself.</rdfs:comment>
        <rdfs:isDefinedBy rdf:resource="https://w3id.org/hacid/onto/top-level"/>
        <rdfs:label xml:lang="it">Valore</rdfs:label>
        <rdfs:label xml:lang="en">Value</rdfs:label>
        <owl:versionInfo xml:lang="it">stabile</owl:versionInfo>
        <owl:versionInfo xml:lang="en">stable</owl:versionInfo>
    </owl:Class>
    


    <!-- https://w3id.org/hacid/onto/top-level/Workflow -->

    <owl:Class rdf:about="https://w3id.org/hacid/onto/top-level/Workflow">
        <rdfs:subClassOf rdf:resource="https://w3id.org/hacid/onto/top-level/Description"/>
        <rdfs:comment xml:lang="en">A workflow with tasks.</rdfs:comment>
        <rdfs:comment xml:lang="it">Un flusso di lavoro composto da attività.</rdfs:comment>
        <rdfs:isDefinedBy rdf:resource="https://w3id.org/hacid/onto/top-level"/>
        <rdfs:label xml:lang="it">Flusso di lavoro</rdfs:label>
        <rdfs:label xml:lang="en">Workflow</rdfs:label>
    </owl:Class>
    


    <!-- https://w3id.org/hacid/onto/top-level/WorkflowExecution -->

    <owl:Class rdf:about="https://w3id.org/hacid/onto/top-level/WorkflowExecution">
        <owl:equivalentClass>
            <owl:Restriction>
                <owl:onProperty rdf:resource="https://w3id.org/hacid/onto/top-level/satisfies"/>
                <owl:someValuesFrom rdf:resource="https://w3id.org/hacid/onto/top-level/Workflow"/>
            </owl:Restriction>
        </owl:equivalentClass>
        <rdfs:subClassOf rdf:resource="https://w3id.org/hacid/onto/top-level/Situation"/>
        <rdfs:isDefinedBy rdf:resource="https://w3id.org/hacid/onto/top-level"/>
        <rdfs:label xml:lang="it">Esecuzione di workflow</rdfs:label>
        <rdfs:label xml:lang="en">Workflow execution</rdfs:label>
        <rdfs:comment xml:lang="en">The execution of a workflow, i.e. a situation that satisfies a workflow.</rdfs:comment>
        <rdfs:isDefinedBy rdf:resource="https://w3id.org/hacid/onto/top-level"/>
    </owl:Class>
    


    <!-- https://w3id.org/hacid/onto/top-level/WorkflowRole -->

    <owl:Class rdf:about="https://w3id.org/hacid/onto/top-level/WorkflowRole">
        <rdfs:subClassOf rdf:resource="http://www.w3.org/2000/01/rdf-schema#Property"/>
        <rdfs:subClassOf rdf:resource="https://w3id.org/hacid/onto/top-level/Role"/>
        <rdfs:subClassOf>
            <owl:Restriction>
                <owl:onProperty rdf:resource="http://www.w3.org/2000/01/rdf-schema#domain"/>
                <owl:allValuesFrom rdf:resource="https://w3id.org/hacid/onto/top-level/WorkflowExecution"/>
            </owl:Restriction>
        </rdfs:subClassOf>
        <rdfs:comment xml:lang="en">A role of a workflow, also a property with WorkflowExecution as domain, to enable the concise representation of objects assigned to the role.</rdfs:comment>
        <rdfs:isDefinedBy rdf:resource="https://w3id.org/hacid/onto/top-level"/>
        <rdfs:label xml:lang="en">Workflow role</rdfs:label>
    </owl:Class>
    


    <!-- https://w3id.org/hacid/onto/top-level/Year -->

    <owl:Class rdf:about="https://w3id.org/hacid/onto/top-level/Year">
        <rdfs:subClassOf rdf:resource="https://w3id.org/hacid/onto/top-level/TemporalEntity"/>
        <rdfs:subClassOf>
            <owl:Restriction>
                <owl:onProperty rdf:resource="https://w3id.org/hacid/onto/top-level/year"/>
                <owl:maxQualifiedCardinality rdf:datatype="http://www.w3.org/2001/XMLSchema#nonNegativeInteger">1</owl:maxQualifiedCardinality>
                <owl:onDataRange rdf:resource="http://www.w3.org/2001/XMLSchema#gYear"/>
            </owl:Restriction>
        </rdfs:subClassOf>
        <rdfs:comment xml:lang="it">La classe per rappresentare un anno.</rdfs:comment>
        <rdfs:comment xml:lang="en">The class for representing a year.</rdfs:comment>
        <rdfs:isDefinedBy rdf:resource="https://w3id.org/hacid/onto/top-level"/>
        <rdfs:label xml:lang="it">Anno</rdfs:label>
        <rdfs:label xml:lang="en">Year</rdfs:label>
    </owl:Class>
</rdf:RDF><!-- Generated by the OWL API (version 4.5.29) https://github.com/owlcs/owlapi -->
