<rdf:RDF xmlns:rdf="http://www.w3.org/1999/02/22-rdf-syntax-ns#" xmlns:terms="http://purl.org/dc/terms/" xmlns:rdfs="http://www.w3.org/2000/01/rdf-schema#" xmlns:owl="http://www.w3.org/2002/07/owl#" xml:base="https://w3id.org/hacid/onto/data">
    <owl:Ontology rdf:about="https://w3id.org/hacid/onto/data">
        <owl:imports rdf:resource="https://w3id.org/hacid/onto/top-level"/>
        <terms:title xml:lang="en">HACID data ontology module</terms:title>
        <rdfs:comment xml:lang="en">This module provides a semantically rich way to represent variables (which may be dependent from other variables or not, computationally derived from other variables or not), the dimensional spaces they take values in (which can be discrete or continuous, made of points or extended regions, limited or not, derived-from/part-of other dimensional spaces), and concrete datasets.

The aim is to represent the concept of variables in a flexible way, while preserving well-defined semantics. Here, as usual in mathematics and other fields, a variable is an abstraction that has meaning in the context of some relation between different variables and can be associated to different values in a set that is usually well defined (e.g., x is anelement of ℝ). In the ontology module presented here, a data:Variable is akin to that concept and the set of possible values is represented by a data:DimensionalSpace; the two are linked via the data:hasValuesOn property. To a variable that is a data:DependentVariable can be implicitly associated with a function having as range the associated dimensional space and as domain the cartesian set of the dimensional spaces of the variables from which it depends. A data:IndependentVariable, conversely, is a variable that does not depend on other variables.

A variable can be aggregating, i.e. include aggregation mechanisms whose execution is deferred to derived variables. This allows to represent variables defined using one or more aggregation functions for combining data along one or more independent variables, without specifying the actual granularity. A general purpose example of usage is representing as variables the SQL expressions including aggregation functions (e.g. AVG(...)) which are then derived to actual serialisable variables by the usage of specific GROUP BY clauses. In the context of climate services, the CMOR Tables variables (e.g., tasmax) fall into this category. From the ontology point of view, a (dependent) variable is aggregating if it offers one or more aggregations: i.e. it is linked with one or more instances of  data:Aggregation via the property data:definesAggregation. Each aggregation is associated with one variable (which must be a variable the dependent variable depends on) and optionally one or more suggested options for the adopted aggregation grid (i.e. specific granularity).

A data:FiniteVariable is a variable for which the set of all the possible values is finite. For an independent variable it means being defined on a finite dimensional space (instance of data:FiniteDimensionalSpace); for a dependent variable it means that all the variables it depends on are finite variables. The concept of data:FiniteVariable is important because it corresponds to variables that can be fully represented extensively with a finite amount of resources. It corresponds functionally to the concept of a dataset. The property data:hasDataSerialisation links such a dataset with a data source (data:DataSource) holding one or more concrete serialisations of it. A data:DataSource (e.g., an URL resolving to a dump of a dataset) is associated to one or more supported data formats (data:DataFormat) via the data:hasAvailableDataFormat property. 

A data:DimensionalSpace is composed of a set (not necessarily finite) of regions (data:Region). It can be either continuous (data:Continuum) or discrete (data:DiscreteDimensionalSpace). A discrete dimensional space can be a grid (data:Grid), i.e. composed of a set of regions that form a partition of all the space.

In order to avoid unnecessary complexity in concrete usage, a data:DimensionalSpace is also a data:IndependentVariable. Conceptually, it associates a dimensional space with a “default variable” with values on that dimensional space (on itself). This allows using directly a dimensional space as a variable when there are no possible ambiguities: e.g., a variable representing time in a context where no other variables represent time, can be directly represented by the corresponding temporal dimensional space.</rdfs:comment>
        <rdfs:label xml:lang="en">HACID data ontology module</rdfs:label>
    </owl:Ontology>
    


    <!-- 
    ///////////////////////////////////////////////////////////////////////////////////////
    //
    // Annotation properties
    //
    ///////////////////////////////////////////////////////////////////////////////////////
     -->

    


    <!-- http://purl.org/dc/terms/title -->

    <owl:AnnotationProperty rdf:about="http://purl.org/dc/terms/title"/>
    


    <!-- 
    ///////////////////////////////////////////////////////////////////////////////////////
    //
    // Object Properties
    //
    ///////////////////////////////////////////////////////////////////////////////////////
     -->

    


    <!-- https://w3id.org/hacid/onto/data/specifiesVariableSpecializationFor -->

    <owl:ObjectProperty rdf:about="https://w3id.org/hacid/onto/data/specifiesVariableSpecializationFor">
        <rdfs:subPropertyOf rdf:resource="https://w3id.org/hacid/onto/top-level/associatedWith"/>
        <owl:inverseOf rdf:resource="https://w3id.org/hacid/onto/data/isSpecializedAccordingTo"/>
        <rdfs:domain rdf:resource="https://w3id.org/hacid/onto/data/VariableSpecialization"/>
        <rdfs:range rdf:resource="https://w3id.org/hacid/onto/data/Variable"/>
        <rdfs:comment xml:lang="en">Associates a variable specialization specification with a variable for which it is used.</rdfs:comment>
        <rdfs:label xml:lang="en">specifies variable specialization for</rdfs:label>
    </owl:ObjectProperty>
    


    <!-- https://w3id.org/hacid/onto/data/aggregatesVariable -->

    <owl:ObjectProperty rdf:about="https://w3id.org/hacid/onto/data/aggregatesVariable">
        <rdfs:subPropertyOf rdf:resource="https://w3id.org/hacid/onto/top-level/associatedWith"/>
        <owl:inverseOf rdf:resource="https://w3id.org/hacid/onto/data/isVariableAggregatedBy"/>
        <rdfs:domain rdf:resource="https://w3id.org/hacid/onto/data/Aggregation"/>
        <rdfs:range rdf:resource="https://w3id.org/hacid/onto/data/Variable"/>
        <rdfs:comment xml:lang="en">Associates an aggregation specification with each variable whose values will be grouped by the aggregation.</rdfs:comment>
        <rdfs:isDefinedBy rdf:resource="https://w3id.org/hacid/onto/data"/>
        <rdfs:label xml:lang="en">aggregates variable</rdfs:label>
    </owl:ObjectProperty>
    


    <!-- https://w3id.org/hacid/onto/data/basedOnDimensionalSpace -->

    <owl:ObjectProperty rdf:about="https://w3id.org/hacid/onto/data/basedOnDimensionalSpace">
        <rdfs:subPropertyOf rdf:resource="https://w3id.org/hacid/onto/data/isSpecializationOfVariable"/>
        <owl:inverseOf rdf:resource="https://w3id.org/hacid/onto/data/isBasisOfDimensionalSpace"/>
        <rdfs:domain rdf:resource="https://w3id.org/hacid/onto/data/DimensionalSpace"/>
        <rdfs:range rdf:resource="https://w3id.org/hacid/onto/data/DimensionalSpace"/>
        <rdfs:comment xml:lang="en">Associates a dimensional space to another dimensional space it is based on, e.g., by structuring or specializing it.</rdfs:comment>
        <rdfs:isDefinedBy rdf:resource="https://w3id.org/hacid/onto/data"/>
        <rdfs:label xml:lang="en">based on dimensional space</rdfs:label>
    </owl:ObjectProperty>
    


    <!-- https://w3id.org/hacid/onto/data/definesAggregation -->

    <owl:ObjectProperty rdf:about="https://w3id.org/hacid/onto/data/definesAggregation">
        <rdfs:subPropertyOf rdf:resource="https://w3id.org/hacid/onto/top-level/associatedWith"/>
        <owl:inverseOf rdf:resource="https://w3id.org/hacid/onto/data/isAggregationDefinedFor"/>
        <rdfs:domain rdf:resource="https://w3id.org/hacid/onto/data/DependentVariable"/>
        <rdfs:range rdf:resource="https://w3id.org/hacid/onto/data/Aggregation"/>
        <rdfs:comment xml:lang="en">Associates a dependent variable with an aggregation specification, when the value of such variable is obtained performing one or more aggregations. The aggregation specification is in turn associated with the variables whose values will be grouped by the aggregation and optionally with a set of suggested quantizations used for such groupings.</rdfs:comment>
        <rdfs:isDefinedBy rdf:resource="https://w3id.org/hacid/onto/data"/>
        <rdfs:label xml:lang="en">defines aggregation</rdfs:label>
    </owl:ObjectProperty>
    


    <!-- https://w3id.org/hacid/onto/data/dependsOnVariable -->

    <owl:ObjectProperty rdf:about="https://w3id.org/hacid/onto/data/dependsOnVariable">
        <rdfs:subPropertyOf rdf:resource="https://w3id.org/hacid/onto/top-level/associatedWith"/>
        <owl:inverseOf rdf:resource="https://w3id.org/hacid/onto/data/hasDependentOnVariable"/>
        <rdfs:domain rdf:resource="https://w3id.org/hacid/onto/data/DependentVariable"/>
        <rdfs:range rdf:resource="https://w3id.org/hacid/onto/data/Variable"/>
        <rdfs:comment xml:lang="en">Associates a dependent variable with a variable it depends on.</rdfs:comment>
        <rdfs:isDefinedBy rdf:resource="https://w3id.org/hacid/onto/data"/>
        <rdfs:label xml:lang="en">depends on variable</rdfs:label>
    </owl:ObjectProperty>
    


    <!-- https://w3id.org/hacid/onto/data/derivedFromVariable -->

    <owl:ObjectProperty rdf:about="https://w3id.org/hacid/onto/data/derivedFromVariable">
        <rdfs:subPropertyOf rdf:resource="https://w3id.org/hacid/onto/top-level/associatedWith"/>
        <owl:inverseOf rdf:resource="https://w3id.org/hacid/onto/data/hasVariableDerivedFrom"/>
        <rdfs:domain rdf:resource="https://w3id.org/hacid/onto/data/DerivedVariable"/>
        <rdfs:range rdf:resource="https://w3id.org/hacid/onto/data/Variable"/>
        <rdfs:comment xml:lang="en">Associates a derived variable with a variable from which is derived.</rdfs:comment>
        <rdfs:isDefinedBy rdf:resource="https://w3id.org/hacid/onto/data"/>
        <rdfs:label xml:lang="en">derived from variable</rdfs:label>
    </owl:ObjectProperty>
    


    <!-- https://w3id.org/hacid/onto/data/hasAvailableDataFormat -->

    <owl:ObjectProperty rdf:about="https://w3id.org/hacid/onto/data/hasAvailableDataFormat">
        <rdfs:subPropertyOf rdf:resource="https://w3id.org/hacid/onto/top-level/associatedWith"/>
        <owl:inverseOf rdf:resource="https://w3id.org/hacid/onto/data/isAvailableDataFormatOf"/>
        <rdfs:domain rdf:resource="https://w3id.org/hacid/onto/data/DataSource"/>
        <rdfs:range rdf:resource="https://w3id.org/hacid/onto/data/DataFormat"/>
        <rdfs:comment xml:lang="en">Associates a data source with a data format in which the data is available.</rdfs:comment>
        <rdfs:isDefinedBy rdf:resource="https://w3id.org/hacid/onto/data"/>
        <rdfs:label xml:lang="en">has available data format</rdfs:label>
    </owl:ObjectProperty>
    


    <!-- https://w3id.org/hacid/onto/data/hasBoundingRegion -->

    <owl:ObjectProperty rdf:about="https://w3id.org/hacid/onto/data/hasBoundingRegion">
        <rdfs:subPropertyOf rdf:resource="https://w3id.org/hacid/onto/top-level/associatedWith"/>
        <owl:inverseOf rdf:resource="https://w3id.org/hacid/onto/data/isBoundingRegionOf"/>
        <rdfs:domain rdf:resource="https://w3id.org/hacid/onto/data/DimensionalSpace"/>
        <rdfs:range rdf:resource="https://w3id.org/hacid/onto/data/Region"/>
        <rdfs:comment xml:lang="en">Associates a dimensional space with a region (possibly defined on a more generic dimensional space) which bounds the dimensional space: i,e., such that the dimensional space is contained in the region.</rdfs:comment>
        <rdfs:isDefinedBy rdf:resource="https://w3id.org/hacid/onto/data"/>
        <rdfs:label xml:lang="en">has bounding region</rdfs:label>
    </owl:ObjectProperty>
    


    <!-- https://w3id.org/hacid/onto/data/hasComponentVariable -->

    <owl:ObjectProperty rdf:about="https://w3id.org/hacid/onto/data/hasComponentVariable">
        <rdfs:subPropertyOf rdf:resource="https://w3id.org/hacid/onto/data/holdsSpecializationOfVariable"/>
        <owl:inverseOf rdf:resource="https://w3id.org/hacid/onto/data/isComponentVariableOf"/>
        <rdfs:domain rdf:resource="https://w3id.org/hacid/onto/data/Variable"/>
        <rdfs:range rdf:resource="https://w3id.org/hacid/onto/data/DerivedVariable"/>
        <rdfs:comment xml:lang="en">Associates a variable with a variable that is a part of the former as component (e.g., a variable with geodetic coordinates has the component variables corrisponding to latitute and longitude).</rdfs:comment>
        <rdfs:isDefinedBy rdf:resource="https://w3id.org/hacid/onto/data"/>
        <rdfs:label xml:lang="en">has component variable</rdfs:label>
    </owl:ObjectProperty>
    


    <!-- https://w3id.org/hacid/onto/data/hasDataSerialization -->

    <owl:ObjectProperty rdf:about="https://w3id.org/hacid/onto/data/hasDataSerialization">
        <rdfs:subPropertyOf rdf:resource="https://w3id.org/hacid/onto/top-level/associatedWith"/>
        <owl:inverseOf rdf:resource="https://w3id.org/hacid/onto/data/isDataSerializationOf"/>
        <rdfs:domain rdf:resource="https://w3id.org/hacid/onto/data/FiniteVariable"/>
        <rdfs:range rdf:resource="https://w3id.org/hacid/onto/data/DataSource"/>
        <rdfs:comment xml:lang="en">Associates a finite variable, i.e., a dataset, with a data source that offers one or more serializations of such dataset.</rdfs:comment>
        <rdfs:isDefinedBy rdf:resource="https://w3id.org/hacid/onto/data"/>
        <rdfs:label xml:lang="en">has data serialization</rdfs:label>
    </owl:ObjectProperty>
    


    <!-- https://w3id.org/hacid/onto/data/hasDependentOnVariable -->

    <owl:ObjectProperty rdf:about="https://w3id.org/hacid/onto/data/hasDependentOnVariable">
        <rdfs:subPropertyOf rdf:resource="https://w3id.org/hacid/onto/top-level/associatedWith"/>
        <rdfs:domain rdf:resource="https://w3id.org/hacid/onto/data/Variable"/>
        <rdfs:range rdf:resource="https://w3id.org/hacid/onto/data/DependentVariable"/>
        <rdfs:comment xml:lang="en">Associates a variable with a dependent variable that depends on the former.</rdfs:comment>
        <rdfs:isDefinedBy rdf:resource="https://w3id.org/hacid/onto/data"/>
        <rdfs:label xml:lang="en">has dependent-on variable</rdfs:label>
    </owl:ObjectProperty>
    


    <!-- https://w3id.org/hacid/onto/data/hasDiscretization -->

    <owl:ObjectProperty rdf:about="https://w3id.org/hacid/onto/data/hasDiscretization">
        <rdfs:subPropertyOf rdf:resource="https://w3id.org/hacid/onto/top-level/associatedWith"/>
        <owl:inverseOf rdf:resource="https://w3id.org/hacid/onto/data/isDiscretizationFor"/>
        <rdfs:domain rdf:resource="https://w3id.org/hacid/onto/data/DiscreteDimensionalSpace"/>
        <rdfs:range rdf:resource="https://w3id.org/hacid/onto/data/Quantization"/>
        <rdfs:comment xml:lang="en">Associates a discrete dimensional space (based on a continuum) with the quantization adopted for discretization.</rdfs:comment>
        <rdfs:isDefinedBy rdf:resource="https://w3id.org/hacid/onto/data"/>
        <rdfs:label xml:lang="en">has discretization</rdfs:label>
    </owl:ObjectProperty>
    


    <!-- https://w3id.org/hacid/onto/data/hasExactBoundingRegion -->

    <owl:ObjectProperty rdf:about="https://w3id.org/hacid/onto/data/hasExactBoundingRegion">
        <rdfs:subPropertyOf rdf:resource="https://w3id.org/hacid/onto/data/hasBoundingRegion"/>
        <owl:inverseOf rdf:resource="https://w3id.org/hacid/onto/data/isExactBoundingRegionOf"/>
        <rdfs:domain rdf:resource="https://w3id.org/hacid/onto/data/DimensionalSpace"/>
        <rdfs:range rdf:resource="https://w3id.org/hacid/onto/data/Region"/>
        <rdfs:comment xml:lang="en">Associates a dimensional space with a region (possibly defined on a more generic dimensional space) which bounds exactly the dimensional space: i,e., the extension of the dimensional space matches with the region.</rdfs:comment>
        <rdfs:isDefinedBy rdf:resource="https://w3id.org/hacid/onto/data"/>
        <rdfs:label xml:lang="en">has exact bounding region</rdfs:label>
    </owl:ObjectProperty>
    


    <!-- https://w3id.org/hacid/onto/data/hasPeriod -->

    <owl:ObjectProperty rdf:about="https://w3id.org/hacid/onto/data/hasPeriod">
        <rdfs:subPropertyOf rdf:resource="https://w3id.org/hacid/onto/top-level/associatedWith"/>
        <owl:inverseOf rdf:resource="https://w3id.org/hacid/onto/data/isPeriodOf"/>
        <rdfs:domain rdf:resource="https://w3id.org/hacid/onto/data/PeriodicRegularGrid"/>
        <rdfs:comment xml:lang="en">Associates a periodic regular grid with its period (to associate direclty a literal use data:hasPeriodValue).</rdfs:comment>
        <rdfs:isDefinedBy rdf:resource="https://w3id.org/hacid/onto/data"/>
        <rdfs:label xml:lang="en">has period</rdfs:label>
    </owl:ObjectProperty>
    


    <!-- https://w3id.org/hacid/onto/data/hasPoint -->

    <owl:ObjectProperty rdf:about="https://w3id.org/hacid/onto/data/hasPoint">
        <rdfs:subPropertyOf rdf:resource="https://w3id.org/hacid/onto/top-level/associatedWith"/>
        <owl:inverseOf rdf:resource="https://w3id.org/hacid/onto/data/isPointOf"/>
        <rdfs:domain rdf:resource="https://w3id.org/hacid/onto/data/DimensionalSpace"/>
        <rdfs:range rdf:resource="https://w3id.org/hacid/onto/data/Point"/>
        <rdfs:comment xml:lang="en">Associates a dimensional space with a point of that dimensional space, i.e. any point that is contained and representable in that dimensional space (use data:hasPointValue to directly associate a literal).</rdfs:comment>
        <rdfs:isDefinedBy rdf:resource="https://w3id.org/hacid/onto/data"/>
        <rdfs:label xml:lang="en">has point</rdfs:label>
    </owl:ObjectProperty>
    


    <!-- https://w3id.org/hacid/onto/data/hasReferencePoint -->

    <owl:ObjectProperty rdf:about="https://w3id.org/hacid/onto/data/hasReferencePoint">
        <rdfs:subPropertyOf rdf:resource="https://w3id.org/hacid/onto/top-level/associatedWith"/>
        <owl:inverseOf rdf:resource="https://w3id.org/hacid/onto/data/isReferencePointOf"/>
        <rdfs:domain rdf:resource="https://w3id.org/hacid/onto/data/DimensionalSpace"/>
        <rdfs:range rdf:resource="https://w3id.org/hacid/onto/data/Point"/>
        <rdfs:comment xml:lang="en">Associates a dimensional space with a point that is used as reference to identify the points of the dimensional space (e.g., the North Pole for geodetic coordinates on Earth).</rdfs:comment>
        <rdfs:isDefinedBy rdf:resource="https://w3id.org/hacid/onto/data"/>
        <rdfs:label xml:lang="en">has reference point</rdfs:label>
    </owl:ObjectProperty>
    


    <!-- https://w3id.org/hacid/onto/data/hasRegion -->

    <owl:ObjectProperty rdf:about="https://w3id.org/hacid/onto/data/hasRegion">
        <rdfs:subPropertyOf rdf:resource="https://w3id.org/hacid/onto/top-level/associatedWith"/>
        <owl:inverseOf rdf:resource="https://w3id.org/hacid/onto/data/isRegionOf"/>
        <rdfs:domain rdf:resource="https://w3id.org/hacid/onto/data/DimensionalSpace"/>
        <rdfs:range rdf:resource="https://w3id.org/hacid/onto/data/Region"/>
        <rdfs:comment xml:lang="en">Associates a dimensional space with a region of that dimensional space, i.e. any region that is contained and representable in that dimensional space (use data:hasRegionValue to directly associate a literal).</rdfs:comment>
        <rdfs:isDefinedBy rdf:resource="https://w3id.org/hacid/onto/data"/>
        <rdfs:label xml:lang="en">has region</rdfs:label>
    </owl:ObjectProperty>
    


    <!-- https://w3id.org/hacid/onto/data/hasResolution -->

    <owl:ObjectProperty rdf:about="https://w3id.org/hacid/onto/data/hasResolution">
        <rdfs:subPropertyOf rdf:resource="https://w3id.org/hacid/onto/top-level/associatedWith"/>
        <owl:inverseOf rdf:resource="https://w3id.org/hacid/onto/data/isResolutionOf"/>
        <rdfs:domain rdf:resource="https://w3id.org/hacid/onto/data/Quantization"/>
        <rdfs:comment xml:lang="en">Associates a quantization with its resolution (to associate directly a literal use data:hasResolutionValue).</rdfs:comment>
        <rdfs:isDefinedBy rdf:resource="https://w3id.org/hacid/onto/data"/>
        <rdfs:label xml:lang="en">has resolution</rdfs:label>
    </owl:ObjectProperty>
    


    <!-- https://w3id.org/hacid/onto/data/hasSelectedRegion -->

    <owl:ObjectProperty rdf:about="https://w3id.org/hacid/onto/data/hasSelectedRegion">
        <rdfs:subPropertyOf rdf:resource="https://w3id.org/hacid/onto/top-level/associatedWith"/>
        <owl:inverseOf rdf:resource="https://w3id.org/hacid/onto/data/isSelectedRegionOf"/>
        <rdfs:domain rdf:resource="https://w3id.org/hacid/onto/data/VariableSpecialization"/>
        <rdfs:range rdf:resource="https://w3id.org/hacid/onto/data/Region"/>
        <rdfs:comment xml:lang="en">Associates a variable specialization with the region used to constrain the variable.</rdfs:comment>
        <rdfs:isDefinedBy rdf:resource="https://w3id.org/hacid/onto/data"/>
        <rdfs:label xml:lang="en">has selected region</rdfs:label>
    </owl:ObjectProperty>
    


    <!-- https://w3id.org/hacid/onto/data/hasSubDimensionalSpace -->

    <owl:ObjectProperty rdf:about="https://w3id.org/hacid/onto/data/hasSubDimensionalSpace">
        <rdfs:subPropertyOf rdf:resource="https://w3id.org/hacid/onto/data/hasComponentVariable"/>
        <owl:inverseOf rdf:resource="https://w3id.org/hacid/onto/data/isSubDimensionalSpaceOf"/>
        <rdfs:domain rdf:resource="https://w3id.org/hacid/onto/data/DimensionalSpace"/>
        <rdfs:range rdf:resource="https://w3id.org/hacid/onto/data/DimensionalSpace"/>
        <rdfs:comment xml:lang="en">Associates a dimensional space with another dimensional space that is a projection of the first one, by selecting  specific components (e.g., time is a subdimensional space of spacetime).</rdfs:comment>
        <rdfs:isDefinedBy rdf:resource="https://w3id.org/hacid/onto/data"/>
        <rdfs:label xml:lang="en">has sub dimensional space</rdfs:label>
    </owl:ObjectProperty>
    


    <!-- https://w3id.org/hacid/onto/data/hasSuggestedQuantization -->

    <owl:ObjectProperty rdf:about="https://w3id.org/hacid/onto/data/hasSuggestedQuantization">
        <rdfs:subPropertyOf rdf:resource="https://w3id.org/hacid/onto/top-level/associatedWith"/>
        <owl:inverseOf rdf:resource="https://w3id.org/hacid/onto/data/isSuggestedQuantizationFor"/>
        <rdfs:domain rdf:resource="https://w3id.org/hacid/onto/data/Aggregation"/>
        <rdfs:range rdf:resource="https://w3id.org/hacid/onto/data/Quantization"/>
        <rdfs:comment xml:lang="en">Associates an aggregation specification with a quantization which is suggested for that aggregation.</rdfs:comment>
        <rdfs:isDefinedBy rdf:resource="https://w3id.org/hacid/onto/data"/>
        <rdfs:label xml:lang="en">has suggested quantization</rdfs:label>
    </owl:ObjectProperty>
    


    <!-- https://w3id.org/hacid/onto/data/hasValuesOn -->

    <owl:ObjectProperty rdf:about="https://w3id.org/hacid/onto/data/hasValuesOn">
        <rdfs:subPropertyOf rdf:resource="https://w3id.org/hacid/onto/top-level/associatedWith"/>
        <owl:inverseOf rdf:resource="https://w3id.org/hacid/onto/data/providesValuesFor"/>
        <rdfs:domain rdf:resource="https://w3id.org/hacid/onto/data/Variable"/>
        <rdfs:range rdf:resource="https://w3id.org/hacid/onto/data/DimensionalSpace"/>
        <rdfs:comment xml:lang="en">Associates a variable with the dimensional space on which the variable is defined, i.e. possibile values for the variable are points in that dimensional space.</rdfs:comment>
        <rdfs:isDefinedBy rdf:resource="https://w3id.org/hacid/onto/data"/>
        <rdfs:label xml:lang="en">has values on</rdfs:label>
    </owl:ObjectProperty>
    


    <!-- https://w3id.org/hacid/onto/data/hasVariableDerivedFrom -->

    <owl:ObjectProperty rdf:about="https://w3id.org/hacid/onto/data/hasVariableDerivedFrom">
        <rdfs:subPropertyOf rdf:resource="https://w3id.org/hacid/onto/top-level/associatedWith"/>
        <rdfs:domain rdf:resource="https://w3id.org/hacid/onto/data/Variable"/>
        <rdfs:range rdf:resource="https://w3id.org/hacid/onto/data/DerivedVariable"/>
        <rdfs:comment xml:lang="en">Associates a variable with a variable that has been derived from it.</rdfs:comment>
        <rdfs:isDefinedBy rdf:resource="https://w3id.org/hacid/onto/data"/>
        <rdfs:label xml:lang="en">has derived-from variable</rdfs:label>
    </owl:ObjectProperty>
    


    <!-- https://w3id.org/hacid/onto/data/hasVariableSpecialization -->

    <owl:ObjectProperty rdf:about="https://w3id.org/hacid/onto/data/hasVariableSpecialization">
        <rdfs:subPropertyOf rdf:resource="https://w3id.org/hacid/onto/data/hasVariableSpecializationAsComponentOf"/>
        <owl:inverseOf rdf:resource="https://w3id.org/hacid/onto/data/isSpecializationOfVariable"/>
        <rdfs:domain rdf:resource="https://w3id.org/hacid/onto/data/Variable"/>
        <rdfs:range rdf:resource="https://w3id.org/hacid/onto/data/DerivedVariable"/>
        <rdfs:comment xml:lang="en">Associates a variable with a variable that is a specialization of the first variable (e.g., the atmospheric temperature on the sea surface is a specialization of the atmospheric temperature).</rdfs:comment>
        <rdfs:isDefinedBy rdf:resource="https://w3id.org/hacid/onto/data"/>
        <rdfs:label xml:lang="en">has variable specialization</rdfs:label>
    </owl:ObjectProperty>
    


    <!-- https://w3id.org/hacid/onto/data/hasVariableSpecializationAsComponentOf -->

    <owl:ObjectProperty rdf:about="https://w3id.org/hacid/onto/data/hasVariableSpecializationAsComponentOf">
        <rdfs:subPropertyOf rdf:resource="https://w3id.org/hacid/onto/data/hasVariableDerivedFrom"/>
        <owl:inverseOf rdf:resource="https://w3id.org/hacid/onto/data/holdsSpecializationOfVariable"/>
        <rdfs:domain rdf:resource="https://w3id.org/hacid/onto/data/Variable"/>
        <rdfs:range rdf:resource="https://w3id.org/hacid/onto/data/DerivedVariable"/>
        <rdfs:comment xml:lang="en">Associates a variable with a variable that contains as component a specialization of the first variable.</rdfs:comment>
        <rdfs:isDefinedBy rdf:resource="https://w3id.org/hacid/onto/data"/>
        <rdfs:label xml:lang="en">has variable specialization as component of</rdfs:label>
    </owl:ObjectProperty>
    


    <!-- https://w3id.org/hacid/onto/data/holdsSpecializationOfVariable -->

    <owl:ObjectProperty rdf:about="https://w3id.org/hacid/onto/data/holdsSpecializationOfVariable">
        <rdfs:subPropertyOf rdf:resource="https://w3id.org/hacid/onto/data/derivedFromVariable"/>
        <rdfs:domain rdf:resource="https://w3id.org/hacid/onto/data/DerivedVariable"/>
        <rdfs:range rdf:resource="https://w3id.org/hacid/onto/data/Variable"/>
        <rdfs:comment xml:lang="en">Associates a variable with a variable for which the former contains, as component, a specialization of.</rdfs:comment>
        <rdfs:isDefinedBy rdf:resource="https://w3id.org/hacid/onto/data"/>
        <rdfs:label xml:lang="en">holds specialization of variable</rdfs:label>
    </owl:ObjectProperty>
    


    <!-- https://w3id.org/hacid/onto/data/isAggregationDefinedFor -->

    <owl:ObjectProperty rdf:about="https://w3id.org/hacid/onto/data/isAggregationDefinedFor">
        <rdfs:subPropertyOf rdf:resource="https://w3id.org/hacid/onto/top-level/associatedWith"/>
        <rdfs:domain rdf:resource="https://w3id.org/hacid/onto/data/Aggregation"/>
        <rdfs:range rdf:resource="https://w3id.org/hacid/onto/data/DependentVariable"/>
        <rdfs:comment xml:lang="en">Associates an aggregation specification with a dependent variable, when the value of such variable is obtained performing that specified aggregation.</rdfs:comment>
        <rdfs:isDefinedBy rdf:resource="https://w3id.org/hacid/onto/data"/>
        <rdfs:label xml:lang="en">is aggregation defined for</rdfs:label>
    </owl:ObjectProperty>
    


    <!-- https://w3id.org/hacid/onto/data/isAvailableDataFormatOf -->

    <owl:ObjectProperty rdf:about="https://w3id.org/hacid/onto/data/isAvailableDataFormatOf">
        <rdfs:subPropertyOf rdf:resource="https://w3id.org/hacid/onto/top-level/associatedWith"/>
        <rdfs:domain rdf:resource="https://w3id.org/hacid/onto/data/DataFormat"/>
        <rdfs:range rdf:resource="https://w3id.org/hacid/onto/data/DataSource"/>
        <rdfs:comment xml:lang="en">Associates a data format with a data source that offers that format.</rdfs:comment>
        <rdfs:isDefinedBy rdf:resource="https://w3id.org/hacid/onto/data"/>
        <rdfs:label xml:lang="en">is available data format of</rdfs:label>
    </owl:ObjectProperty>
    


    <!-- https://w3id.org/hacid/onto/data/isBasisOfDimensionalSpace -->

    <owl:ObjectProperty rdf:about="https://w3id.org/hacid/onto/data/isBasisOfDimensionalSpace">
        <rdfs:subPropertyOf rdf:resource="https://w3id.org/hacid/onto/data/hasVariableSpecialization"/>
        <rdfs:domain rdf:resource="https://w3id.org/hacid/onto/data/DimensionalSpace"/>
        <rdfs:range rdf:resource="https://w3id.org/hacid/onto/data/DimensionalSpace"/>
        <rdfs:comment xml:lang="en">Associates a dimensional space to another dimensional space that is based on the former one, e.g., by structuring or specializing it.</rdfs:comment>
        <rdfs:isDefinedBy rdf:resource="https://w3id.org/hacid/onto/data"/>
        <rdfs:label xml:lang="en">is basis of dimensional space</rdfs:label>
    </owl:ObjectProperty>
    


    <!-- https://w3id.org/hacid/onto/data/isBoundingRegionOf -->

    <owl:ObjectProperty rdf:about="https://w3id.org/hacid/onto/data/isBoundingRegionOf">
        <rdfs:subPropertyOf rdf:resource="https://w3id.org/hacid/onto/top-level/associatedWith"/>
        <rdfs:domain rdf:resource="https://w3id.org/hacid/onto/data/Region"/>
        <rdfs:range rdf:resource="https://w3id.org/hacid/onto/data/DimensionalSpace"/>
        <rdfs:comment xml:lang="en">Associates a region with a dimensional space (possibly more specific that the one on which the region is defined) which is bounded by the region: i,e., such that the dimensional space is contained in the region.</rdfs:comment>
        <rdfs:isDefinedBy rdf:resource="https://w3id.org/hacid/onto/data"/>
        <rdfs:label xml:lang="en">is bounding region of</rdfs:label>
    </owl:ObjectProperty>
    


    <!-- https://w3id.org/hacid/onto/data/isComponentVariableOf -->

    <owl:ObjectProperty rdf:about="https://w3id.org/hacid/onto/data/isComponentVariableOf">
        <rdfs:subPropertyOf rdf:resource="https://w3id.org/hacid/onto/data/hasVariableSpecializationAsComponentOf"/>
        <rdfs:domain rdf:resource="https://w3id.org/hacid/onto/data/DerivedVariable"/>
        <rdfs:range rdf:resource="https://w3id.org/hacid/onto/data/Variable"/>
        <rdfs:comment xml:lang="en">Associates a variable with a variable of which the former is a component (e.g., a variable with geodetic coordinates has the component variables corrisponding to latitute and longitude).</rdfs:comment>
        <rdfs:isDefinedBy rdf:resource="https://w3id.org/hacid/onto/data"/>
        <rdfs:label xml:lang="en">is component variable of</rdfs:label>
    </owl:ObjectProperty>
    


    <!-- https://w3id.org/hacid/onto/data/isConstrainedVariableIn -->

    <owl:ObjectProperty rdf:about="https://w3id.org/hacid/onto/data/isConstrainedVariableIn">
        <rdfs:subPropertyOf rdf:resource="https://w3id.org/hacid/onto/top-level/associatedWith"/>
        <owl:inverseOf rdf:resource="https://w3id.org/hacid/onto/data/isSpecializationOn"/>
        <rdfs:domain rdf:resource="https://w3id.org/hacid/onto/data/IndependentVariable"/>
        <rdfs:range rdf:resource="https://w3id.org/hacid/onto/data/VariableSpecialization"/>
        <rdfs:comment xml:lang="en">Associates an independent variable with a variable specialization specification in which that variable is constrained.</rdfs:comment>
        <rdfs:isDefinedBy rdf:resource="https://w3id.org/hacid/onto/data"/>
        <rdfs:label xml:lang="en">is constrained variable in</rdfs:label>
    </owl:ObjectProperty>
    


    <!-- https://w3id.org/hacid/onto/data/isDataSerializationOf -->

    <owl:ObjectProperty rdf:about="https://w3id.org/hacid/onto/data/isDataSerializationOf">
        <rdfs:subPropertyOf rdf:resource="https://w3id.org/hacid/onto/top-level/associatedWith"/>
        <rdfs:domain rdf:resource="https://w3id.org/hacid/onto/data/DataSource"/>
        <rdfs:range rdf:resource="https://w3id.org/hacid/onto/data/FiniteVariable"/>
        <rdfs:comment xml:lang="en">Associates a data source with the finite variable, i.e., the dataset, that is serialized by that source.</rdfs:comment>
        <rdfs:isDefinedBy rdf:resource="https://w3id.org/hacid/onto/data"/>
        <rdfs:label xml:lang="en">is data serialization of</rdfs:label>
    </owl:ObjectProperty>
    


    <!-- https://w3id.org/hacid/onto/data/isDiscretizationFor -->

    <owl:ObjectProperty rdf:about="https://w3id.org/hacid/onto/data/isDiscretizationFor">
        <rdfs:subPropertyOf rdf:resource="https://w3id.org/hacid/onto/top-level/associatedWith"/>
        <rdfs:domain rdf:resource="https://w3id.org/hacid/onto/data/Quantization"/>
        <rdfs:range rdf:resource="https://w3id.org/hacid/onto/data/DiscreteDimensionalSpace"/>
        <rdfs:comment xml:lang="en">Associates a quantization with a discrete dimensional space (based on a continuum) that has been discretized by such quantization.</rdfs:comment>
        <rdfs:isDefinedBy rdf:resource="https://w3id.org/hacid/onto/data"/>
        <rdfs:label xml:lang="en">is discretization for</rdfs:label>
    </owl:ObjectProperty>
    


    <!-- https://w3id.org/hacid/onto/data/isExactBoundingRegionOf -->

    <owl:ObjectProperty rdf:about="https://w3id.org/hacid/onto/data/isExactBoundingRegionOf">
        <rdfs:subPropertyOf rdf:resource="https://w3id.org/hacid/onto/data/isBoundingRegionOf"/>
        <rdfs:domain rdf:resource="https://w3id.org/hacid/onto/data/Region"/>
        <rdfs:range rdf:resource="https://w3id.org/hacid/onto/data/DimensionalSpace"/>
        <rdfs:comment xml:lang="en">Associates a region with a dimensional space (possibly more specific that the one on which the region is defined) which is exactly bounded by the region: i,e., such that the extension of the dimensional space matches with the region.</rdfs:comment>
        <rdfs:isDefinedBy rdf:resource="https://w3id.org/hacid/onto/data"/>
        <rdfs:label xml:lang="en">is exact bounding region of</rdfs:label>
    </owl:ObjectProperty>
    


    <!-- https://w3id.org/hacid/onto/data/isPeriodOf -->

    <owl:ObjectProperty rdf:about="https://w3id.org/hacid/onto/data/isPeriodOf">
        <rdfs:subPropertyOf rdf:resource="https://w3id.org/hacid/onto/top-level/associatedWith"/>
        <rdfs:range rdf:resource="https://w3id.org/hacid/onto/data/PeriodicRegularGrid"/>
        <rdfs:comment xml:lang="en">Associates a resource with a periodic regular grid of which the resource is the period.</rdfs:comment>
        <rdfs:isDefinedBy rdf:resource="https://w3id.org/hacid/onto/data"/>
        <rdfs:label xml:lang="en">is period of</rdfs:label>
    </owl:ObjectProperty>
    


    <!-- https://w3id.org/hacid/onto/data/isPointOf -->

    <owl:ObjectProperty rdf:about="https://w3id.org/hacid/onto/data/isPointOf">
        <rdfs:subPropertyOf rdf:resource="https://w3id.org/hacid/onto/top-level/associatedWith"/>
        <rdfs:domain rdf:resource="https://w3id.org/hacid/onto/data/Point"/>
        <rdfs:range rdf:resource="https://w3id.org/hacid/onto/data/DimensionalSpace"/>
        <rdfs:comment xml:lang="en">Associates a point with a dimensional space it is part of (any dimensional space that contains and is able to represent that point).</rdfs:comment>
        <rdfs:isDefinedBy rdf:resource="https://w3id.org/hacid/onto/data"/>
        <rdfs:label xml:lang="en">is point of</rdfs:label>
    </owl:ObjectProperty>
    


    <!-- https://w3id.org/hacid/onto/data/isReferencePointOf -->

    <owl:ObjectProperty rdf:about="https://w3id.org/hacid/onto/data/isReferencePointOf">
        <rdfs:subPropertyOf rdf:resource="https://w3id.org/hacid/onto/top-level/associatedWith"/>
        <rdfs:domain rdf:resource="https://w3id.org/hacid/onto/data/Point"/>
        <rdfs:range rdf:resource="https://w3id.org/hacid/onto/data/DimensionalSpace"/>
        <rdfs:comment xml:lang="en">Associates a point with a dimensional space for which that point is used as reference to identify the points of the dimensional space (e.g., the North Pole for geodetic coordinates on Earth).</rdfs:comment>
        <rdfs:isDefinedBy rdf:resource="https://w3id.org/hacid/onto/data"/>
        <rdfs:label xml:lang="en">is reference point of</rdfs:label>
    </owl:ObjectProperty>
    


    <!-- https://w3id.org/hacid/onto/data/isRegionOf -->

    <owl:ObjectProperty rdf:about="https://w3id.org/hacid/onto/data/isRegionOf">
        <rdfs:subPropertyOf rdf:resource="https://w3id.org/hacid/onto/top-level/associatedWith"/>
        <rdfs:domain rdf:resource="https://w3id.org/hacid/onto/data/Region"/>
        <rdfs:range rdf:resource="https://w3id.org/hacid/onto/data/DimensionalSpace"/>
        <rdfs:comment xml:lang="en">Associates a region with a dimensional space it is part of (any dimensional space that contains and is able to represent that region).</rdfs:comment>
        <rdfs:isDefinedBy rdf:resource="https://w3id.org/hacid/onto/data"/>
        <rdfs:label xml:lang="en">is region of</rdfs:label>
    </owl:ObjectProperty>
    


    <!-- https://w3id.org/hacid/onto/data/isResolutionOf -->

    <owl:ObjectProperty rdf:about="https://w3id.org/hacid/onto/data/isResolutionOf">
        <rdfs:subPropertyOf rdf:resource="https://w3id.org/hacid/onto/top-level/associatedWith"/>
        <rdfs:range rdf:resource="https://w3id.org/hacid/onto/data/Quantization"/>
        <rdfs:comment xml:lang="en">Associates a resource with a quantization of which the resource is the resolution.</rdfs:comment>
        <rdfs:isDefinedBy rdf:resource="https://w3id.org/hacid/onto/data"/>
        <rdfs:label xml:lang="en">is resolution of</rdfs:label>
    </owl:ObjectProperty>
    


    <!-- https://w3id.org/hacid/onto/data/isSelectedRegionOf -->

    <owl:ObjectProperty rdf:about="https://w3id.org/hacid/onto/data/isSelectedRegionOf">
        <rdfs:subPropertyOf rdf:resource="https://w3id.org/hacid/onto/top-level/associatedWith"/>
        <rdfs:domain rdf:resource="https://w3id.org/hacid/onto/data/Region"/>
        <rdfs:range rdf:resource="https://w3id.org/hacid/onto/data/VariableSpecialization"/>
        <rdfs:comment xml:lang="en">Associates a region with a variable specialization in which that region is used to constrain the variable.</rdfs:comment>
        <rdfs:isDefinedBy rdf:resource="https://w3id.org/hacid/onto/data"/>
        <rdfs:label xml:lang="en">is selected region of</rdfs:label>
    </owl:ObjectProperty>
    


    <!-- https://w3id.org/hacid/onto/data/isSpecializationOfVariable -->

    <owl:ObjectProperty rdf:about="https://w3id.org/hacid/onto/data/isSpecializationOfVariable">
        <rdfs:subPropertyOf rdf:resource="https://w3id.org/hacid/onto/data/holdsSpecializationOfVariable"/>
        <rdfs:domain rdf:resource="https://w3id.org/hacid/onto/data/DerivedVariable"/>
        <rdfs:range rdf:resource="https://w3id.org/hacid/onto/data/Variable"/>
        <owl:propertyChainAxiom rdf:parseType="Collection">
            <rdf:Description rdf:about="https://w3id.org/hacid/onto/data/isSpecializedAccordingTo"/>
            <rdf:Description rdf:about="https://w3id.org/hacid/onto/data/isSpecializationOn"/>
        </owl:propertyChainAxiom>
        <rdfs:comment xml:lang="en">Associates a variable with a variable of which the former is a specialization of.</rdfs:comment>
        <rdfs:isDefinedBy rdf:resource="https://w3id.org/hacid/onto/data"/>
        <rdfs:label xml:lang="en">is specialization of variable</rdfs:label>
    </owl:ObjectProperty>
    


    <!-- https://w3id.org/hacid/onto/data/isSpecializationOn -->

    <owl:ObjectProperty rdf:about="https://w3id.org/hacid/onto/data/isSpecializationOn">
        <rdfs:subPropertyOf rdf:resource="https://w3id.org/hacid/onto/top-level/associatedWith"/>
        <rdfs:domain rdf:resource="https://w3id.org/hacid/onto/data/VariableSpecialization"/>
        <rdfs:range rdf:resource="https://w3id.org/hacid/onto/data/IndependentVariable"/>
        <rdfs:comment xml:lang="en">Associates a variable specialization specification with the independent variable that is constrained.</rdfs:comment>
        <rdfs:isDefinedBy rdf:resource="https://w3id.org/hacid/onto/data"/>
        <rdfs:label xml:lang="en">is specialization on</rdfs:label>
    </owl:ObjectProperty>
    


    <!-- https://w3id.org/hacid/onto/data/isSpecializedAccordingTo -->

    <owl:ObjectProperty rdf:about="https://w3id.org/hacid/onto/data/isSpecializedAccordingTo">
        <rdfs:subPropertyOf rdf:resource="https://w3id.org/hacid/onto/top-level/associatedWith"/>
        <rdfs:domain rdf:resource="https://w3id.org/hacid/onto/data/Variable"/>
        <rdfs:range rdf:resource="https://w3id.org/hacid/onto/data/VariableSpecialization"/>
        <rdfs:comment xml:lang="en">Associates a variable with the specification of how it is specialized from a more generic variable.</rdfs:comment>
        <rdfs:isDefinedBy rdf:resource="https://w3id.org/hacid/onto/data"/>
        <rdfs:label xml:lang="en">is specialized according to</rdfs:label>
    </owl:ObjectProperty>
    


    <!-- https://w3id.org/hacid/onto/data/isSubDimensionalSpaceOf -->

    <owl:ObjectProperty rdf:about="https://w3id.org/hacid/onto/data/isSubDimensionalSpaceOf">
        <rdfs:subPropertyOf rdf:resource="https://w3id.org/hacid/onto/data/isComponentVariableOf"/>
        <rdfs:domain rdf:resource="https://w3id.org/hacid/onto/data/DimensionalSpace"/>
        <rdfs:range rdf:resource="https://w3id.org/hacid/onto/data/DimensionalSpace"/>
        <rdfs:comment xml:lang="en">Associates a dimensional space with another dimensional space of which the first one is a projection, by selecting  specific components (e.g., time is a subdimensional space of spacetime).</rdfs:comment>
        <rdfs:isDefinedBy rdf:resource="https://w3id.org/hacid/onto/data"/>
        <rdfs:label xml:lang="en">is sub dimensional space of</rdfs:label>
    </owl:ObjectProperty>
    


    <!-- https://w3id.org/hacid/onto/data/isSuggestedQuantizationFor -->

    <owl:ObjectProperty rdf:about="https://w3id.org/hacid/onto/data/isSuggestedQuantizationFor">
        <rdfs:subPropertyOf rdf:resource="https://w3id.org/hacid/onto/top-level/associatedWith"/>
        <rdfs:domain rdf:resource="https://w3id.org/hacid/onto/data/Quantization"/>
        <rdfs:range rdf:resource="https://w3id.org/hacid/onto/data/Aggregation"/>
        <rdfs:comment xml:lang="en">Associates a quantization with an aggregation specification for which that aggregation is suggested.</rdfs:comment>
        <rdfs:isDefinedBy rdf:resource="https://w3id.org/hacid/onto/data"/>
        <rdfs:label xml:lang="en">is suggested quantization for</rdfs:label>
    </owl:ObjectProperty>
    


    <!-- https://w3id.org/hacid/onto/data/isVariableAggregatedBy -->

    <owl:ObjectProperty rdf:about="https://w3id.org/hacid/onto/data/isVariableAggregatedBy">
        <rdfs:subPropertyOf rdf:resource="https://w3id.org/hacid/onto/top-level/associatedWith"/>
        <rdfs:domain rdf:resource="https://w3id.org/hacid/onto/data/Variable"/>
        <rdfs:range rdf:resource="https://w3id.org/hacid/onto/data/Aggregation"/>
        <rdfs:comment xml:lang="en">Associates a variable to an aggregation specification for which its values are grouped.</rdfs:comment>
        <rdfs:isDefinedBy rdf:resource="https://w3id.org/hacid/onto/data"/>
        <rdfs:label xml:lang="en">is variable aggregated by</rdfs:label>
    </owl:ObjectProperty>
    


    <!-- https://w3id.org/hacid/onto/data/providesValuesFor -->

    <owl:ObjectProperty rdf:about="https://w3id.org/hacid/onto/data/providesValuesFor">
        <rdfs:subPropertyOf rdf:resource="https://w3id.org/hacid/onto/top-level/associatedWith"/>
        <rdfs:domain rdf:resource="https://w3id.org/hacid/onto/data/DimensionalSpace"/>
        <rdfs:range rdf:resource="https://w3id.org/hacid/onto/data/Variable"/>
        <rdfs:comment xml:lang="en">Associates a dimensional space with a variable defined on it, i.e. possibile values for the variable are points in that dimensional space.</rdfs:comment>
        <rdfs:isDefinedBy rdf:resource="https://w3id.org/hacid/onto/data"/>
        <rdfs:label xml:lang="en">provides values for</rdfs:label>
    </owl:ObjectProperty>
    


    <!-- https://w3id.org/hacid/onto/top-level/associatedWith -->

    <owl:ObjectProperty rdf:about="https://w3id.org/hacid/onto/top-level/associatedWith"/>
    


    <!-- https://w3id.org/hacid/onto/top-level/hasPart -->

    <owl:ObjectProperty rdf:about="https://w3id.org/hacid/onto/top-level/hasPart"/>
    


    <!-- 
    ///////////////////////////////////////////////////////////////////////////////////////
    //
    // Data properties
    //
    ///////////////////////////////////////////////////////////////////////////////////////
     -->

    


    <!-- https://w3id.org/hacid/onto/data/hasPeriodValue -->

    <owl:DatatypeProperty rdf:about="https://w3id.org/hacid/onto/data/hasPeriodValue">
        <rdfs:subPropertyOf rdf:resource="http://www.w3.org/2002/07/owl#topDataProperty"/>
        <rdfs:domain rdf:resource="https://w3id.org/hacid/onto/data/PeriodicRegularGrid"/>
        <rdfs:comment xml:lang="en">Associates a periodic regular grid with its period (to associate a non-literal resource use data:hasPeriod).</rdfs:comment>
        <rdfs:isDefinedBy rdf:resource="https://w3id.org/hacid/onto/data"/>
        <rdfs:label xml:lang="en">has period value</rdfs:label>
    </owl:DatatypeProperty>
    


    <!-- https://w3id.org/hacid/onto/data/hasPointValue -->

    <owl:DatatypeProperty rdf:about="https://w3id.org/hacid/onto/data/hasPointValue">
        <rdfs:domain rdf:resource="https://w3id.org/hacid/onto/data/DimensionalSpace"/>
        <rdfs:comment xml:lang="en">Associates a dimensional space with a point of that dimensional space, i.e. any point that is contained and representable in that dimensional space, directly expressed as literal (use data:hasPoint to associate a non-literal resource).</rdfs:comment>
        <rdfs:isDefinedBy rdf:resource="https://w3id.org/hacid/onto/data"/>
        <rdfs:label xml:lang="en">has point value</rdfs:label>
    </owl:DatatypeProperty>
    


    <!-- https://w3id.org/hacid/onto/data/hasRegionValue -->

    <owl:DatatypeProperty rdf:about="https://w3id.org/hacid/onto/data/hasRegionValue">
        <rdfs:domain rdf:resource="https://w3id.org/hacid/onto/data/DimensionalSpace"/>
        <rdfs:comment xml:lang="en">Associates a dimensional space with a region of that dimensional space, i.e. any region that is contained and representable in that dimensional space, directly expressed as literal (use data:hasRegion to associate a non-literal resource).</rdfs:comment>
        <rdfs:isDefinedBy rdf:resource="https://w3id.org/hacid/onto/data"/>
        <rdfs:label xml:lang="en">has region value</rdfs:label>
    </owl:DatatypeProperty>
    


    <!-- https://w3id.org/hacid/onto/data/hasResolutionValue -->

    <owl:DatatypeProperty rdf:about="https://w3id.org/hacid/onto/data/hasResolutionValue">
        <rdfs:domain rdf:resource="https://w3id.org/hacid/onto/data/Quantization"/>
        <rdfs:comment xml:lang="en">Associates a quantization with its resolution (to associate a non-literal resource use data:hasResolution).</rdfs:comment>
        <rdfs:isDefinedBy rdf:resource="https://w3id.org/hacid/onto/data"/>
        <rdfs:label xml:lang="en">has resolution value</rdfs:label>
    </owl:DatatypeProperty>
    


    <!-- https://w3id.org/hacid/onto/data/hasURL -->

    <owl:DatatypeProperty rdf:about="https://w3id.org/hacid/onto/data/hasURL">
        <rdfs:domain rdf:resource="https://w3id.org/hacid/onto/data/DataSource"/>
        <rdfs:range rdf:resource="http://www.w3.org/2001/XMLSchema#anyURI"/>
        <rdfs:isDefinedBy rdf:resource="https://w3id.org/hacid/onto/data"/>
        <rdfs:label xml:lang="en">has URL</rdfs:label>
    </owl:DatatypeProperty>
    


    <!-- 
    ///////////////////////////////////////////////////////////////////////////////////////
    //
    // Classes
    //
    ///////////////////////////////////////////////////////////////////////////////////////
     -->

    


    <!-- http://www.opengis.net/ont/geosparql#Geometry -->

    <owl:Class rdf:about="http://www.opengis.net/ont/geosparql#Geometry"/>
    


    <!-- https://w3id.org/hacid/onto/data/GeodeticPoint -->

    <owl:Class rdf:about="https://w3id.org/hacid/onto/data/GeodeticPoint">
        <rdfs:subClassOf rdf:resource="http://www.opengis.net/ont/geosparql#Geometry"/>
        <rdfs:subClassOf rdf:resource="https://w3id.org/hacid/onto/data/Point"/>
        <rdfs:comment xml:lang="en">A point in a geodetic dimensional space, i.e. a georaphic location of the Earth surface.</rdfs:comment>
        <rdfs:label xml:lang="en">Geodetic Point</rdfs:label>
    </owl:Class>
    


    <!-- https://w3id.org/hacid/onto/data/Instant -->

    <owl:Class rdf:about="https://w3id.org/hacid/onto/data/Instant">
        <rdfs:subClassOf rdf:resource="https://w3id.org/hacid/onto/data/Point"/>
        <rdfs:comment xml:lang="en">An instant in time, i.e. a point in a temporal dimensional space.</rdfs:comment>
        <rdfs:label xml:lang="en">Instant</rdfs:label>
    </owl:Class>
    


    <!-- https://w3id.org/hacid/onto/data/Aggregation -->

    <owl:Class rdf:about="https://w3id.org/hacid/onto/data/Aggregation">
        <rdfs:subClassOf rdf:resource="https://w3id.org/hacid/onto/top-level/Concept"/>
        <rdfs:comment xml:lang="en">An aggregation of a dependent variable over a variable it depends on. While the actual application of the aggregation depends on a grouping (more in general a quantization) over the independent variable, the aggregation is agnostic to the chosen quantization. It represents just that an aggregation function is to be applied along that dimension.</rdfs:comment>
        <rdfs:isDefinedBy rdf:resource="https://w3id.org/hacid/onto/data"/>
        <rdfs:label xml:lang="en">Aggregation</rdfs:label>
    </owl:Class>
    


    <!-- https://w3id.org/hacid/onto/data/BoundedDimensionalSpace -->

    <owl:Class rdf:about="https://w3id.org/hacid/onto/data/BoundedDimensionalSpace">
        <rdfs:subClassOf rdf:resource="https://w3id.org/hacid/onto/data/DimensionalSpace"/>
        <rdfs:comment xml:lang="en">A dimensional space that has finite boundaries (does not extend indefinitely), although not necessarily discrete and so still holding possibly infinite values (e.g., a finite interval of time).</rdfs:comment>
        <rdfs:isDefinedBy rdf:resource="https://w3id.org/hacid/onto/data"/>
        <rdfs:label xml:lang="en">Bounded Dimensional Space</rdfs:label>
    </owl:Class>
    


    <!-- https://w3id.org/hacid/onto/data/ConstantDimensionalSpace -->

    <owl:Class rdf:about="https://w3id.org/hacid/onto/data/ConstantDimensionalSpace">
        <rdfs:subClassOf rdf:resource="https://w3id.org/hacid/onto/data/DiscreteDimensionalSpace"/>
        <rdfs:comment xml:lang="en">A degenerate dimensional space consisting of a single value.</rdfs:comment>
        <rdfs:isDefinedBy rdf:resource="https://w3id.org/hacid/onto/data"/>
        <rdfs:label xml:lang="en">Constant Dimensional Space</rdfs:label>
    </owl:Class>
    


    <!-- https://w3id.org/hacid/onto/data/Continuum -->

    <owl:Class rdf:about="https://w3id.org/hacid/onto/data/Continuum">
        <rdfs:subClassOf rdf:resource="https://w3id.org/hacid/onto/data/DimensionalSpace"/>
        <owl:disjointWith rdf:resource="https://w3id.org/hacid/onto/data/DiscreteDimensionalSpace"/>
        <rdfs:comment xml:lang="en">A continuous dimensional space.</rdfs:comment>
        <rdfs:isDefinedBy rdf:resource="https://w3id.org/hacid/onto/data"/>
        <rdfs:label xml:lang="en">Continuum</rdfs:label>
    </owl:Class>
    


    <!-- https://w3id.org/hacid/onto/data/DataFormat -->

    <owl:Class rdf:about="https://w3id.org/hacid/onto/data/DataFormat">
        <rdfs:subClassOf rdf:resource="https://w3id.org/hacid/onto/top-level/Concept"/>
        <rdfs:comment xml:lang="en">A data format that can be used to serialize a dataset (e.g., CSV). Usage of controlled vocabularies is suggested.</rdfs:comment>
        <rdfs:isDefinedBy rdf:resource="https://w3id.org/hacid/onto/data"/>
        <rdfs:label xml:lang="en">Data Format</rdfs:label>
    </owl:Class>
    


    <!-- https://w3id.org/hacid/onto/data/DataSource -->

    <owl:Class rdf:about="https://w3id.org/hacid/onto/data/DataSource">
        <rdfs:subClassOf rdf:resource="https://w3id.org/hacid/onto/top-level/InformationEntity"/>
        <rdfs:comment xml:lang="en">A data source is a location (in a broader sense, but typically an URL or a path in a specific file system) which contains somehow a dataset, alongside with the technical specification of how to access it. The hosted dataset should be available in one or more data formats.</rdfs:comment>
        <rdfs:isDefinedBy rdf:resource="https://w3id.org/hacid/onto/data"/>
        <rdfs:label xml:lang="en">Data Source</rdfs:label>
    </owl:Class>
    


    <!-- https://w3id.org/hacid/onto/data/Dataset -->

    <owl:Class rdf:about="https://w3id.org/hacid/onto/data/Dataset">
        <owl:equivalentClass rdf:resource="https://w3id.org/hacid/onto/data/FiniteVariable"/>
        <rdfs:subClassOf rdf:resource="https://w3id.org/hacid/onto/data/Variable"/>
        <rdfs:comment xml:lang="en">A dataset is a variable (which can be composed of multiple sub-variables) whose extension is finitely expressable, i.e. a finite variable. This is an alias of data:FiniteVariable to be used when this alternative phrasing fits to the context  better.</rdfs:comment>
        <rdfs:isDefinedBy rdf:resource="https://w3id.org/hacid/onto/data"/>
        <rdfs:label xml:lang="en">Dataset</rdfs:label>
    </owl:Class>
    


    <!-- https://w3id.org/hacid/onto/data/DependentVariable -->

    <owl:Class rdf:about="https://w3id.org/hacid/onto/data/DependentVariable">
        <rdfs:subClassOf rdf:resource="https://w3id.org/hacid/onto/data/Variable"/>
        <owl:disjointWith rdf:resource="https://w3id.org/hacid/onto/data/IndependentVariable"/>
        <rdfs:comment xml:lang="en">A variable that is depedent on one or more (independent) variables in the given context of use.</rdfs:comment>
        <rdfs:isDefinedBy rdf:resource="https://w3id.org/hacid/onto/data"/>
        <rdfs:label xml:lang="en">Dependent Variable</rdfs:label>
    </owl:Class>
    


    <!-- https://w3id.org/hacid/onto/data/DerivedVariable -->

    <owl:Class rdf:about="https://w3id.org/hacid/onto/data/DerivedVariable">
        <rdfs:subClassOf rdf:resource="https://w3id.org/hacid/onto/data/Variable"/>
        <rdfs:comment xml:lang="en">A variable that has been derived mathematically from one or more variables</rdfs:comment>
        <rdfs:isDefinedBy rdf:resource="https://w3id.org/hacid/onto/data"/>
        <rdfs:label xml:lang="en">Derived Variable</rdfs:label>
    </owl:Class>
    


    <!-- https://w3id.org/hacid/onto/data/DimensionalSpace -->

    <owl:Class rdf:about="https://w3id.org/hacid/onto/data/DimensionalSpace">
        <rdfs:subClassOf rdf:resource="https://w3id.org/hacid/onto/data/IndependentVariable"/>
        <rdfs:subClassOf>
            <owl:Restriction>
                <owl:onProperty rdf:resource="https://w3id.org/hacid/onto/data/hasValuesOn"/>
                <owl:hasSelf rdf:datatype="http://www.w3.org/2001/XMLSchema#boolean">true</owl:hasSelf>
            </owl:Restriction>
        </rdfs:subClassOf>
        <rdfs:comment xml:lang="en">A dimension that can be somehow quantified, possibly structured by a system of measurement/classification. It can be bounded (e.g., a period of time) or not (e.g., the "whole" time), discrete (e.g, time by days) or continuous (e.g., a time continuum). It is a special case of an independent variable, specifically the most generic variable defined on the dimensional space. This enables a simple representation when the context of use does not require the distinction between variable and dimensional space.</rdfs:comment>
        <rdfs:isDefinedBy rdf:resource="https://w3id.org/hacid/onto/data"/>
        <rdfs:label xml:lang="en">Dimensional Space</rdfs:label>
    </owl:Class>
    


    <!-- https://w3id.org/hacid/onto/data/DiscreteDimensionalSpace -->

    <owl:Class rdf:about="https://w3id.org/hacid/onto/data/DiscreteDimensionalSpace">
        <rdfs:subClassOf rdf:resource="https://w3id.org/hacid/onto/data/DimensionalSpace"/>
        <rdfs:comment xml:lang="en">A dimensional space composed of discrete values. It could be inherently discrete (e.g., the set of international recognized countries) or obtained discretizing a continuous dimensional space (e.g., by sampling or partitioning). It can still have infinite (but countable) values if it is not bounded (e.g., the time sampled by hours, streching indefinetely in one or both directions).</rdfs:comment>
        <rdfs:isDefinedBy rdf:resource="https://w3id.org/hacid/onto/data"/>
        <rdfs:label xml:lang="en">Discrete Dimensional Space</rdfs:label>
    </owl:Class>
    


    <!-- https://w3id.org/hacid/onto/data/FiniteDimensionalSpace -->

    <owl:Class rdf:about="https://w3id.org/hacid/onto/data/FiniteDimensionalSpace">
        <owl:equivalentClass>
            <owl:Class>
                <owl:intersectionOf rdf:parseType="Collection">
                    <rdf:Description rdf:about="https://w3id.org/hacid/onto/data/BoundedDimensionalSpace"/>
                    <rdf:Description rdf:about="https://w3id.org/hacid/onto/data/DiscreteDimensionalSpace"/>
                </owl:intersectionOf>
            </owl:Class>
        </owl:equivalentClass>
        <rdfs:subClassOf rdf:resource="https://w3id.org/hacid/onto/data/BoundedDimensionalSpace"/>
        <rdfs:subClassOf rdf:resource="https://w3id.org/hacid/onto/data/DiscreteDimensionalSpace"/>
        <rdfs:subClassOf rdf:resource="https://w3id.org/hacid/onto/data/FiniteVariable"/>
        <rdfs:comment xml:lang="en">A finite dimensional space, i.e. a dimensional space that is both discrete and bounded.</rdfs:comment>
        <rdfs:isDefinedBy rdf:resource="https://w3id.org/hacid/onto/data"/>
        <rdfs:label xml:lang="en">Finite Dimensional Space</rdfs:label>
    </owl:Class>
    


    <!-- https://w3id.org/hacid/onto/data/FiniteVariable -->

    <owl:Class rdf:about="https://w3id.org/hacid/onto/data/FiniteVariable">
        <rdfs:subClassOf rdf:resource="https://w3id.org/hacid/onto/data/Variable"/>
        <rdfs:subClassOf>
            <owl:Restriction>
                <owl:onProperty rdf:resource="https://w3id.org/hacid/onto/top-level/hasPart"/>
                <owl:allValuesFrom rdf:resource="https://w3id.org/hacid/onto/data/FiniteVariable"/>
            </owl:Restriction>
        </rdfs:subClassOf>
        <rdfs:comment xml:lang="en">A finite variable, i.e. a variable whose set of possible values is finite. For an independent variable, it means the corresponding dimensional space is finite. For a depedent variable, it means the independent variables it depends on are finite.</rdfs:comment>
        <rdfs:isDefinedBy rdf:resource="https://w3id.org/hacid/onto/data"/>
        <rdfs:label xml:lang="en">Finite Variable</rdfs:label>
    </owl:Class>
    


    <!-- https://w3id.org/hacid/onto/data/GeodeticPoint -->

    <owl:Class rdf:about="https://w3id.org/hacid/onto/data/GeodeticPoint">
        <rdfs:isDefinedBy rdf:resource="https://w3id.org/hacid/onto/data"/>
    </owl:Class>
    


    <!-- https://w3id.org/hacid/onto/data/GeodeticRegion -->

    <owl:Class rdf:about="https://w3id.org/hacid/onto/data/GeodeticRegion">
        <rdfs:subClassOf rdf:resource="http://www.opengis.net/ont/geosparql#Geometry"/>
        <rdfs:subClassOf rdf:resource="https://w3id.org/hacid/onto/data/Region"/>
        <rdfs:comment xml:lang="en">A region in a geodetic dimensional space, i.e. a georaphic area of the Earth surface (e.g., the area of a country).</rdfs:comment>
        <rdfs:isDefinedBy rdf:resource="https://w3id.org/hacid/onto/data"/>
        <rdfs:label xml:lang="en">Geodetic Region</rdfs:label>
    </owl:Class>
    


    <!-- https://w3id.org/hacid/onto/data/IndependentVariable -->

    <owl:Class rdf:about="https://w3id.org/hacid/onto/data/IndependentVariable">
        <rdfs:subClassOf rdf:resource="https://w3id.org/hacid/onto/data/Variable"/>
        <rdfs:comment xml:lang="en">A variable that is indepedent (not dependent from other variables) in the given context of use.</rdfs:comment>
        <rdfs:isDefinedBy rdf:resource="https://w3id.org/hacid/onto/data"/>
        <rdfs:label xml:lang="en">Independent Variable</rdfs:label>
    </owl:Class>
    


    <!-- https://w3id.org/hacid/onto/data/IntervalSampling -->

    <owl:Class rdf:about="https://w3id.org/hacid/onto/data/IntervalSampling">
        <rdfs:isDefinedBy rdf:resource="https://w3id.org/hacid/onto/data"/>
    </owl:Class>
    


    <!-- https://w3id.org/hacid/onto/data/Partitioning -->

    <owl:Class rdf:about="https://w3id.org/hacid/onto/data/Partitioning">
        <rdfs:subClassOf rdf:resource="https://w3id.org/hacid/onto/data/Quantization"/>
        <rdfs:isDefinedBy rdf:resource="https://w3id.org/hacid/onto/data"/>
        <rdfs:label xml:lang="en">Partitioning</rdfs:label>
    </owl:Class>
    


    <!-- https://w3id.org/hacid/onto/data/PeriodicRegularGrid -->

    <owl:Class rdf:about="https://w3id.org/hacid/onto/data/PeriodicRegularGrid">
        <rdfs:subClassOf rdf:resource="https://w3id.org/hacid/onto/data/RegularGrid"/>
        <rdfs:isDefinedBy rdf:resource="https://w3id.org/hacid/onto/data"/>
        <rdfs:label xml:lang="en">Periodic Regular Partitioning</rdfs:label>
    </owl:Class>
    


    <!-- https://w3id.org/hacid/onto/data/Point -->

    <owl:Class rdf:about="https://w3id.org/hacid/onto/data/Point">
        <rdfs:subClassOf rdf:resource="https://w3id.org/hacid/onto/top-level/Entity"/>
        <rdfs:isDefinedBy rdf:resource="https://w3id.org/hacid/onto/data"/>
        <rdfs:label xml:lang="en">Point</rdfs:label>
    </owl:Class>
    


    <!-- https://w3id.org/hacid/onto/data/Quantization -->

    <owl:Class rdf:about="https://w3id.org/hacid/onto/data/Quantization">
        <rdfs:subClassOf rdf:resource="https://w3id.org/hacid/onto/data/DiscreteDimensionalSpace"/>
        <rdfs:isDefinedBy rdf:resource="https://w3id.org/hacid/onto/data"/>
        <rdfs:label xml:lang="en">Quantization</rdfs:label>
    </owl:Class>
    


    <!-- https://w3id.org/hacid/onto/data/Region -->

    <owl:Class rdf:about="https://w3id.org/hacid/onto/data/Region">
        <rdfs:subClassOf rdf:resource="https://w3id.org/hacid/onto/top-level/Region"/>
        <rdfs:isDefinedBy rdf:resource="https://w3id.org/hacid/onto/data"/>
        <rdfs:label xml:lang="en">Region</rdfs:label>
    </owl:Class>
    


    <!-- https://w3id.org/hacid/onto/data/RegularGrid -->

    <owl:Class rdf:about="https://w3id.org/hacid/onto/data/RegularGrid">
        <rdfs:subClassOf rdf:resource="https://w3id.org/hacid/onto/data/Partitioning"/>
        <rdfs:isDefinedBy rdf:resource="https://w3id.org/hacid/onto/data"/>
        <rdfs:label xml:lang="en">Regular Partitioning</rdfs:label>
    </owl:Class>
    


    <!-- https://w3id.org/hacid/onto/data/RollingRegularGrid -->

    <owl:Class rdf:about="https://w3id.org/hacid/onto/data/RollingRegularGrid">
        <rdfs:subClassOf rdf:resource="https://w3id.org/hacid/onto/data/RegularGrid"/>
        <rdfs:isDefinedBy rdf:resource="https://w3id.org/hacid/onto/data"/>
        <rdfs:label xml:lang="en">RollingRegularGrid</rdfs:label>
    </owl:Class>
    


    <!-- https://w3id.org/hacid/onto/data/Sampling -->

    <owl:Class rdf:about="https://w3id.org/hacid/onto/data/Sampling">
        <rdfs:subClassOf rdf:resource="https://w3id.org/hacid/onto/data/Quantization"/>
        <rdfs:isDefinedBy rdf:resource="https://w3id.org/hacid/onto/data"/>
        <rdfs:label xml:lang="en">Sampling</rdfs:label>
    </owl:Class>
    


    <!-- https://w3id.org/hacid/onto/data/SingleRegionPartitioning -->

    <owl:Class rdf:about="https://w3id.org/hacid/onto/data/SingleRegionPartitioning">
        <rdfs:subClassOf rdf:resource="https://w3id.org/hacid/onto/data/ConstantDimensionalSpace"/>
        <rdfs:subClassOf rdf:resource="https://w3id.org/hacid/onto/data/Partitioning"/>
        <rdfs:comment xml:lang="en">A degenerate partitioning of a dimensional space, such that it is composed of one single region encompassin the whole dimensional space.</rdfs:comment>
        <rdfs:isDefinedBy rdf:resource="https://w3id.org/hacid/onto/data"/>
        <rdfs:label xml:lang="en">Single-Region Partitioning</rdfs:label>
    </owl:Class>
    


    <!-- https://w3id.org/hacid/onto/data/TemporalRegion -->

    <owl:Class rdf:about="https://w3id.org/hacid/onto/data/TemporalRegion">
        <rdfs:subClassOf rdf:resource="https://w3id.org/hacid/onto/data/Region"/>
        <rdfs:comment xml:lang="en">A region in time.</rdfs:comment>
        <rdfs:isDefinedBy rdf:resource="https://w3id.org/hacid/onto/data"/>
        <rdfs:label xml:lang="en">Temporal region</rdfs:label>
    </owl:Class>
    


    <!-- https://w3id.org/hacid/onto/data/Variable -->

    <owl:Class rdf:about="https://w3id.org/hacid/onto/data/Variable">
        <rdfs:subClassOf rdf:resource="https://w3id.org/hacid/onto/top-level/Concept"/>
        <rdfs:subClassOf>
            <owl:Restriction>
                <owl:onProperty rdf:resource="https://w3id.org/hacid/onto/top-level/hasPart"/>
                <owl:allValuesFrom rdf:resource="https://w3id.org/hacid/onto/data/Variable"/>
            </owl:Restriction>
        </rdfs:subClassOf>
        <rdfs:comment xml:lang="en">A variable is an abstraction that has meaning in the context of some relation between different variables and can be associated to different values in a set that is usually well defined. The set of possible values is represented by a data:DimensionalSpace; the two are linked via the data:hasValuesOn property.</rdfs:comment>
        <rdfs:isDefinedBy rdf:resource="https://w3id.org/hacid/onto/data"/>
        <rdfs:label xml:lang="en">Variable</rdfs:label>
    </owl:Class>
    


    <!-- https://w3id.org/hacid/onto/data/VariableSpecialization -->

    <owl:Class rdf:about="https://w3id.org/hacid/onto/data/VariableSpecialization">
        <rdfs:subClassOf rdf:resource="https://w3id.org/hacid/onto/top-level/Concept"/>
        <rdfs:comment xml:lang="en">The specialization of a dependent variable by choosing a specific region for the values of one or more of the inependent variables it depends on.</rdfs:comment>
        <rdfs:isDefinedBy rdf:resource="https://w3id.org/hacid/onto/data"/>
        <rdfs:label xml:lang="en">Variable Specialization</rdfs:label>
    </owl:Class>
    


    <!-- https://w3id.org/hacid/onto/top-level/Concept -->

    <owl:Class rdf:about="https://w3id.org/hacid/onto/top-level/Concept"/>
    


    <!-- https://w3id.org/hacid/onto/top-level/Entity -->

    <owl:Class rdf:about="https://w3id.org/hacid/onto/top-level/Entity"/>
    


    <!-- https://w3id.org/hacid/onto/top-level/InformationEntity -->

    <owl:Class rdf:about="https://w3id.org/hacid/onto/top-level/InformationEntity"/>
    


    <!-- https://w3id.org/hacid/onto/top-level/Region -->

    <owl:Class rdf:about="https://w3id.org/hacid/onto/top-level/Region"/>
</rdf:RDF><!-- Generated by the OWL API (version 4.5.29) https://github.com/owlcs/owlapi -->
