<?xml version="1.0"?>
<rdf:RDF xmlns="https://w3id.org/hacid/onto/cs/"
     xml:base="https://w3id.org/hacid/onto/cs/"
     xmlns:owl="http://www.w3.org/2002/07/owl#"
     xmlns:rdf="http://www.w3.org/1999/02/22-rdf-syntax-ns#"
     xmlns:xml="http://www.w3.org/XML/1998/namespace"
     xmlns:xsd="http://www.w3.org/2001/XMLSchema#"
     xmlns:core="https://w3id.org/arco/ontology/core/"
     xmlns:rdfs="http://www.w3.org/2000/01/rdf-schema#">
    <owl:Ontology rdf:about="https://w3id.org/hacid/onto/cs/">
        <rdfs:comment xml:lang="en">This ontology describes the process of handling a request for climate information.</rdfs:comment>
        <rdfs:label xml:lang="en">Climate Science Process Workflow</rdfs:label>
    </owl:Ontology>
    


    <!-- 
    ///////////////////////////////////////////////////////////////////////////////////////
    //
    // Object Properties
    //
    ///////////////////////////////////////////////////////////////////////////////////////
     -->

    


    <!-- https://w3id.org/arco/ontology/core/definesRole -->

    <owl:ObjectProperty rdf:about="https://w3id.org/arco/ontology/core/definesRole">
        <owl:inverseOf rdf:resource="https://w3id.org/arco/ontology/core/isRoleDefinedIn"/>
        <rdfs:domain rdf:resource="https://w3id.org/hacid/onto/cs/ClimateProcessWorkflow"/>
        <rdfs:comment xml:lang="en">A relation between a description and a role, e.g. the recipe for a cake defines the role &apos;ingredient&apos;</rdfs:comment>
        <rdfs:isDefinedBy rdf:resource="https://w3id.org/hacid/onto/top-level/"/>
        <rdfs:label xml:lang="en">defines role</rdfs:label>
    </owl:ObjectProperty>
    


    <!-- https://w3id.org/arco/ontology/core/definesTask -->

    <owl:ObjectProperty rdf:about="https://w3id.org/arco/ontology/core/definesTask">
        <owl:inverseOf rdf:resource="https://w3id.org/arco/ontology/core/isTaskDefinedIn"/>
        <rdfs:domain rdf:resource="https://w3id.org/hacid/onto/cs/ClimateProcessWorkflow"/>
        <rdfs:range rdf:resource="https://w3id.org/arco/ontology/core/ClimateProcessTask"/>
        <rdfs:comment xml:lang="en">A relation between a description and a task, e.g. the recipe for a cake defines the task &apos;boil&apos;.</rdfs:comment>
        <rdfs:isDefinedBy rdf:resource="https://w3id.org/hacid/onto/top-level/"/>
        <rdfs:label xml:lang="en">defines task</rdfs:label>
    </owl:ObjectProperty>
    


    <!-- https://w3id.org/arco/ontology/core/directlyFollows -->

    <owl:ObjectProperty rdf:about="https://w3id.org/arco/ontology/core/directlyFollows">
        <rdfs:subPropertyOf rdf:resource="https://w3id.org/hacid/onto/top-level/follows"/>
        <owl:inverseOf rdf:resource="https://w3id.org/arco/ontology/core/directlyPrecedes"/>
        <rdfs:domain rdf:resource="https://w3id.org/hacid/onto/top-level/Task"/>
        <rdfs:range rdf:resource="https://w3id.org/hacid/onto/top-level/Task"/>
        <rdfs:isDefinedBy rdf:resource="https://w3id.org/hacid/onto/top-level/"/>
        <rdfs:label xml:lang="en">directly follows</rdfs:label>
    </owl:ObjectProperty>
    


    <!-- https://w3id.org/arco/ontology/core/directlyPrecedes -->

    <owl:ObjectProperty rdf:about="https://w3id.org/arco/ontology/core/directlyPrecedes">
        <rdfs:subPropertyOf rdf:resource="https://w3id.org/hacid/onto/top-level/precedes"/>
        <rdfs:isDefinedBy rdf:resource="https://w3id.org/hacid/onto/top-level/"/>
        <rdfs:label xml:lang="en">directly precedes</rdfs:label>
    </owl:ObjectProperty>
    


    <!-- https://w3id.org/arco/ontology/core/hasPart -->

    <owl:ObjectProperty rdf:about="https://w3id.org/arco/ontology/core/hasPart">
        <owl:inverseOf rdf:resource="https://w3id.org/arco/ontology/core/isPartOf"/>
        <rdf:type rdf:resource="http://www.w3.org/2002/07/owl#TransitiveProperty"/>
        <rdf:type rdf:resource="http://www.w3.org/2002/07/owl#ReflexiveProperty"/>
        <rdfs:domain rdf:resource="https://w3id.org/arco/ontology/core/ClimateProcessTask"/>
        <rdfs:range rdf:resource="https://w3id.org/arco/ontology/core/ClimateProcessTask"/>
        <rdfs:comment xml:lang="en">A schematic relation between any entities, e.g. &apos;the human body has a brain as part&apos;, &apos;20th century contains year 1923&apos;, &apos;World War II includes the Pearl Harbour event&apos;.

Parthood should assume the basic properties of mereology: transitivity, antisymmetry, and reflexivity (propert Parthood of course misses reflexivity). 
However, antisymmetry is not supported in OWL2 explicitly, therefore DUL has to adopt one of two patterns:
1) dropping asymmetry axioms, while granting reflexivity: this means that symmetry is not enforced, but permitted for the case of reflexivity. Of course, in this way we cannot prevent symmetric usages of hasPart;
2) dropping the reflexivity axiom, and enforce asymmetry: in this case, we would prevent all symmetric usages, but we loose the possibility of enforcing reflexivity, which is commonsensical in parthood.
In DUL, we adopt pattern #1 for partOf, and pattern #2 for properPartOf, which seems a good approximation: due to the lack of inheritance of property characteristics, each asymmetric hasPropertPart assertion would also be a reflexive hasPart assertion (reflexive reduction design pattern).

Subproperties and restrictions can be used to specialize hasPart for objects, events, etc.</rdfs:comment>
        <rdfs:isDefinedBy rdf:resource="https://w3id.org/hacid/onto/top-level/"/>
        <rdfs:label xml:lang="en">has part</rdfs:label>
    </owl:ObjectProperty>
    


    <!-- https://w3id.org/arco/ontology/core/hasTask -->

    <owl:ObjectProperty rdf:about="https://w3id.org/arco/ontology/core/hasTask">
        <owl:inverseOf rdf:resource="https://w3id.org/arco/ontology/core/isTaskOf"/>
        <rdfs:comment xml:lang="en">A relation between roles and tasks, e.g. &apos;students have the duty of giving exams&apos; (i.e. the Role &apos;student&apos; hasTask the Task &apos;giving exams&apos;).</rdfs:comment>
        <rdfs:isDefinedBy rdf:resource="https://w3id.org/hacid/onto/top-level/"/>
        <rdfs:label xml:lang="en">has task</rdfs:label>
    </owl:ObjectProperty>
    


    <!-- https://w3id.org/arco/ontology/core/isPartOf -->

    <owl:ObjectProperty rdf:about="https://w3id.org/arco/ontology/core/isPartOf">
        <rdf:type rdf:resource="http://www.w3.org/2002/07/owl#TransitiveProperty"/>
        <rdf:type rdf:resource="http://www.w3.org/2002/07/owl#ReflexiveProperty"/>
        <rdfs:comment xml:lang="en">A relation between any entities, e.g. &apos;brain is a part of the human body&apos;. See dul:hasPart for additional documentation.</rdfs:comment>
        <rdfs:isDefinedBy rdf:resource="https://w3id.org/hacid/onto/top-level/"/>
        <rdfs:label xml:lang="en">is part of</rdfs:label>
    </owl:ObjectProperty>
    


    <!-- https://w3id.org/arco/ontology/core/isRoleDefinedIn -->

    <owl:ObjectProperty rdf:about="https://w3id.org/arco/ontology/core/isRoleDefinedIn">
        <rdfs:comment xml:lang="en">A relation between a description and a role, e.g. the role &apos;Ingredient&apos; is defined in the recipe for a cake.</rdfs:comment>
        <rdfs:isDefinedBy rdf:resource="https://w3id.org/hacid/onto/top-level/"/>
        <rdfs:label xml:lang="en">is role defined in</rdfs:label>
    </owl:ObjectProperty>
    


    <!-- https://w3id.org/arco/ontology/core/isTaskDefinedIn -->

    <owl:ObjectProperty rdf:about="https://w3id.org/arco/ontology/core/isTaskDefinedIn">
        <rdfs:comment xml:lang="en">A relation between a description and a task, e.g. the task &apos;boil&apos; is defined in a recipe for a cake.</rdfs:comment>
        <rdfs:isDefinedBy rdf:resource="https://w3id.org/hacid/onto/top-level/"/>
        <rdfs:label xml:lang="en">is task defined in</rdfs:label>
    </owl:ObjectProperty>
    


    <!-- https://w3id.org/arco/ontology/core/isTaskOf -->

    <owl:ObjectProperty rdf:about="https://w3id.org/arco/ontology/core/isTaskOf">
        <rdfs:domain rdf:resource="https://w3id.org/arco/ontology/core/ClimateProcessTask"/>
        <rdfs:comment xml:lang="en">A relation between roles and tasks, e.g. &apos;students have the duty of giving exams&apos; (i.e. the Role &apos;student&apos; hasTask the Task &apos;giving exams&apos;).</rdfs:comment>
        <rdfs:isDefinedBy rdf:resource="https://w3id.org/hacid/onto/top-level/"/>
        <rdfs:label xml:lang="en">is task of</rdfs:label>
    </owl:ObjectProperty>
    


    <!-- https://w3id.org/arco/ontology/core/satisfies -->

    <owl:ObjectProperty rdf:about="https://w3id.org/arco/ontology/core/satisfies">
        <rdfs:domain rdf:resource="https://w3id.org/hacid/onto/top-level/Situation"/>
        <rdfs:range rdf:resource="https://w3id.org/hacid/onto/top-level/Plan"/>
        <rdfs:comment xml:lang="en">A relation between a Situation and a Description, e.g. the execution of a Plan satisfies that plan.</rdfs:comment>
        <rdfs:isDefinedBy rdf:resource="https://w3id.org/hacid/onto/top-level/"/>
        <rdfs:label xml:lang="en">satisfies</rdfs:label>
    </owl:ObjectProperty>
    


    <!-- https://w3id.org/hacid/onto/cs/classifies -->

    <owl:ObjectProperty rdf:about="https://w3id.org/hacid/onto/cs/classifies">
        <owl:inverseOf rdf:resource="https://w3id.org/hacid/onto/cs/isClassifiedBy"/>
        <rdfs:domain rdf:resource="http://www.w3.org/2002/07/owl#Thing"/>
        <rdfs:range rdf:resource="http://www.w3.org/2002/07/owl#Thing"/>
        <rdfs:comment xml:lang="en">A relation between a Concept and an Entity, e.g. the Role &apos;student&apos; classifies a Person &apos;John&apos;.</rdfs:comment>
        <rdfs:isDefinedBy rdf:resource="https://w3id.org/hacid/onto/top-level/"/>
        <rdfs:label xml:lang="en">classifies</rdfs:label>
    </owl:ObjectProperty>
    


    <!-- https://w3id.org/hacid/onto/cs/executesTask -->

    <owl:ObjectProperty rdf:about="https://w3id.org/hacid/onto/cs/executesTask">
        <rdfs:subPropertyOf rdf:resource="https://w3id.org/hacid/onto/cs/isClassifiedBy"/>
        <owl:inverseOf rdf:resource="https://w3id.org/hacid/onto/cs/isExecutedIn"/>
        <rdfs:domain rdf:resource="https://w3id.org/hacid/onto/cs/Action"/>
        <rdfs:range rdf:resource="https://w3id.org/hacid/onto/top-level/Task"/>
        <rdfs:comment xml:lang="en">A relation between an action and a task, e.g. &apos;putting some water in a pot and putting the pot on a fire until the water starts bubbling&apos; executes the task &apos;boiling&apos;.</rdfs:comment>
        <rdfs:isDefinedBy rdf:resource="https://w3id.org/hacid/onto/top-level/"/>
        <rdfs:label xml:lang="en">executes task</rdfs:label>
    </owl:ObjectProperty>
    


    <!-- https://w3id.org/hacid/onto/cs/hasParticipant -->

    <owl:ObjectProperty rdf:about="https://w3id.org/hacid/onto/cs/hasParticipant">
        <owl:inverseOf rdf:resource="https://w3id.org/hacid/onto/cs/isParticipantIn"/>
        <rdfs:domain rdf:resource="https://w3id.org/hacid/onto/top-level/Event"/>
        <rdfs:range rdf:resource="http://www.w3.org/2002/07/owl#Thing"/>
        <rdfs:comment xml:lang="en">A relation between an object and a process, e.g. &apos;John took part in the discussion&apos;, &apos;a large mass of snow fell during the avalanche&apos;, or &apos;a cook, some sugar, flour, etc. are all present in the cooking of a cake&apos;</rdfs:comment>
        <rdfs:isDefinedBy rdf:resource="https://w3id.org/hacid/onto/top-level/"/>
        <rdfs:label xml:lang="en">has participant</rdfs:label>
    </owl:ObjectProperty>
    


    <!-- https://w3id.org/hacid/onto/cs/involves -->

    <owl:ObjectProperty rdf:about="https://w3id.org/hacid/onto/cs/involves">
        <owl:inverseOf rdf:resource="https://w3id.org/hacid/onto/cs/isInvolvedIn"/>
        <rdfs:domain rdf:resource="http://www.w3.org/2002/07/owl#Thing"/>
        <rdfs:range rdf:resource="http://www.w3.org/2002/07/owl#Thing"/>
        <rdfs:comment xml:lang="en">The property that allows to assert that a task involves a certain concept.</rdfs:comment>
        <rdfs:label xml:lang="en">involves</rdfs:label>
    </owl:ObjectProperty>
    


    <!-- https://w3id.org/hacid/onto/cs/isClassifiedBy -->

    <owl:ObjectProperty rdf:about="https://w3id.org/hacid/onto/cs/isClassifiedBy">
        <rdfs:comment xml:lang="en">A relation between a Concept and an Entity, e.g. &apos;John is considered a typical rude man&apos;; your last concert constitutes the achievement of a lifetime; &apos;20-year-old means she&apos;s mature enough&apos;.</rdfs:comment>
        <rdfs:isDefinedBy rdf:resource="https://w3id.org/hacid/onto/top-level/"/>
        <rdfs:label xml:lang="en">is classified by</rdfs:label>
    </owl:ObjectProperty>
    


    <!-- https://w3id.org/hacid/onto/cs/isExecutedIn -->

    <owl:ObjectProperty rdf:about="https://w3id.org/hacid/onto/cs/isExecutedIn">
        <rdfs:domain rdf:resource="https://w3id.org/hacid/onto/top-level/Task"/>
        <rdfs:range rdf:resource="https://w3id.org/hacid/onto/cs/Action"/>
        <rdfs:comment xml:lang="en">A relation between an action and a task, e.g. &apos;putting some water in a pot and putting the pot on a fire until the water starts bubbling&apos; executes the task &apos;boiling&apos;.</rdfs:comment>
        <rdfs:isDefinedBy rdf:resource="https://w3id.org/hacid/onto/top-level/"/>
        <rdfs:label xml:lang="en">is executed in</rdfs:label>
    </owl:ObjectProperty>
    


    <!-- https://w3id.org/hacid/onto/cs/isInvolvedIn -->

    <owl:ObjectProperty rdf:about="https://w3id.org/hacid/onto/cs/isInvolvedIn">
        <rdfs:comment xml:lang="en">The peroperty that allows one to assert that a concept is involved in a task.</rdfs:comment>
    </owl:ObjectProperty>
    


    <!-- https://w3id.org/hacid/onto/cs/isParticipantIn -->

    <owl:ObjectProperty rdf:about="https://w3id.org/hacid/onto/cs/isParticipantIn">
        <rdfs:comment xml:lang="en">A relation between an object and a process, e.g. &apos;John took part in the discussion&apos;, &apos;a large mass of snow fell during the avalanche&apos;, or &apos;a cook, some sugar, flour, etc. are all present in the cooking of a cake&apos;.</rdfs:comment>
        <rdfs:isDefinedBy rdf:resource="https://w3id.org/hacid/onto/top-level/"/>
        <rdfs:label xml:lang="en">is participant in</rdfs:label>
    </owl:ObjectProperty>
    


    <!-- https://w3id.org/hacid/onto/top-level/follows -->

    <owl:ObjectProperty rdf:about="https://w3id.org/hacid/onto/top-level/follows">
        <rdfs:comment xml:lang="en">The intransitive follows relation.</rdfs:comment>
        <rdfs:isDefinedBy rdf:resource="https://w3id.org/hacid/onto/top-level/"/>
        <rdfs:label xml:lang="en">follows</rdfs:label>
    </owl:ObjectProperty>
    


    <!-- https://w3id.org/hacid/onto/top-level/precedes -->

    <owl:ObjectProperty rdf:about="https://w3id.org/hacid/onto/top-level/precedes">
        <rdfs:comment xml:lang="en">A relation between entities, expressing a sequence&apos;s schema.</rdfs:comment>
        <rdfs:isDefinedBy rdf:resource="https://w3id.org/hacid/onto/top-level/"/>
        <rdfs:label xml:lang="en">precedes</rdfs:label>
    </owl:ObjectProperty>
    


    <!-- 
    ///////////////////////////////////////////////////////////////////////////////////////
    //
    // Classes
    //
    ///////////////////////////////////////////////////////////////////////////////////////
     -->

    


    <!-- https://w3id.org/arco/ontology/core/ClimateProcessTask -->

    <owl:Class rdf:about="https://w3id.org/arco/ontology/core/ClimateProcessTask">
        <rdfs:subClassOf rdf:resource="https://w3id.org/hacid/onto/top-level/Task"/>
        <rdfs:subClassOf>
            <owl:Restriction>
                <owl:onProperty rdf:resource="https://w3id.org/hacid/onto/cs/involves"/>
                <owl:someValuesFrom rdf:resource="https://w3id.org/hacid/onto/ccso/ClimateModel"/>
            </owl:Restriction>
        </rdfs:subClassOf>
        <rdfs:subClassOf>
            <owl:Restriction>
                <owl:onProperty rdf:resource="https://w3id.org/hacid/onto/cs/involves"/>
                <owl:someValuesFrom rdf:resource="https://w3id.org/hacid/onto/ccso/Dataset"/>
            </owl:Restriction>
        </rdfs:subClassOf>
        <rdfs:subClassOf>
            <owl:Restriction>
                <owl:onProperty rdf:resource="https://w3id.org/hacid/onto/cs/involves"/>
                <owl:someValuesFrom rdf:resource="https://w3id.org/hacid/onto/ccso/Scenario"/>
            </owl:Restriction>
        </rdfs:subClassOf>
        <rdfs:subClassOf>
            <owl:Restriction>
                <owl:onProperty rdf:resource="https://w3id.org/hacid/onto/cs/involves"/>
                <owl:someValuesFrom rdf:resource="https://w3id.org/hacid/onto/ccso/Variable"/>
            </owl:Restriction>
        </rdfs:subClassOf>
        <rdfs:comment xml:lang="en">Tasks that are executed within the climate process workflow.</rdfs:comment>
        <rdfs:label xml:lang="en">Climate process task</rdfs:label>
    </owl:Class>
    


    <!-- https://w3id.org/hacid/onto/ccso/ClimateModel -->

    <owl:Class rdf:about="https://w3id.org/hacid/onto/ccso/ClimateModel">
        <rdfs:isDefinedBy rdf:resource="https://w3id.org/hacid/onto/ccso"/>
        <rdfs:label xml:lang="en">Cimate Model</rdfs:label>
    </owl:Class>
    


    <!-- https://w3id.org/hacid/onto/ccso/Dataset -->

    <owl:Class rdf:about="https://w3id.org/hacid/onto/ccso/Dataset">
        <rdfs:isDefinedBy rdf:resource="https://w3id.org/hacid/onto/csso"/>
        <rdfs:label xml:lang="en">Dataset</rdfs:label>
    </owl:Class>
    


    <!-- https://w3id.org/hacid/onto/ccso/Scenario -->

    <owl:Class rdf:about="https://w3id.org/hacid/onto/ccso/Scenario">
        <rdfs:isDefinedBy rdf:resource="https://w3id.org/hacid/onto/csso"/>
        <rdfs:label xml:lang="en">Scenario</rdfs:label>
    </owl:Class>
    


    <!-- https://w3id.org/hacid/onto/ccso/Variable -->

    <owl:Class rdf:about="https://w3id.org/hacid/onto/ccso/Variable">
        <rdfs:isDefinedBy rdf:resource="https://w3id.org/hacid/onto/csso"/>
        <rdfs:label xml:lang="en">Variable</rdfs:label>
    </owl:Class>
    


    <!-- https://w3id.org/hacid/onto/cs/Action -->

    <owl:Class rdf:about="https://w3id.org/hacid/onto/cs/Action">
        <rdfs:subClassOf rdf:resource="https://w3id.org/hacid/onto/top-level/Event"/>
        <rdfs:subClassOf>
            <owl:Restriction>
                <owl:onProperty rdf:resource="https://w3id.org/hacid/onto/cs/hasParticipant"/>
                <owl:someValuesFrom rdf:resource="https://w3id.org/hacid/onto/top-level/Agent"/>
            </owl:Restriction>
        </rdfs:subClassOf>
        <rdfs:subClassOf>
            <owl:Restriction>
                <owl:onProperty rdf:resource="https://w3id.org/hacid/onto/cs/executesTask"/>
                <owl:minQualifiedCardinality rdf:datatype="http://www.w3.org/2001/XMLSchema#nonNegativeInteger">1</owl:minQualifiedCardinality>
                <owl:onClass rdf:resource="https://w3id.org/hacid/onto/top-level/Task"/>
            </owl:Restriction>
        </rdfs:subClassOf>
        <rdfs:comment xml:lang="en">An Event with at least one Agent that isParticipantIn it, and that executes a Task that typically isDefinedIn a Plan, Workflow, Project, etc.</rdfs:comment>
        <rdfs:isDefinedBy rdf:resource="https://w3id.org/hacid/onto/top-level"/>
        <rdfs:label xml:lang="en">Action</rdfs:label>
    </owl:Class>
    


    <!-- https://w3id.org/hacid/onto/cs/ClimateProcessWorkflow -->

    <owl:Class rdf:about="https://w3id.org/hacid/onto/cs/ClimateProcessWorkflow">
        <rdfs:subClassOf rdf:resource="https://w3id.org/hacid/onto/top-level/Workflow"/>
        <rdfs:comment xml:lang="en">A workflow describing the handling of a request for climate information by instances such as MettOfice.</rdfs:comment>
        <rdfs:label xml:lang="en">Climate science case</rdfs:label>
    </owl:Class>
    


    <!-- https://w3id.org/hacid/onto/top-level/Agent -->

    <owl:Class rdf:about="https://w3id.org/hacid/onto/top-level/Agent">
        <rdfs:comment xml:lang="en">Any agentive Object , either physical (e.g. a whale, a robot, an oak), or social (e.g. a corporation, an institution, a community)</rdfs:comment>
        <rdfs:isDefinedBy rdf:resource="https://w3id.org/hacid/onto/top-level"/>
        <rdfs:label xml:lang="en">Agent</rdfs:label>
    </owl:Class>
    


    <!-- https://w3id.org/hacid/onto/top-level/Event -->

    <owl:Class rdf:about="https://w3id.org/hacid/onto/top-level/Event">
        <rdfs:comment xml:lang="en">Any physical, social, or mental process, event, or state.</rdfs:comment>
        <rdfs:isDefinedBy rdf:resource="https://w3id.org/hacid/onto/top-level"/>
        <rdfs:label xml:lang="en">Event</rdfs:label>
    </owl:Class>
    


    <!-- https://w3id.org/hacid/onto/top-level/EventType -->

    <owl:Class rdf:about="https://w3id.org/hacid/onto/top-level/EventType">
        <rdfs:subClassOf>
            <owl:Restriction>
                <owl:onProperty rdf:resource="https://w3id.org/hacid/onto/cs/classifies"/>
                <owl:someValuesFrom rdf:resource="https://w3id.org/hacid/onto/top-level/Event"/>
            </owl:Restriction>
        </rdfs:subClassOf>
        <owl:disjointWith rdf:resource="https://w3id.org/hacid/onto/top-level/Role"/>
        <rdfs:comment xml:lang="en">A Concept that classifies an Event . An event type describes how an Event should be interpreted, executed, expected, seen, etc., according to the Description that the EventType isDefinedIn (or used in)</rdfs:comment>
        <rdfs:isDefinedBy rdf:resource="https://w3id.org/hacid/onto/top-level"/>
        <rdfs:label xml:lang="en">Event Type</rdfs:label>
    </owl:Class>
    


    <!-- https://w3id.org/hacid/onto/top-level/Organisation -->

    <owl:Class rdf:about="https://w3id.org/hacid/onto/top-level/Organisation">
        <rdfs:subClassOf rdf:resource="https://w3id.org/hacid/onto/top-level/Agent"/>
        <rdfs:comment xml:lang="en">An organisation.</rdfs:comment>
        <rdfs:isDefinedBy rdf:resource="https://w3id.org/hacid/onto/top-level"/>
        <rdfs:label xml:lang="en">Organisation</rdfs:label>
    </owl:Class>
    


    <!-- https://w3id.org/hacid/onto/top-level/Plan -->

    <owl:Class rdf:about="https://w3id.org/hacid/onto/top-level/Plan">
        <rdfs:comment xml:lang="en">A Description having an explicit Goal, to be achieved by executing the plan</rdfs:comment>
        <rdfs:isDefinedBy rdf:resource="https://w3id.org/hacid/onto/top-level"/>
        <rdfs:label xml:lang="en">Plan</rdfs:label>
    </owl:Class>
    


    <!-- https://w3id.org/hacid/onto/top-level/Role -->

    <owl:Class rdf:about="https://w3id.org/hacid/onto/top-level/Role">
        <rdfs:comment xml:lang="en">A Concept that classifies an Object</rdfs:comment>
        <rdfs:isDefinedBy rdf:resource="https://w3id.org/hacid/onto/top-level"/>
        <rdfs:label xml:lang="en">Role</rdfs:label>
    </owl:Class>
    


    <!-- https://w3id.org/hacid/onto/top-level/Situation -->

    <owl:Class rdf:about="https://w3id.org/hacid/onto/top-level/Situation">
        <rdfs:comment xml:lang="en">A view, consistent with (&apos;satisfying&apos;) a Description, on a set of entities. 
It can also be seen as a &apos;relational context&apos; created by an observer on the basis of a &apos;frame&apos; (i.e. a Description). 
For example, a PlanExecution is a context including some actions executed by agents according to certain parameters and expected tasks to be achieved from a Plan; a DiagnosedSituation is a context of observed entities that is interpreted on the basis of a Diagnosis, etc.
Situation is also able to represent reified n-ary relations, where isSettingFor is the top-level relation for all binary projections of the n-ary relation. 
If used in a transformation pattern for n-ary relations, the designer should take care of adding (some or all) OWL2 keys, corresponding to binary projections of the n-ary, to a subclass of Situation. Otherwise the &apos;identification constraint&apos; (Calvanese et al., IJCAI 2001) might be violated.</rdfs:comment>
        <rdfs:isDefinedBy rdf:resource="https://w3id.org/hacid/onto/top-level/"/>
        <rdfs:label xml:lang="en">Situation</rdfs:label>
    </owl:Class>
    


    <!-- https://w3id.org/hacid/onto/top-level/Task -->

    <owl:Class rdf:about="https://w3id.org/hacid/onto/top-level/Task">
        <rdfs:subClassOf rdf:resource="https://w3id.org/hacid/onto/top-level/EventType"/>
        <rdfs:comment xml:lang="en">An EventType that classifies an Action to be executed. 
For example, reaching a destination is a task that can be executed by performing certain actions, e.g. driving a car, buying a train ticket, etc. 
The actions to execute a task can also be organized according to a Plan that is not the same as the one that defines the task (if any). 
For example, reaching a destination could be defined by a plan to get on holidays, while the plan to execute the task can consist of putting some travels into a sequence.</rdfs:comment>
        <rdfs:isDefinedBy rdf:resource="https://w3id.org/hacid/onto/top-level"/>
        <rdfs:label xml:lang="en">Task</rdfs:label>
    </owl:Class>
    


    <!-- https://w3id.org/hacid/onto/top-level/Workflow -->

    <owl:Class rdf:about="https://w3id.org/hacid/onto/top-level/Workflow">
        <rdfs:subClassOf rdf:resource="https://w3id.org/hacid/onto/top-level/Plan"/>
        <rdfs:comment xml:lang="en">A Plan that defines Role(s), Task(s), and a specific structure for tasks to be executed, usually supporting the work of an Organization.</rdfs:comment>
        <rdfs:isDefinedBy rdf:resource="https://w3id.org/hacid/onto/top-level/"/>
        <rdfs:label xml:lang="en">Workflow</rdfs:label>
    </owl:Class>
    


    <!-- https://w3id.org/hacid/onto/top-level/WorkflowExecution -->

    <owl:Class rdf:about="https://w3id.org/hacid/onto/top-level/WorkflowExecution">
        <rdfs:subClassOf rdf:resource="https://w3id.org/hacid/onto/top-level/Situation"/>
        <rdfs:comment xml:lang="en">The execution of a workflow</rdfs:comment>
        <rdfs:isDefinedBy rdf:resource="https://w3id.org/hacid/onto/top-level/"/>
        <rdfs:label xml:lang="en">Workflow Execution</rdfs:label>
    </owl:Class>
    


    <!-- 
    ///////////////////////////////////////////////////////////////////////////////////////
    //
    // Individuals
    //
    ///////////////////////////////////////////////////////////////////////////////////////
     -->

    


    <!-- https://w3id.org/hacid/onto/cs/BaselineChoice -->

    <owl:NamedIndividual rdf:about="https://w3id.org/hacid/onto/cs/BaselineChoice">
        <rdf:type rdf:resource="https://w3id.org/arco/ontology/core/ClimateProcessTask"/>
        <core:directlyPrecedes rdf:resource="https://w3id.org/hacid/onto/cs/FuturePeriodChoice"/>
        <core:isTaskOf rdf:resource="https://w3id.org/hacid/onto/cs/Solver"/>
        <rdfs:comment xml:lang="en">The task of choosing the baseline.</rdfs:comment>
        <rdfs:label xml:lang="en">Baseline choice</rdfs:label>
    </owl:NamedIndividual>
    


    <!-- https://w3id.org/hacid/onto/cs/CaseCreation -->

    <owl:NamedIndividual rdf:about="https://w3id.org/hacid/onto/cs/CaseCreation">
        <rdf:type rdf:resource="https://w3id.org/arco/ontology/core/ClimateProcessTask"/>
        <core:directlyFollows rdf:resource="https://w3id.org/hacid/onto/cs/UserInformationExtraction"/>
        <core:directlyPrecedes rdf:resource="https://w3id.org/hacid/onto/cs/ClimateInformationPreparation"/>
        <core:directlyPrecedes rdf:resource="https://w3id.org/hacid/onto/cs/ExternalExpertiseRequest"/>
        <core:isTaskOf rdf:resource="https://w3id.org/hacid/onto/cs/Creator"/>
        <rdfs:comment xml:lang="en">The task of creating a case.</rdfs:comment>
        <rdfs:label xml:lang="en">Case creation</rdfs:label>
    </owl:NamedIndividual>
    


    <!-- https://w3id.org/hacid/onto/cs/ClimateChangeQuantificationApplication -->

    <owl:NamedIndividual rdf:about="https://w3id.org/hacid/onto/cs/ClimateChangeQuantificationApplication">
        <rdf:type rdf:resource="https://w3id.org/arco/ontology/core/ClimateProcessTask"/>
        <core:directlyFollows rdf:resource="https://w3id.org/hacid/onto/cs/FuturePeriodChoice"/>
        <core:directlyPrecedes rdf:resource="https://w3id.org/hacid/onto/cs/UncertaintyQuantificationApplication"/>
        <core:isTaskOf rdf:resource="https://w3id.org/hacid/onto/cs/Creator"/>
        <rdfs:comment xml:lang="en">The task of applying the climate change quantification method.</rdfs:comment>
        <rdfs:label xml:lang="en">Climate change quantification application</rdfs:label>
    </owl:NamedIndividual>
    


    <!-- https://w3id.org/hacid/onto/cs/ClimateInformationAnalysis -->

    <owl:NamedIndividual rdf:about="https://w3id.org/hacid/onto/cs/ClimateInformationAnalysis">
        <rdf:type rdf:resource="https://w3id.org/arco/ontology/core/ClimateProcessTask"/>
        <core:directlyFollows rdf:resource="https://w3id.org/hacid/onto/cs/ClimateInformationPreparation"/>
        <core:directlyFollows rdf:resource="https://w3id.org/hacid/onto/cs/ExternalExpertiseRequest"/>
        <core:directlyPrecedes rdf:resource="https://w3id.org/hacid/onto/cs/SendClimateInformation"/>
        <core:hasPart rdf:resource="https://w3id.org/hacid/onto/cs/BaselineChoice"/>
        <core:hasPart rdf:resource="https://w3id.org/hacid/onto/cs/ClimateChangeQuantificationApplication"/>
        <core:hasPart rdf:resource="https://w3id.org/hacid/onto/cs/FuturePeriodChoice"/>
        <core:hasPart rdf:resource="https://w3id.org/hacid/onto/cs/MethodologicalRequirementApplication"/>
        <core:hasPart rdf:resource="https://w3id.org/hacid/onto/cs/UncertaintyQuantificationApplication"/>
        <core:isTaskOf rdf:resource="https://w3id.org/hacid/onto/cs/Solver"/>
        <rdfs:comment xml:lang="en">The task of analysing the climate information.</rdfs:comment>
        <rdfs:label xml:lang="en">Climate information analysis</rdfs:label>
    </owl:NamedIndividual>
    


    <!-- https://w3id.org/hacid/onto/cs/ClimateInformationCommunication -->

    <owl:NamedIndividual rdf:about="https://w3id.org/hacid/onto/cs/ClimateInformationCommunication">
        <rdf:type rdf:resource="https://w3id.org/arco/ontology/core/ClimateProcessTask"/>
        <core:directlyFollows rdf:resource="https://w3id.org/hacid/onto/cs/SendClimateInformation"/>
        <core:isTaskOf rdf:resource="https://w3id.org/hacid/onto/cs/User"/>
        <rdfs:comment xml:lang="en">The task of communicating the climate information.</rdfs:comment>
        <rdfs:label xml:lang="en">Climate information communication</rdfs:label>
    </owl:NamedIndividual>
    


    <!-- https://w3id.org/hacid/onto/cs/ClimateInformationPreparation -->

    <owl:NamedIndividual rdf:about="https://w3id.org/hacid/onto/cs/ClimateInformationPreparation">
        <rdf:type rdf:resource="https://w3id.org/arco/ontology/core/ClimateProcessTask"/>
        <core:directlyFollows rdf:resource="https://w3id.org/hacid/onto/cs/CaseCreation"/>
        <core:directlyPrecedes rdf:resource="https://w3id.org/hacid/onto/cs/ClimateInformationAnalysis"/>
        <core:hasPart rdf:resource="https://w3id.org/hacid/onto/cs/ClimateModelEvaluation"/>
        <core:hasPart rdf:resource="https://w3id.org/hacid/onto/cs/ClimateModelSelection"/>
        <core:hasPart rdf:resource="https://w3id.org/hacid/onto/cs/DataSelection"/>
        <core:hasPart rdf:resource="https://w3id.org/hacid/onto/cs/EmissionScenarioDefinition"/>
        <core:hasPart rdf:resource="https://w3id.org/hacid/onto/cs/MetricAndVariableIdentification"/>
        <core:isTaskOf rdf:resource="https://w3id.org/hacid/onto/cs/Solver"/>
        <rdfs:comment xml:lang="en">The task of preparing the climate information.</rdfs:comment>
        <rdfs:label xml:lang="en">Climate information preparation</rdfs:label>
    </owl:NamedIndividual>
    


    <!-- https://w3id.org/hacid/onto/cs/ClimateInformationRequest -->

    <owl:NamedIndividual rdf:about="https://w3id.org/hacid/onto/cs/ClimateInformationRequest">
        <rdf:type rdf:resource="https://w3id.org/arco/ontology/core/ClimateProcessTask"/>
        <core:directlyPrecedes rdf:resource="https://w3id.org/hacid/onto/cs/UserBackgroundInformationRequest"/>
        <core:isTaskOf rdf:resource="https://w3id.org/hacid/onto/cs/User"/>
        <rdfs:comment xml:lang="en">The task of requesting the climate information.</rdfs:comment>
        <rdfs:label xml:lang="en">Climate information request</rdfs:label>
    </owl:NamedIndividual>
    


    <!-- https://w3id.org/hacid/onto/cs/ClimateInformationRequestGoalDefinition -->

    <owl:NamedIndividual rdf:about="https://w3id.org/hacid/onto/cs/ClimateInformationRequestGoalDefinition">
        <rdf:type rdf:resource="https://w3id.org/arco/ontology/core/ClimateProcessTask"/>
        <core:isTaskOf rdf:resource="https://w3id.org/hacid/onto/cs/User"/>
        <rdfs:comment xml:lang="en">The task of defining the goal of the climate information request.</rdfs:comment>
        <rdfs:label xml:lang="en">Climate information request goal definition</rdfs:label>
    </owl:NamedIndividual>
    


    <!-- https://w3id.org/hacid/onto/cs/ClimateModelEvaluation -->

    <owl:NamedIndividual rdf:about="https://w3id.org/hacid/onto/cs/ClimateModelEvaluation">
        <rdf:type rdf:resource="https://w3id.org/arco/ontology/core/ClimateProcessTask"/>
        <core:directlyFollows rdf:resource="https://w3id.org/hacid/onto/cs/DataSelection"/>
        <core:directlyPrecedes rdf:resource="https://w3id.org/hacid/onto/cs/ClimateModelSelection"/>
        <core:isTaskOf rdf:resource="https://w3id.org/hacid/onto/cs/Solver"/>
        <rdfs:comment xml:lang="en">The task of evaluating the climate model.</rdfs:comment>
        <rdfs:label xml:lang="en">Climate model evaluation</rdfs:label>
    </owl:NamedIndividual>
    


    <!-- https://w3id.org/hacid/onto/cs/ClimateModelSelection -->

    <owl:NamedIndividual rdf:about="https://w3id.org/hacid/onto/cs/ClimateModelSelection">
        <rdf:type rdf:resource="https://w3id.org/arco/ontology/core/ClimateProcessTask"/>
        <core:directlyFollows rdf:resource="https://w3id.org/hacid/onto/cs/ClimateModelEvaluation"/>
        <core:isTaskOf rdf:resource="https://w3id.org/hacid/onto/cs/Solver"/>
        <rdfs:comment xml:lang="en">The task of selecing the climate model.</rdfs:comment>
        <rdfs:label xml:lang="en">Climate model selection</rdfs:label>
    </owl:NamedIndividual>
    


    <!-- https://w3id.org/hacid/onto/cs/ClimateRiskFramingSpecification -->

    <owl:NamedIndividual rdf:about="https://w3id.org/hacid/onto/cs/ClimateRiskFramingSpecification">
        <rdf:type rdf:resource="https://w3id.org/arco/ontology/core/ClimateProcessTask"/>
        <core:isTaskOf rdf:resource="https://w3id.org/hacid/onto/cs/User"/>
        <rdfs:comment xml:lang="en">The task of specifying the climate risk framing.</rdfs:comment>
        <rdfs:label xml:lang="en">Climate risk framing specification</rdfs:label>
    </owl:NamedIndividual>
    


    <!-- https://w3id.org/hacid/onto/cs/Creator -->

    <owl:NamedIndividual rdf:about="https://w3id.org/hacid/onto/cs/Creator">
        <rdf:type rdf:resource="https://w3id.org/hacid/onto/top-level/Role"/>
        <rdfs:comment xml:lang="en">The creator of the climate case.</rdfs:comment>
        <rdfs:label xml:lang="en">Creator</rdfs:label>
    </owl:NamedIndividual>
    


    <!-- https://w3id.org/hacid/onto/cs/DataSelection -->

    <owl:NamedIndividual rdf:about="https://w3id.org/hacid/onto/cs/DataSelection">
        <rdf:type rdf:resource="https://w3id.org/arco/ontology/core/ClimateProcessTask"/>
        <core:directlyFollows rdf:resource="https://w3id.org/hacid/onto/cs/EmissionScenarioDefinition"/>
        <core:directlyPrecedes rdf:resource="https://w3id.org/hacid/onto/cs/ClimateModelEvaluation"/>
        <core:isTaskOf rdf:resource="https://w3id.org/hacid/onto/cs/Solver"/>
        <rdfs:comment xml:lang="en">The task of selecting the data.</rdfs:comment>
        <rdfs:label xml:lang="en">Data selection</rdfs:label>
    </owl:NamedIndividual>
    


    <!-- https://w3id.org/hacid/onto/cs/EmissionScenarioDefinition -->

    <owl:NamedIndividual rdf:about="https://w3id.org/hacid/onto/cs/EmissionScenarioDefinition">
        <rdf:type rdf:resource="https://w3id.org/arco/ontology/core/ClimateProcessTask"/>
        <core:directlyFollows rdf:resource="https://w3id.org/hacid/onto/cs/MetricAndVariableIdentification"/>
        <core:directlyPrecedes rdf:resource="https://w3id.org/hacid/onto/cs/DataSelection"/>
        <core:isTaskOf rdf:resource="https://w3id.org/hacid/onto/cs/Solver"/>
        <rdfs:comment xml:lang="en">The task of defining the emission scenarios.</rdfs:comment>
        <rdfs:label xml:lang="en">Emission scenario definition</rdfs:label>
    </owl:NamedIndividual>
    


    <!-- https://w3id.org/hacid/onto/cs/ExternalExpertiseRequest -->

    <owl:NamedIndividual rdf:about="https://w3id.org/hacid/onto/cs/ExternalExpertiseRequest">
        <rdf:type rdf:resource="https://w3id.org/arco/ontology/core/ClimateProcessTask"/>
        <core:directlyFollows rdf:resource="https://w3id.org/hacid/onto/cs/CaseCreation"/>
        <core:directlyPrecedes rdf:resource="https://w3id.org/hacid/onto/cs/ClimateInformationAnalysis"/>
        <core:isTaskOf rdf:resource="https://w3id.org/hacid/onto/cs/Solver"/>
        <rdfs:comment xml:lang="en">The task of requesting external expertise such as an expert or literature review.</rdfs:comment>
        <rdfs:label xml:lang="en">External expertise request</rdfs:label>
    </owl:NamedIndividual>
    


    <!-- https://w3id.org/hacid/onto/cs/FuturePeriodChoice -->

    <owl:NamedIndividual rdf:about="https://w3id.org/hacid/onto/cs/FuturePeriodChoice">
        <rdf:type rdf:resource="https://w3id.org/arco/ontology/core/ClimateProcessTask"/>
        <core:directlyFollows rdf:resource="https://w3id.org/hacid/onto/cs/BaselineChoice"/>
        <core:directlyPrecedes rdf:resource="https://w3id.org/hacid/onto/cs/ClimateChangeQuantificationApplication"/>
        <core:isTaskOf rdf:resource="https://w3id.org/hacid/onto/cs/Solver"/>
        <rdfs:comment xml:lang="en">The task of choosig the future period.</rdfs:comment>
        <rdfs:label xml:lang="en">Future period choice</rdfs:label>
    </owl:NamedIndividual>
    


    <!-- https://w3id.org/hacid/onto/cs/HazardIdentification -->

    <owl:NamedIndividual rdf:about="https://w3id.org/hacid/onto/cs/HazardIdentification">
        <rdf:type rdf:resource="https://w3id.org/arco/ontology/core/ClimateProcessTask"/>
        <core:isTaskOf rdf:resource="https://w3id.org/hacid/onto/cs/Solver"/>
        <core:isTaskOf rdf:resource="https://w3id.org/hacid/onto/cs/User"/>
        <rdfs:comment xml:lang="en">The task of identifying hazards.</rdfs:comment>
        <rdfs:label xml:lang="en">Hazard identification</rdfs:label>
    </owl:NamedIndividual>
    


    <!-- https://w3id.org/hacid/onto/cs/InformationOnExposureIdentification -->

    <owl:NamedIndividual rdf:about="https://w3id.org/hacid/onto/cs/InformationOnExposureIdentification">
        <rdf:type rdf:resource="https://w3id.org/arco/ontology/core/ClimateProcessTask"/>
        <core:isTaskOf rdf:resource="https://w3id.org/hacid/onto/cs/User"/>
        <rdfs:comment xml:lang="en">The task of identifying information on exposure.</rdfs:comment>
        <rdfs:label xml:lang="en">Information on exposure identification</rdfs:label>
    </owl:NamedIndividual>
    


    <!-- https://w3id.org/hacid/onto/cs/MethodologicalRequirementApplication -->

    <owl:NamedIndividual rdf:about="https://w3id.org/hacid/onto/cs/MethodologicalRequirementApplication">
        <rdf:type rdf:resource="https://w3id.org/arco/ontology/core/ClimateProcessTask"/>
        <core:directlyFollows rdf:resource="https://w3id.org/hacid/onto/cs/UncertaintyQuantificationApplication"/>
        <core:isTaskOf rdf:resource="https://w3id.org/hacid/onto/cs/Solver"/>
        <rdfs:comment xml:lang="en">The task of applying methodological requirements.</rdfs:comment>
        <rdfs:label xml:lang="en">Methodological requirement application</rdfs:label>
    </owl:NamedIndividual>
    


    <!-- https://w3id.org/hacid/onto/cs/MetricAndVariableIdentification -->

    <owl:NamedIndividual rdf:about="https://w3id.org/hacid/onto/cs/MetricAndVariableIdentification">
        <rdf:type rdf:resource="https://w3id.org/arco/ontology/core/ClimateProcessTask"/>
        <core:directlyPrecedes rdf:resource="https://w3id.org/hacid/onto/cs/EmissionScenarioDefinition"/>
        <core:isTaskOf rdf:resource="https://w3id.org/hacid/onto/cs/Solver"/>
        <rdfs:comment xml:lang="en">The task of identifying metrics and variables.</rdfs:comment>
        <rdfs:label xml:lang="en">Metric and variable identification</rdfs:label>
    </owl:NamedIndividual>
    


    <!-- https://w3id.org/hacid/onto/cs/OrganisationInformationDescription -->

    <owl:NamedIndividual rdf:about="https://w3id.org/hacid/onto/cs/OrganisationInformationDescription">
        <rdf:type rdf:resource="https://w3id.org/arco/ontology/core/ClimateProcessTask"/>
        <core:isTaskOf rdf:resource="https://w3id.org/hacid/onto/cs/User"/>
        <rdfs:comment xml:lang="en">The task of describing organisation information.</rdfs:comment>
        <rdfs:label xml:lang="en">Organisation information description</rdfs:label>
    </owl:NamedIndividual>
    


    <!-- https://w3id.org/hacid/onto/cs/PlanningTimeScalesDefinition -->

    <owl:NamedIndividual rdf:about="https://w3id.org/hacid/onto/cs/PlanningTimeScalesDefinition">
        <rdf:type rdf:resource="https://w3id.org/arco/ontology/core/ClimateProcessTask"/>
        <core:isTaskOf rdf:resource="https://w3id.org/hacid/onto/cs/User"/>
        <rdfs:comment xml:lang="en">The task of defining planning time scales.</rdfs:comment>
        <rdfs:label xml:lang="en">Planning time scales definition</rdfs:label>
    </owl:NamedIndividual>
    


    <!-- https://w3id.org/hacid/onto/cs/ProvideBackgroundInformation -->

    <owl:NamedIndividual rdf:about="https://w3id.org/hacid/onto/cs/ProvideBackgroundInformation">
        <rdf:type rdf:resource="https://w3id.org/arco/ontology/core/ClimateProcessTask"/>
        <core:directlyFollows rdf:resource="https://w3id.org/hacid/onto/cs/UserBackgroundInformationRequest"/>
        <core:directlyPrecedes rdf:resource="https://w3id.org/hacid/onto/cs/ProvideDecisionContextInformation"/>
        <core:hasPart rdf:resource="https://w3id.org/hacid/onto/cs/ClimateInformationRequestGoalDefinition"/>
        <core:hasPart rdf:resource="https://w3id.org/hacid/onto/cs/OrganisationInformationDescription"/>
        <core:isTaskOf rdf:resource="https://w3id.org/hacid/onto/cs/User"/>
        <rdfs:comment xml:lang="en">The task of providing background information.</rdfs:comment>
        <rdfs:label xml:lang="en">Provide background information</rdfs:label>
    </owl:NamedIndividual>
    


    <!-- https://w3id.org/hacid/onto/cs/ProvideDecisionContextInformation -->

    <owl:NamedIndividual rdf:about="https://w3id.org/hacid/onto/cs/ProvideDecisionContextInformation">
        <rdf:type rdf:resource="https://w3id.org/arco/ontology/core/ClimateProcessTask"/>
        <core:directlyFollows rdf:resource="https://w3id.org/hacid/onto/cs/ProvideDecisionContextInformation"/>
        <core:directlyPrecedes rdf:resource="https://w3id.org/hacid/onto/cs/UserInformationExtraction"/>
        <core:hasPart rdf:resource="https://w3id.org/hacid/onto/cs/ClimateRiskFramingSpecification"/>
        <core:hasPart rdf:resource="https://w3id.org/hacid/onto/cs/HazardIdentification"/>
        <core:hasPart rdf:resource="https://w3id.org/hacid/onto/cs/InformationOnExposureIdentification"/>
        <core:hasPart rdf:resource="https://w3id.org/hacid/onto/cs/PlanningTimeScalesDefinition"/>
        <core:isTaskOf rdf:resource="https://w3id.org/hacid/onto/cs/User"/>
        <rdfs:comment xml:lang="en">The task of providing decision context information.</rdfs:comment>
        <rdfs:label xml:lang="en">Provide decision context information</rdfs:label>
    </owl:NamedIndividual>
    


    <!-- https://w3id.org/hacid/onto/cs/SendClimateInformation -->

    <owl:NamedIndividual rdf:about="https://w3id.org/hacid/onto/cs/SendClimateInformation">
        <rdf:type rdf:resource="https://w3id.org/arco/ontology/core/ClimateProcessTask"/>
        <core:directlyFollows rdf:resource="https://w3id.org/hacid/onto/cs/ClimateInformationAnalysis"/>
        <core:directlyFollows rdf:resource="https://w3id.org/hacid/onto/cs/ClimateInformationCommunication"/>
        <core:isTaskOf rdf:resource="https://w3id.org/hacid/onto/cs/Solver"/>
        <rdfs:comment xml:lang="en">The task of sending climate information.</rdfs:comment>
        <rdfs:label xml:lang="en">Send climate information</rdfs:label>
    </owl:NamedIndividual>
    


    <!-- https://w3id.org/hacid/onto/cs/Solver -->

    <owl:NamedIndividual rdf:about="https://w3id.org/hacid/onto/cs/Solver">
        <rdf:type rdf:resource="https://w3id.org/hacid/onto/top-level/Role"/>
        <rdfs:comment xml:lang="en">The solver of the climate case.</rdfs:comment>
        <rdfs:label xml:lang="en">Solver</rdfs:label>
    </owl:NamedIndividual>
    


    <!-- https://w3id.org/hacid/onto/cs/UncertaintyQuantificationApplication -->

    <owl:NamedIndividual rdf:about="https://w3id.org/hacid/onto/cs/UncertaintyQuantificationApplication">
        <rdf:type rdf:resource="https://w3id.org/arco/ontology/core/ClimateProcessTask"/>
        <core:directlyFollows rdf:resource="https://w3id.org/hacid/onto/cs/ClimateChangeQuantificationApplication"/>
        <core:directlyPrecedes rdf:resource="https://w3id.org/hacid/onto/cs/MethodologicalRequirementApplication"/>
        <core:isTaskOf rdf:resource="https://w3id.org/hacid/onto/cs/Solver"/>
        <rdfs:comment xml:lang="en">The task of applying uncertainty quantification</rdfs:comment>
        <rdfs:label xml:lang="en">Uncertainty quantification application</rdfs:label>
    </owl:NamedIndividual>
    


    <!-- https://w3id.org/hacid/onto/cs/User -->

    <owl:NamedIndividual rdf:about="https://w3id.org/hacid/onto/cs/User">
        <rdf:type rdf:resource="https://w3id.org/hacid/onto/top-level/Role"/>
        <rdfs:comment xml:lang="en">The user that requests and uses the climate information.</rdfs:comment>
        <rdfs:label xml:lang="en">User</rdfs:label>
    </owl:NamedIndividual>
    


    <!-- https://w3id.org/hacid/onto/cs/UserBackgroundInformationRequest -->

    <owl:NamedIndividual rdf:about="https://w3id.org/hacid/onto/cs/UserBackgroundInformationRequest">
        <rdf:type rdf:resource="https://w3id.org/arco/ontology/core/ClimateProcessTask"/>
        <core:directlyFollows rdf:resource="https://w3id.org/hacid/onto/cs/ClimateInformationRequest"/>
        <core:directlyPrecedes rdf:resource="https://w3id.org/hacid/onto/cs/ProvideBackgroundInformation"/>
        <core:isTaskOf rdf:resource="https://w3id.org/hacid/onto/cs/Creator"/>
        <rdfs:comment xml:lang="en">The task of requesting user background information.</rdfs:comment>
        <rdfs:label xml:lang="en">User background information request</rdfs:label>
    </owl:NamedIndividual>
    


    <!-- https://w3id.org/hacid/onto/cs/UserInformationExtraction -->

    <owl:NamedIndividual rdf:about="https://w3id.org/hacid/onto/cs/UserInformationExtraction">
        <rdf:type rdf:resource="https://w3id.org/arco/ontology/core/ClimateProcessTask"/>
        <core:directlyFollows rdf:resource="https://w3id.org/hacid/onto/cs/ProvideDecisionContextInformation"/>
        <core:directlyPrecedes rdf:resource="https://w3id.org/hacid/onto/cs/CaseCreation"/>
        <core:isTaskOf rdf:resource="https://w3id.org/hacid/onto/cs/Creator"/>
        <rdfs:comment xml:lang="en">The task of extracting user information.</rdfs:comment>
        <rdfs:label xml:lang="en">User information request</rdfs:label>
    </owl:NamedIndividual>
</rdf:RDF>



<!-- Generated by the OWL API (version 4.5.9.2019-02-01T07:24:44Z) https://github.com/owlcs/owlapi -->

