<?xml version="1.0"?>
<rdf:RDF xmlns="https://w3id.org/hacid/onto/ccso#"
     xml:base="https://w3id.org/hacid/onto/ccso"
     xmlns:dc="http://purl.org/dc/elements/1.1/"
     xmlns:owl="http://www.w3.org/2002/07/owl#"
     xmlns:rdf="http://www.w3.org/1999/02/22-rdf-syntax-ns#"
     xmlns:top="https://w3id.org/hacid/onto/top-level/"
     xmlns:xml="http://www.w3.org/XML/1998/namespace"
     xmlns:xsd="http://www.w3.org/2001/XMLSchema#"
     xmlns:dcat="http://www.w3.org/ns/dcat#"
     xmlns:rdfs="http://www.w3.org/2000/01/rdf-schema#"
     xmlns:terms="http://purl.org/dc/terms/">
    <owl:Ontology rdf:about="https://w3id.org/hacid/onto/ccso">
        <owl:versionIRI rdf:resource="https://w3id.org/hacid/onto/ccso/2.0/"/>
        <owl:imports rdf:resource="https://w3id.org/hacid/onto/data"/>
        <owl:imports rdf:resource="https://w3id.org/hacid/onto/top-level"/>
        <dc:description rdf:resource="https://raw.githubusercontent.com/hacid-project/knowledge-graph/main/ontologies/climate-services/visual/simpler_model_rev.png"/>
        <terms:creator rdf:resource="https://w3id.org/hacid/data/cs/person/andrea-giovanni-nuzzolese"/>
        <terms:creator rdf:resource="https://w3id.org/hacid/data/cs/person/miguel-ceriani"/>
        <terms:title xml:lang="en">CCSO - Core Climate Services Ontology</terms:title>
        <rdfs:comment xml:lang="en">The Core Climate Services Ontology (CCSO) is a comprehensive framework designed to facilitate the representation and integration of diverse climate-related data and knowledge. This ontology encompasses key concepts related to climate models, simulations, datasets, variables, and scenarios, along with their associated characteristics. The CCSO enables structured and standardized descriptions of these elements, promoting interoperability and data sharing among various stakeholders in climate science.

Key features of the ontology include definitions of object properties such as spatial and temporal coverage, spatial and temporal resolution, and the relationships between simulations, datasets, climate models, and scenarios. These relationships are crucial for linking datasets with the variables they contain, the models used to generate climate projections, and the scenarios that guide simulation experiments.

The ontology also categorizes different types of scenarios, such as Greenhouse Gas Concentration Pathways and Shared Socioeconomic Pathways, which are essential for modeling and predicting the impacts of various emission trajectories on the climate system. By providing a clear and systematic way to describe and relate these complex elements, the CCSO aims to enhance the understanding, analysis, and dissemination of climate data, ultimately supporting more informed decision-making in climate research and policy.

Overall, the Core Climate Services Ontology serves as a vital tool for organizing climate knowledge, facilitating data interoperability, and advancing the study and application of climate science.</rdfs:comment>
        <rdfs:label xml:lang="en">CCSO - Core Climate Services Ontology</rdfs:label>
        <dcat:keyword xml:lang="en">climate model simulations</dcat:keyword>
        <dcat:keyword xml:lang="en">climate models</dcat:keyword>
        <dcat:keyword xml:lang="en">climate services</dcat:keyword>
        <dcat:keyword xml:lang="en">climate variables</dcat:keyword>
        <dcat:theme xml:lang="en">Climate services</dcat:theme>
    </owl:Ontology>
    


    <!-- 
    ///////////////////////////////////////////////////////////////////////////////////////
    //
    // Annotation properties
    //
    ///////////////////////////////////////////////////////////////////////////////////////
     -->

    


    <!-- http://purl.org/dc/elements/1.1/description -->

    <owl:AnnotationProperty rdf:about="http://purl.org/dc/elements/1.1/description"/>
    


    <!-- http://purl.org/dc/terms/creator -->

    <owl:AnnotationProperty rdf:about="http://purl.org/dc/terms/creator"/>
    


    <!-- http://purl.org/dc/terms/title -->

    <owl:AnnotationProperty rdf:about="http://purl.org/dc/terms/title"/>
    


    <!-- http://www.w3.org/ns/dcat#keyword -->

    <owl:AnnotationProperty rdf:about="http://www.w3.org/ns/dcat#keyword"/>
    


    <!-- http://www.w3.org/ns/dcat#theme -->

    <owl:AnnotationProperty rdf:about="http://www.w3.org/ns/dcat#theme"/>
    


    <!-- 
    ///////////////////////////////////////////////////////////////////////////////////////
    //
    // Object Properties
    //
    ///////////////////////////////////////////////////////////////////////////////////////
     -->

    


    <!-- https://w3id.org/hacid/onto/ccso/assertsVulnerabilityToImpactType -->

    <owl:ObjectProperty rdf:about="https://w3id.org/hacid/onto/ccso/assertsVulnerabilityToImpactType">
        <rdfs:subPropertyOf rdf:resource="https://w3id.org/hacid/onto/top-level/associatedWith"/>
        <owl:inverseOf rdf:resource="https://w3id.org/hacid/onto/ccso/isImpactTypeOfAssertedVulnerability"/>
        <rdfs:domain rdf:resource="https://w3id.org/hacid/onto/ccso/Vulnerability"/>
        <rdfs:range rdf:resource="https://w3id.org/hacid/onto/ccso/ImpactType"/>
        <rdfs:comment xml:lang="en">Associates a vulnerability with an impact type that the vulnerability asserts.</rdfs:comment>
        <rdfs:isDefinedBy rdf:resource="https://w3id.org/hacid/onto/ccso"/>
        <rdfs:label xml:lang="en">asserts vulnerability to impact type</rdfs:label>
    </owl:ObjectProperty>
    


    <!-- https://w3id.org/hacid/onto/ccso/causesPhenomenaOfType -->

    <owl:ObjectProperty rdf:about="https://w3id.org/hacid/onto/ccso/causesPhenomenaOfType">
        <rdfs:subPropertyOf rdf:resource="https://w3id.org/hacid/onto/top-level/associatedWith"/>
        <owl:inverseOf rdf:resource="https://w3id.org/hacid/onto/ccso/isCausedByPhenomenaOfType"/>
        <rdfs:domain rdf:resource="https://w3id.org/hacid/onto/ccso/ClimatePhenomenonType"/>
        <rdfs:range rdf:resource="https://w3id.org/hacid/onto/ccso/ClimatePhenomenonType"/>
        <rdfs:comment xml:lang="en">Associates two types of phenomena that can be causally related, the first causing the second.</rdfs:comment>
        <rdfs:isDefinedBy rdf:resource="https://w3id.org/hacid/onto/ccso"/>
        <rdfs:label xml:lang="en">causes phenomena of type</rdfs:label>
    </owl:ObjectProperty>
    


    <!-- https://w3id.org/hacid/onto/ccso/hasDownscaling -->

    <owl:ObjectProperty rdf:about="https://w3id.org/hacid/onto/ccso/hasDownscaling">
        <rdfs:subPropertyOf rdf:resource="https://w3id.org/hacid/onto/top-level/associatedWith"/>
        <owl:inverseOf rdf:resource="https://w3id.org/hacid/onto/ccso/isDownscalingOf"/>
        <rdfs:domain rdf:resource="https://w3id.org/hacid/onto/ccso/ClimateSimulation"/>
        <rdfs:range rdf:resource="https://w3id.org/hacid/onto/ccso/Downscaling"/>
        <rdfs:comment xml:lang="en">The property that allows one to assert that the output of a climate simulation has been used for a simulation downscaling.</rdfs:comment>
        <rdfs:isDefinedBy rdf:resource="https://w3id.org/hacid/onto/ccso"/>
        <rdfs:label xml:lang="en">has downscaling</rdfs:label>
    </owl:ObjectProperty>
    


    <!-- https://w3id.org/hacid/onto/ccso/hasImpact -->

    <owl:ObjectProperty rdf:about="https://w3id.org/hacid/onto/ccso/hasImpact">
        <rdfs:subPropertyOf rdf:resource="https://w3id.org/hacid/onto/top-level/associatedWith"/>
        <rdfs:domain rdf:resource="https://w3id.org/hacid/onto/ccso/ClimatePhenomenon"/>
        <rdfs:range rdf:resource="https://w3id.org/hacid/onto/ccso/Impact"/>
        <rdfs:comment xml:lang="en">Associates a climate phenomenon with its impact on some asset.</rdfs:comment>
        <rdfs:isDefinedBy rdf:resource="https://w3id.org/hacid/onto/ccso"/>
        <rdfs:label xml:lang="en">has impact</rdfs:label>
    </owl:ObjectProperty>
    


    <!-- https://w3id.org/hacid/onto/ccso/hasMemberSimulation -->

    <owl:ObjectProperty rdf:about="https://w3id.org/hacid/onto/ccso/hasMemberSimulation">
        <rdfs:subPropertyOf rdf:resource="https://w3id.org/hacid/onto/top-level/associatedWith"/>
        <owl:inverseOf rdf:resource="https://w3id.org/hacid/onto/ccso/isMemberSimulationOf"/>
        <rdfs:domain rdf:resource="https://w3id.org/hacid/onto/ccso/EnsembleSimulation"/>
        <rdfs:range rdf:resource="https://w3id.org/hacid/onto/ccso/Simulation"/>
        <rdfs:comment xml:lang="en">Associates an ensemble simulation with each of the simulations of which it is composed of.</rdfs:comment>
        <rdfs:isDefinedBy rdf:resource="https://w3id.org/hacid/onto/ccso"/>
        <rdfs:label xml:lang="en">has member simulation</rdfs:label>
    </owl:ObjectProperty>
    


    <!-- https://w3id.org/hacid/onto/ccso/hasPotentialImpactType -->

    <owl:ObjectProperty rdf:about="https://w3id.org/hacid/onto/ccso/hasPotentialImpactType">
        <rdfs:subPropertyOf rdf:resource="https://w3id.org/hacid/onto/top-level/associatedWith"/>
        <owl:inverseOf rdf:resource="https://w3id.org/hacid/onto/ccso/isPotentialImpactTypeOf"/>
        <rdfs:domain rdf:resource="https://w3id.org/hacid/onto/ccso/HazardType"/>
        <rdfs:range rdf:resource="https://w3id.org/hacid/onto/ccso/ImpactType"/>
        <rdfs:isDefinedBy rdf:resource="https://w3id.org/hacid/onto/ccso"/>
        <rdfs:label xml:lang="en">has potential impact type</rdfs:label>
    </owl:ObjectProperty>
    


    <!-- https://w3id.org/hacid/onto/ccso/hasPotentialVulnerabilityType -->

    <owl:ObjectProperty rdf:about="https://w3id.org/hacid/onto/ccso/hasPotentialVulnerabilityType">
        <rdfs:subPropertyOf rdf:resource="https://w3id.org/hacid/onto/top-level/associatedWith"/>
        <owl:inverseOf rdf:resource="https://w3id.org/hacid/onto/ccso/isPotentialVulnerabilityTypeOf"/>
        <rdfs:domain rdf:resource="https://w3id.org/hacid/onto/ccso/Asset_Type"/>
        <rdfs:range rdf:resource="https://w3id.org/hacid/onto/ccso/VulnerabilityType"/>
        <rdfs:isDefinedBy rdf:resource="https://w3id.org/hacid/onto/ccso"/>
        <rdfs:label xml:lang="en">has potential vulnerability type</rdfs:label>
    </owl:ObjectProperty>
    


    <!-- https://w3id.org/hacid/onto/ccso/hasPotentiallyImpactedVulnerability -->

    <owl:ObjectProperty rdf:about="https://w3id.org/hacid/onto/ccso/hasPotentiallyImpactedVulnerability">
        <rdfs:subPropertyOf rdf:resource="https://w3id.org/hacid/onto/top-level/associatedWith"/>
        <owl:inverseOf rdf:resource="https://w3id.org/hacid/onto/ccso/isVulnerabilityToImpactType"/>
        <rdfs:domain rdf:resource="https://w3id.org/hacid/onto/ccso/ImpactType"/>
        <rdfs:range rdf:resource="https://w3id.org/hacid/onto/ccso/Vulnerability"/>
        <rdfs:isDefinedBy rdf:resource="https://w3id.org/hacid/onto/ccso"/>
        <rdfs:label xml:lang="en">has potentially impacted vulnerability</rdfs:label>
    </owl:ObjectProperty>
    


    <!-- https://w3id.org/hacid/onto/ccso/hasVulnerability -->

    <owl:ObjectProperty rdf:about="https://w3id.org/hacid/onto/ccso/hasVulnerability">
        <rdfs:subPropertyOf rdf:resource="https://w3id.org/hacid/onto/top-level/associatedWith"/>
        <owl:inverseOf rdf:resource="https://w3id.org/hacid/onto/ccso/isVulnerabilityOf"/>
        <rdfs:domain rdf:resource="https://w3id.org/hacid/onto/ccso/Asset"/>
        <rdfs:range rdf:resource="https://w3id.org/hacid/onto/ccso/Vulnerability"/>
        <rdfs:isDefinedBy rdf:resource="https://w3id.org/hacid/onto/ccso"/>
        <rdfs:label xml:lang="en">has vulnerability</rdfs:label>
    </owl:ObjectProperty>
    


    <!-- https://w3id.org/hacid/onto/ccso/isCausedByPhenomenaOfType -->

    <owl:ObjectProperty rdf:about="https://w3id.org/hacid/onto/ccso/isCausedByPhenomenaOfType">
        <rdfs:subPropertyOf rdf:resource="https://w3id.org/hacid/onto/top-level/associatedWith"/>
        <rdfs:domain rdf:resource="https://w3id.org/hacid/onto/ccso/ClimatePhenomenonType"/>
        <rdfs:range rdf:resource="https://w3id.org/hacid/onto/ccso/ClimatePhenomenonType"/>
        <rdfs:comment xml:lang="en">Associates two types of phenomena that can be causally related, the second causing the first.</rdfs:comment>
        <rdfs:isDefinedBy rdf:resource="https://w3id.org/hacid/onto/ccso"/>
        <rdfs:label xml:lang="en">is caused by phenomena of type</rdfs:label>
    </owl:ObjectProperty>
    


    <!-- https://w3id.org/hacid/onto/ccso/isDownscalingOf -->

    <owl:ObjectProperty rdf:about="https://w3id.org/hacid/onto/ccso/isDownscalingOf">
        <rdfs:subPropertyOf rdf:resource="https://w3id.org/hacid/onto/top-level/associatedWith"/>
        <rdfs:domain rdf:resource="https://w3id.org/hacid/onto/ccso/Downscaling"/>
        <rdfs:range rdf:resource="https://w3id.org/hacid/onto/ccso/ClimateSimulation"/>
        <rdfs:comment xml:lang="en">The property that allows one to assert that a simulation downscaling has as source the output of climate simulation.</rdfs:comment>
        <rdfs:isDefinedBy rdf:resource="https://w3id.org/hacid/onto/ccso"/>
        <rdfs:label xml:lang="en">is downscaling of</rdfs:label>
    </owl:ObjectProperty>
    


    <!-- https://w3id.org/hacid/onto/ccso/isImpactTypeOfAssertedVulnerability -->

    <owl:ObjectProperty rdf:about="https://w3id.org/hacid/onto/ccso/isImpactTypeOfAssertedVulnerability">
        <rdfs:subPropertyOf rdf:resource="https://w3id.org/hacid/onto/top-level/associatedWith"/>
        <owl:inverseOf rdf:resource="https://w3id.org/hacid/onto/ccso/potentiallyAssertsVulnerabilityToImpactType"/>
        <rdfs:domain rdf:resource="https://w3id.org/hacid/onto/ccso/ImpactType"/>
        <rdfs:range rdf:resource="https://w3id.org/hacid/onto/ccso/VulnerabilityType"/>
        <rdfs:isDefinedBy rdf:resource="https://w3id.org/hacid/onto/ccso"/>
        <rdfs:label xml:lang="en">is impact type of asserted vulnerability</rdfs:label>
    </owl:ObjectProperty>
    


    <!-- https://w3id.org/hacid/onto/ccso/isMaintainedBy -->

    <owl:ObjectProperty rdf:about="https://w3id.org/hacid/onto/ccso/isMaintainedBy">
        <rdfs:subPropertyOf rdf:resource="https://w3id.org/hacid/onto/top-level/associatedWith"/>
        <owl:inverseOf rdf:resource="https://w3id.org/hacid/onto/ccso/maintains"/>
        <rdfs:domain rdf:resource="https://w3id.org/hacid/onto/top-level/Entity"/>
        <rdfs:comment xml:lang="en">The relation that allows to link an object to a maintainer.</rdfs:comment>
        <rdfs:isDefinedBy rdf:resource="https://w3id.org/hacid/onto/ccso"/>
        <rdfs:label xml:lang="en">is maintained by</rdfs:label>
    </owl:ObjectProperty>
    


    <!-- https://w3id.org/hacid/onto/ccso/isMemberSimulationOf -->

    <owl:ObjectProperty rdf:about="https://w3id.org/hacid/onto/ccso/isMemberSimulationOf">
        <rdfs:subPropertyOf rdf:resource="https://w3id.org/hacid/onto/top-level/associatedWith"/>
        <rdfs:domain rdf:resource="https://w3id.org/hacid/onto/ccso/Simulation"/>
        <rdfs:range rdf:resource="https://w3id.org/hacid/onto/ccso/EnsembleSimulation"/>
        <rdfs:comment xml:lang="en">Associates a simulation with an ensemble simulation that includes it.</rdfs:comment>
        <rdfs:isDefinedBy rdf:resource="https://w3id.org/hacid/onto/ccso"/>
        <rdfs:label xml:lang="en">is member simulation of</rdfs:label>
    </owl:ObjectProperty>
    


    <!-- https://w3id.org/hacid/onto/ccso/isModelUsedBy -->

    <owl:ObjectProperty rdf:about="https://w3id.org/hacid/onto/ccso/isModelUsedBy">
        <rdfs:subPropertyOf rdf:resource="https://w3id.org/hacid/onto/top-level/associatedWith"/>
        <owl:inverseOf rdf:resource="https://w3id.org/hacid/onto/ccso/usesModel"/>
        <rdfs:domain rdf:resource="https://w3id.org/hacid/onto/ccso/ClimateModel"/>
        <rdfs:range rdf:resource="https://w3id.org/hacid/onto/ccso/ClimateSimulation"/>
        <rdfs:isDefinedBy rdf:resource="https://w3id.org/hacid/onto/ccso"/>
        <rdfs:label xml:lang="en">is model used by</rdfs:label>
    </owl:ObjectProperty>
    


    <!-- https://w3id.org/hacid/onto/ccso/isPotentialImpactTypeOf -->

    <owl:ObjectProperty rdf:about="https://w3id.org/hacid/onto/ccso/isPotentialImpactTypeOf">
        <rdfs:subPropertyOf rdf:resource="https://w3id.org/hacid/onto/top-level/associatedWith"/>
        <rdfs:domain rdf:resource="https://w3id.org/hacid/onto/ccso/ImpactType"/>
        <rdfs:range rdf:resource="https://w3id.org/hacid/onto/ccso/HazardType"/>
        <rdfs:isDefinedBy rdf:resource="https://w3id.org/hacid/onto/ccso"/>
        <rdfs:label xml:lang="en">is potential impact of</rdfs:label>
    </owl:ObjectProperty>
    


    <!-- https://w3id.org/hacid/onto/ccso/isPotentialVulnerabilityTypeOf -->

    <owl:ObjectProperty rdf:about="https://w3id.org/hacid/onto/ccso/isPotentialVulnerabilityTypeOf">
        <rdfs:subPropertyOf rdf:resource="https://w3id.org/hacid/onto/top-level/associatedWith"/>
        <rdfs:domain rdf:resource="https://w3id.org/hacid/onto/ccso/VulnerabilityType"/>
        <rdfs:range rdf:resource="https://w3id.org/hacid/onto/ccso/Asset_Type"/>
        <rdfs:isDefinedBy rdf:resource="https://w3id.org/hacid/onto/ccso"/>
        <rdfs:label xml:lang="en">is potential vulnerability type of</rdfs:label>
    </owl:ObjectProperty>
    


    <!-- https://w3id.org/hacid/onto/ccso/isPotentiallySufferedImpactTypeOf -->

    <owl:ObjectProperty rdf:about="https://w3id.org/hacid/onto/ccso/isPotentiallySufferedImpactTypeOf">
        <rdfs:subPropertyOf rdf:resource="https://w3id.org/hacid/onto/top-level/associatedWith"/>
        <owl:inverseOf rdf:resource="https://w3id.org/hacid/onto/ccso/potentiallySuffersImpactType"/>
        <rdfs:domain rdf:resource="https://w3id.org/hacid/onto/ccso/ImpactType"/>
        <rdfs:range rdf:resource="https://w3id.org/hacid/onto/ccso/Asset_Type"/>
        <rdfs:isDefinedBy rdf:resource="https://w3id.org/hacid/onto/ccso"/>
        <rdfs:label xml:lang="en">is potentially suffered impact type of</rdfs:label>
    </owl:ObjectProperty>
    


    <!-- https://w3id.org/hacid/onto/ccso/isScenarioReferredBy -->

    <owl:ObjectProperty rdf:about="https://w3id.org/hacid/onto/ccso/isScenarioReferredBy">
        <rdfs:subPropertyOf rdf:resource="https://w3id.org/hacid/onto/top-level/associatedWith"/>
        <owl:inverseOf rdf:resource="https://w3id.org/hacid/onto/ccso/refersToScenario"/>
        <rdfs:domain rdf:resource="https://w3id.org/hacid/onto/ccso/EmissionScenario"/>
        <rdfs:range rdf:resource="https://w3id.org/hacid/onto/ccso/ClimateSimulation"/>
        <rdfs:comment xml:lang="en">The object property that allows a scenario to be referred by a simulation.</rdfs:comment>
        <rdfs:isDefinedBy rdf:resource="https://w3id.org/hacid/onto/ccso"/>
        <rdfs:label xml:lang="en">is scenario referred by</rdfs:label>
    </owl:ObjectProperty>
    


    <!-- https://w3id.org/hacid/onto/ccso/isSufferedImpactOf -->

    <owl:ObjectProperty rdf:about="https://w3id.org/hacid/onto/ccso/isSufferedImpactOf">
        <rdfs:subPropertyOf rdf:resource="https://w3id.org/hacid/onto/top-level/associatedWith"/>
        <owl:inverseOf rdf:resource="https://w3id.org/hacid/onto/ccso/sufferedImpact"/>
        <rdfs:domain rdf:resource="https://w3id.org/hacid/onto/ccso/Impact"/>
        <rdfs:range rdf:resource="https://w3id.org/hacid/onto/ccso/Asset"/>
        <rdfs:isDefinedBy rdf:resource="https://w3id.org/hacid/onto/ccso"/>
        <rdfs:label xml:lang="en">is suffered impact of</rdfs:label>
    </owl:ObjectProperty>
    


    <!-- https://w3id.org/hacid/onto/ccso/isSufferedImpactTypeOf -->

    <owl:ObjectProperty rdf:about="https://w3id.org/hacid/onto/ccso/isSufferedImpactTypeOf">
        <rdfs:subPropertyOf rdf:resource="https://w3id.org/hacid/onto/top-level/associatedWith"/>
        <owl:inverseOf rdf:resource="https://w3id.org/hacid/onto/ccso/suffersImpactType"/>
        <rdfs:domain rdf:resource="https://w3id.org/hacid/onto/ccso/ImpactType"/>
        <rdfs:range rdf:resource="https://w3id.org/hacid/onto/ccso/Asset"/>
        <rdfs:isDefinedBy rdf:resource="https://w3id.org/hacid/onto/ccso"/>
        <rdfs:label xml:lang="en">is suffered impact type of</rdfs:label>
    </owl:ObjectProperty>
    


    <!-- https://w3id.org/hacid/onto/ccso/isVulnerabilityOf -->

    <owl:ObjectProperty rdf:about="https://w3id.org/hacid/onto/ccso/isVulnerabilityOf">
        <rdfs:subPropertyOf rdf:resource="https://w3id.org/hacid/onto/top-level/associatedWith"/>
        <rdfs:domain rdf:resource="https://w3id.org/hacid/onto/ccso/Vulnerability"/>
        <rdfs:range rdf:resource="https://w3id.org/hacid/onto/ccso/Asset"/>
        <rdfs:isDefinedBy rdf:resource="https://w3id.org/hacid/onto/ccso"/>
        <rdfs:label xml:lang="en">is vulnerability of</rdfs:label>
    </owl:ObjectProperty>
    


    <!-- https://w3id.org/hacid/onto/ccso/isVulnerabilityToImpactType -->

    <owl:ObjectProperty rdf:about="https://w3id.org/hacid/onto/ccso/isVulnerabilityToImpactType">
        <rdfs:subPropertyOf rdf:resource="https://w3id.org/hacid/onto/top-level/associatedWith"/>
        <rdfs:domain rdf:resource="https://w3id.org/hacid/onto/ccso/Vulnerability"/>
        <rdfs:range rdf:resource="https://w3id.org/hacid/onto/ccso/ImpactType"/>
        <rdfs:isDefinedBy rdf:resource="https://w3id.org/hacid/onto/ccso"/>
        <rdfs:label xml:lang="en">is vulnerability to impact type</rdfs:label>
    </owl:ObjectProperty>
    


    <!-- https://w3id.org/hacid/onto/ccso/maintains -->

    <owl:ObjectProperty rdf:about="https://w3id.org/hacid/onto/ccso/maintains">
        <rdfs:subPropertyOf rdf:resource="https://w3id.org/hacid/onto/top-level/associatedWith"/>
        <rdfs:range rdf:resource="https://w3id.org/hacid/onto/top-level/Entity"/>
        <rdfs:isDefinedBy rdf:resource="https://w3id.org/hacid/onto/ccso"/>
        <rdfs:label xml:lang="en">maintains</rdfs:label>
    </owl:ObjectProperty>
    


    <!-- https://w3id.org/hacid/onto/ccso/potentiallyAssertsVulnerabilityToImpactType -->

    <owl:ObjectProperty rdf:about="https://w3id.org/hacid/onto/ccso/potentiallyAssertsVulnerabilityToImpactType">
        <rdfs:subPropertyOf rdf:resource="https://w3id.org/hacid/onto/top-level/associatedWith"/>
        <rdfs:domain rdf:resource="https://w3id.org/hacid/onto/ccso/VulnerabilityType"/>
        <rdfs:range rdf:resource="https://w3id.org/hacid/onto/ccso/ImpactType"/>
        <rdfs:comment xml:lang="en">Associates a type of vulnerability with an impact type that is potentially asserted in the classified vulnerabilities.</rdfs:comment>
        <rdfs:isDefinedBy rdf:resource="https://w3id.org/hacid/onto/ccso"/>
        <rdfs:label xml:lang="en">potentially asserts vulnerability to impact type</rdfs:label>
    </owl:ObjectProperty>
    


    <!-- https://w3id.org/hacid/onto/ccso/potentiallySuffersImpactType -->

    <owl:ObjectProperty rdf:about="https://w3id.org/hacid/onto/ccso/potentiallySuffersImpactType">
        <rdfs:subPropertyOf rdf:resource="https://w3id.org/hacid/onto/top-level/associatedWith"/>
        <rdfs:domain rdf:resource="https://w3id.org/hacid/onto/ccso/Asset_Type"/>
        <rdfs:range rdf:resource="https://w3id.org/hacid/onto/ccso/ImpactType"/>
        <rdfs:isDefinedBy rdf:resource="https://w3id.org/hacid/onto/ccso"/>
        <rdfs:label xml:lang="en">potentially suffers impact type</rdfs:label>
    </owl:ObjectProperty>
    


    <!-- https://w3id.org/hacid/onto/ccso/refersToScenario -->

    <owl:ObjectProperty rdf:about="https://w3id.org/hacid/onto/ccso/refersToScenario">
        <rdfs:subPropertyOf rdf:resource="https://w3id.org/hacid/onto/top-level/associatedWith"/>
        <rdfs:domain rdf:resource="https://w3id.org/hacid/onto/ccso/ClimateSimulation"/>
        <rdfs:range rdf:resource="https://w3id.org/hacid/onto/ccso/EmissionScenario"/>
        <rdfs:comment xml:lang="en">The object property that allows a simulation to refer a scenario.</rdfs:comment>
        <rdfs:isDefinedBy rdf:resource="https://w3id.org/hacid/onto/ccso"/>
        <rdfs:label xml:lang="en">refers to scenario</rdfs:label>
    </owl:ObjectProperty>
    


    <!-- https://w3id.org/hacid/onto/ccso/relatedWithPhenomenon -->

    <owl:ObjectProperty rdf:about="https://w3id.org/hacid/onto/ccso/relatedWithPhenomenon">
        <rdfs:subPropertyOf rdf:resource="https://w3id.org/hacid/onto/top-level/associatedWith"/>
        <owl:inverseOf rdf:resource="https://w3id.org/hacid/onto/ccso/relatedWithPhenomenon"/>
        <rdf:type rdf:resource="http://www.w3.org/2002/07/owl#SymmetricProperty"/>
        <rdfs:isDefinedBy rdf:resource="https://w3id.org/hacid/onto/ccso"/>
        <rdfs:label xml:lang="en">related with phenomenon</rdfs:label>
    </owl:ObjectProperty>
    


    <!-- https://w3id.org/hacid/onto/ccso/sufferedImpact -->

    <owl:ObjectProperty rdf:about="https://w3id.org/hacid/onto/ccso/sufferedImpact">
        <rdfs:subPropertyOf rdf:resource="https://w3id.org/hacid/onto/top-level/associatedWith"/>
        <rdfs:domain rdf:resource="https://w3id.org/hacid/onto/ccso/Asset"/>
        <rdfs:range rdf:resource="https://w3id.org/hacid/onto/ccso/Impact"/>
        <rdfs:isDefinedBy rdf:resource="https://w3id.org/hacid/onto/ccso"/>
        <rdfs:label xml:lang="en">suffered impact</rdfs:label>
    </owl:ObjectProperty>
    


    <!-- https://w3id.org/hacid/onto/ccso/suffersImpactType -->

    <owl:ObjectProperty rdf:about="https://w3id.org/hacid/onto/ccso/suffersImpactType">
        <rdfs:subPropertyOf rdf:resource="https://w3id.org/hacid/onto/top-level/associatedWith"/>
        <rdfs:domain rdf:resource="https://w3id.org/hacid/onto/ccso/Asset"/>
        <rdfs:range rdf:resource="https://w3id.org/hacid/onto/ccso/ImpactType"/>
        <rdfs:isDefinedBy rdf:resource="https://w3id.org/hacid/onto/ccso"/>
        <rdfs:label xml:lang="en">suffers impact type</rdfs:label>
    </owl:ObjectProperty>
    


    <!-- https://w3id.org/hacid/onto/ccso/usesModel -->

    <owl:ObjectProperty rdf:about="https://w3id.org/hacid/onto/ccso/usesModel">
        <rdfs:subPropertyOf rdf:resource="https://w3id.org/hacid/onto/top-level/associatedWith"/>
        <rdfs:domain rdf:resource="https://w3id.org/hacid/onto/ccso/ClimateSimulation"/>
        <rdfs:range rdf:resource="https://w3id.org/hacid/onto/ccso/ClimateModel"/>
        <rdfs:comment xml:lang="en">The property that allows one to assert that a climate model is used by an experiment to simulate the behavior and evolution of the Earth’s climate system over a specified period.</rdfs:comment>
        <rdfs:comment xml:lang="en">The property that allows one to assert that an experiment uses a climate model to simulate the behavior and evolution of the Earth’s climate system over a specified period.</rdfs:comment>
        <rdfs:isDefinedBy rdf:resource="https://w3id.org/hacid/onto/ccso"/>
        <rdfs:label xml:lang="en">uses model</rdfs:label>
    </owl:ObjectProperty>
    


    <!-- 
    ///////////////////////////////////////////////////////////////////////////////////////
    //
    // Classes
    //
    ///////////////////////////////////////////////////////////////////////////////////////
     -->

    


    <!-- https://w3id.org/hacid/onto/ccso/Asset -->

    <owl:Class rdf:about="https://w3id.org/hacid/onto/ccso/Asset">
        <rdfs:subClassOf rdf:resource="https://w3id.org/hacid/onto/top-level#Object"/>
        <rdfs:isDefinedBy rdf:resource="https://w3id.org/hacid/onto/ccso"/>
        <rdfs:label xml:lang="en">Asset</rdfs:label>
    </owl:Class>
    


    <!-- https://w3id.org/hacid/onto/ccso/Asset_Type -->

    <owl:Class rdf:about="https://w3id.org/hacid/onto/ccso/Asset_Type">
        <rdfs:subClassOf rdf:resource="https://w3id.org/hacid/onto/top-level/Concept"/>
        <rdfs:subClassOf>
            <owl:Restriction>
                <owl:onProperty rdf:resource="https://w3id.org/hacid/onto/top-level/classifies"/>
                <owl:allValuesFrom rdf:resource="https://w3id.org/hacid/onto/ccso/Asset"/>
            </owl:Restriction>
        </rdfs:subClassOf>
        <rdfs:isDefinedBy rdf:resource="https://w3id.org/hacid/onto/ccso"/>
        <rdfs:label xml:lang="en">Asset Type</rdfs:label>
    </owl:Class>
    


    <!-- https://w3id.org/hacid/onto/ccso/ClimateModel -->

    <owl:Class rdf:about="https://w3id.org/hacid/onto/ccso/ClimateModel">
        <rdfs:subClassOf rdf:resource="https://w3id.org/hacid/onto/top-level/Entity"/>
        <rdfs:comment xml:lang="en">A representation of the Earth’s climate system. A model is used to simulate and understand the climate, including its variability and changes over time, by using a set of equations based on physical, chemical, and biological principles.</rdfs:comment>
        <rdfs:isDefinedBy rdf:resource="https://w3id.org/hacid/onto/ccso"/>
        <rdfs:label xml:lang="en">Climate Model</rdfs:label>
    </owl:Class>
    


    <!-- https://w3id.org/hacid/onto/ccso/ClimatePhenomenon -->

    <owl:Class rdf:about="https://w3id.org/hacid/onto/ccso/ClimatePhenomenon">
        <rdfs:subClassOf rdf:resource="https://w3id.org/hacid/onto/top-level/Situation"/>
        <rdfs:isDefinedBy rdf:resource="https://w3id.org/hacid/onto/ccso"/>
        <rdfs:label xml:lang="en">Climate Phenomenon</rdfs:label>
    </owl:Class>
    


    <!-- https://w3id.org/hacid/onto/ccso/ClimatePhenomenonType -->

    <owl:Class rdf:about="https://w3id.org/hacid/onto/ccso/ClimatePhenomenonType">
        <rdfs:subClassOf rdf:resource="https://w3id.org/hacid/onto/top-level/Concept"/>
        <rdfs:subClassOf>
            <owl:Restriction>
                <owl:onProperty rdf:resource="https://w3id.org/hacid/onto/top-level/classifies"/>
                <owl:allValuesFrom rdf:resource="https://w3id.org/hacid/onto/ccso/ClimatePhenomenon"/>
            </owl:Restriction>
        </rdfs:subClassOf>
        <rdfs:isDefinedBy rdf:resource="https://w3id.org/hacid/onto/ccso"/>
        <rdfs:label xml:lang="en">Climate Phenomenon Type</rdfs:label>
    </owl:Class>
    


    <!-- https://w3id.org/hacid/onto/ccso/ClimateSimulation -->

    <owl:Class rdf:about="https://w3id.org/hacid/onto/ccso/ClimateSimulation">
        <rdfs:subClassOf rdf:resource="https://w3id.org/hacid/onto/ccso/Simulation"/>
        <rdfs:subClassOf>
            <owl:Restriction>
                <owl:onProperty rdf:resource="https://w3id.org/hacid/onto/ccso/usesModel"/>
                <owl:someValuesFrom rdf:resource="https://w3id.org/hacid/onto/ccso/ClimateModel"/>
            </owl:Restriction>
        </rdfs:subClassOf>
        <rdfs:comment xml:lang="en">A computational experiment that uses a climate model to simulate the behavior and evolution of the Earth’s climate system over a specified period. These simulations are designed to understand how various components of the climate system interact and respond to different forcing factors, such as changes in greenhouse gas concentrations, solar radiation, volcanic activity, and land use.</rdfs:comment>
        <rdfs:isDefinedBy rdf:resource="https://w3id.org/hacid/onto/ccso"/>
        <rdfs:label xml:lang="en">Climate Simulation</rdfs:label>
    </owl:Class>
    


    <!-- https://w3id.org/hacid/onto/ccso/Downscaling -->

    <owl:Class rdf:about="https://w3id.org/hacid/onto/ccso/Downscaling">
        <rdfs:subClassOf rdf:resource="https://w3id.org/hacid/onto/data/DataGeneratingProcess"/>
        <rdfs:subClassOf>
            <owl:Restriction>
                <owl:onProperty rdf:resource="https://w3id.org/hacid/onto/ccso/isDownscalingOf"/>
                <owl:someValuesFrom rdf:resource="https://w3id.org/hacid/onto/ccso/ClimateSimulation"/>
            </owl:Restriction>
        </rdfs:subClassOf>
        <rdfs:comment xml:lang="en">A process taking as input the output of a climate simulation and obtaining finer granularity, usually at the cost of reduced geographic coverage.</rdfs:comment>
        <rdfs:isDefinedBy rdf:resource="https://w3id.org/hacid/onto/ccso"/>
        <rdfs:label xml:lang="en">Downscaling</rdfs:label>
    </owl:Class>
    


    <!-- https://w3id.org/hacid/onto/ccso/DynamicalDownscaling -->

    <owl:Class rdf:about="https://w3id.org/hacid/onto/ccso/DynamicalDownscaling">
        <rdfs:subClassOf rdf:resource="https://w3id.org/hacid/onto/ccso/ClimateSimulation"/>
        <rdfs:subClassOf rdf:resource="https://w3id.org/hacid/onto/ccso/Downscaling"/>
        <rdfs:comment xml:lang="en">A simulation using as constraint the output of another simulation, run at a coarser granularity (with typically broader coverage): e.g., a regional simulation run using as constraint the output a global simulation.</rdfs:comment>
        <rdfs:isDefinedBy rdf:resource="https://w3id.org/hacid/onto/ccso"/>
        <rdfs:label xml:lang="en">Dynamical Downscaling</rdfs:label>
    </owl:Class>
    


    <!-- https://w3id.org/hacid/onto/ccso/EmissionScenario -->

    <owl:Class rdf:about="https://w3id.org/hacid/onto/ccso/EmissionScenario">
        <rdfs:subClassOf rdf:resource="https://w3id.org/hacid/onto/top-level/Entity"/>
        <rdfs:comment xml:lang="en">A projected trajectory of future greenhouse gas emissions, atmospheric concentrations, and corresponding impacts on the climate system. These scenarios are used in climate modeling to explore how different levels of emissions might influence global temperatures, weather patterns, sea level rise, and other climate-related phenomena.</rdfs:comment>
        <rdfs:isDefinedBy rdf:resource="https://w3id.org/hacid/onto/ccso"/>
        <rdfs:label xml:lang="en">Emission Scenario</rdfs:label>
    </owl:Class>
    


    <!-- https://w3id.org/hacid/onto/ccso/EnsembleSimulation -->

    <owl:Class rdf:about="https://w3id.org/hacid/onto/ccso/EnsembleSimulation">
        <rdfs:subClassOf rdf:resource="https://w3id.org/hacid/onto/ccso/Simulation"/>
        <rdfs:isDefinedBy rdf:resource="https://w3id.org/hacid/onto/ccso"/>
        <rdfs:label>Ensemble Simulation</rdfs:label>
    </owl:Class>
    


    <!-- https://w3id.org/hacid/onto/ccso/GlobalClimateModel -->

    <owl:Class rdf:about="https://w3id.org/hacid/onto/ccso/GlobalClimateModel">
        <rdfs:subClassOf rdf:resource="https://w3id.org/hacid/onto/ccso/ClimateModel"/>
        <rdfs:comment xml:lang="en">A climate model meant to be used to simulate climate at global (Earth) scale.</rdfs:comment>
        <rdfs:isDefinedBy rdf:resource="https://w3id.org/hacid/onto/ccso"/>
        <rdfs:label xml:lang="en">Global Climate Model</rdfs:label>
    </owl:Class>
    


    <!-- https://w3id.org/hacid/onto/ccso/GlobalClimateSimulation -->

    <owl:Class rdf:about="https://w3id.org/hacid/onto/ccso/GlobalClimateSimulation">
        <rdfs:subClassOf rdf:resource="https://w3id.org/hacid/onto/ccso/ClimateSimulation"/>
        <rdfs:comment xml:lang="en">A climate simulation run at global scale, i.e. for all the surface of Earth.</rdfs:comment>
        <rdfs:isDefinedBy rdf:resource="https://w3id.org/hacid/onto/ccso"/>
        <rdfs:label xml:lang="en">Global Climate Simulation</rdfs:label>
    </owl:Class>
    


    <!-- https://w3id.org/hacid/onto/ccso/GreenhouseGasConcentrationPathway -->

    <owl:Class rdf:about="https://w3id.org/hacid/onto/ccso/GreenhouseGasConcentrationPathway">
        <rdfs:subClassOf rdf:resource="https://w3id.org/hacid/onto/ccso/EmissionScenario"/>
        <rdfs:comment xml:lang="en">These pathways are used to model and predict the impacts of different levels of greenhouse gas emissions on the climate system. They are essential for understanding how different emissions scenarios might influence global temperatures, climate patterns, and related environmental changes.</rdfs:comment>
        <rdfs:isDefinedBy rdf:resource="https://w3id.org/hacid/onto/ccso"/>
        <rdfs:label xml:lang="en">Greenhouse gas concentration pathway</rdfs:label>
    </owl:Class>
    


    <!-- https://w3id.org/hacid/onto/ccso/HazardType -->

    <owl:Class rdf:about="https://w3id.org/hacid/onto/ccso/HazardType">
        <rdfs:subClassOf rdf:resource="https://w3id.org/hacid/onto/ccso/ClimatePhenomenonType"/>
        <rdfs:isDefinedBy rdf:resource="https://w3id.org/hacid/onto/ccso"/>
        <rdfs:label xml:lang="en">Hazard Type</rdfs:label>
    </owl:Class>
    


    <!-- https://w3id.org/hacid/onto/ccso/Impact -->

    <owl:Class rdf:about="https://w3id.org/hacid/onto/ccso/Impact">
        <rdfs:subClassOf rdf:resource="https://w3id.org/hacid/onto/top-level/Situation"/>
        <rdfs:isDefinedBy rdf:resource="https://w3id.org/hacid/onto/ccso"/>
        <rdfs:label xml:lang="en">Impact</rdfs:label>
    </owl:Class>
    


    <!-- https://w3id.org/hacid/onto/ccso/ImpactType -->

    <owl:Class rdf:about="https://w3id.org/hacid/onto/ccso/ImpactType">
        <rdfs:subClassOf rdf:resource="https://w3id.org/hacid/onto/top-level/Concept"/>
        <rdfs:subClassOf>
            <owl:Restriction>
                <owl:onProperty rdf:resource="https://w3id.org/hacid/onto/top-level/classifies"/>
                <owl:allValuesFrom rdf:resource="https://w3id.org/hacid/onto/ccso/Impact"/>
            </owl:Restriction>
        </rdfs:subClassOf>
        <rdfs:isDefinedBy rdf:resource="https://w3id.org/hacid/onto/ccso"/>
        <rdfs:label xml:lang="en">Impact Type</rdfs:label>
    </owl:Class>
    


    <!-- https://w3id.org/hacid/onto/ccso/RegionalClimateModel -->

    <owl:Class rdf:about="https://w3id.org/hacid/onto/ccso/RegionalClimateModel">
        <rdfs:subClassOf rdf:resource="https://w3id.org/hacid/onto/ccso/ClimateModel"/>
        <rdfs:comment xml:lang="en">A climate model meant to be used to simulate climate at regional scale.</rdfs:comment>
        <rdfs:isDefinedBy rdf:resource="https://w3id.org/hacid/onto/ccso"/>
        <rdfs:label xml:lang="en">Regional Climate Model</rdfs:label>
    </owl:Class>
    


    <!-- https://w3id.org/hacid/onto/ccso/SharedSocioeconomicPathway -->

    <owl:Class rdf:about="https://w3id.org/hacid/onto/ccso/SharedSocioeconomicPathway">
        <rdfs:subClassOf rdf:resource="https://w3id.org/hacid/onto/ccso/EmissionScenario"/>
        <rdfs:comment xml:lang="en">Shared socio-economic Pathways (SSPs) are scenarios developed to describe different trajectories of socioeconomic development, which can influence future greenhouse gas emissions and the ability of societies to mitigate and adapt to climate change. The SSPs are used in climate modeling to explore the interactions between socioeconomic factors, emissions pathways, and climate impacts.</rdfs:comment>
        <rdfs:isDefinedBy rdf:resource="https://w3id.org/hacid/onto/ccso"/>
        <rdfs:label xml:lang="en">Shared socio-economic pathway</rdfs:label>
    </owl:Class>
    


    <!-- https://w3id.org/hacid/onto/ccso/Simulation -->

    <owl:Class rdf:about="https://w3id.org/hacid/onto/ccso/Simulation">
        <rdfs:subClassOf rdf:resource="https://w3id.org/hacid/onto/data/DataGeneratingProcess"/>
        <rdfs:isDefinedBy rdf:resource="https://w3id.org/hacid/onto/ccso"/>
        <rdfs:label xml:lang="en">Simulation</rdfs:label>
    </owl:Class>
    


    <!-- https://w3id.org/hacid/onto/ccso/StatisticalDownscaling -->

    <owl:Class rdf:about="https://w3id.org/hacid/onto/ccso/StatisticalDownscaling">
        <rdfs:subClassOf rdf:resource="https://w3id.org/hacid/onto/ccso/Downscaling"/>
        <rdfs:isDefinedBy rdf:resource="https://w3id.org/hacid/onto/ccso"/>
        <rdfs:label xml:lang="en">Statistical Downscaling</rdfs:label>
    </owl:Class>
    


    <!-- https://w3id.org/hacid/onto/ccso/TimeDuration -->

    <owl:Class rdf:about="https://w3id.org/hacid/onto/ccso/TimeDuration">
        <rdfs:subClassOf rdf:resource="https://w3id.org/hacid/onto/top-level/TimeEntity"/>
        <rdfs:comment xml:lang="en">A time duration: e.g., 486 seconds; 3 years; 1 hour and 20 minutes; etc.</rdfs:comment>
        <rdfs:isDefinedBy rdf:resource="https://w3id.org/hacid/onto/ccso"/>
        <rdfs:label xml:lang="en">Time Duration</rdfs:label>
    </owl:Class>
    


    <!-- https://w3id.org/hacid/onto/ccso/TimeInterval -->

    <owl:Class rdf:about="https://w3id.org/hacid/onto/ccso/TimeInterval">
        <rdfs:subClassOf rdf:resource="https://w3id.org/hacid/onto/top-level/TimeEntity"/>
        <rdfs:comment xml:lang="en">An interval in time: e.g., from the 1st January 2020 to 31th December 2070.</rdfs:comment>
        <rdfs:isDefinedBy rdf:resource="https://w3id.org/hacid/onto/ccso"/>
        <rdfs:label xml:lang="en">Time Interval</rdfs:label>
    </owl:Class>
    


    <!-- https://w3id.org/hacid/onto/ccso/Vulnerability -->

    <owl:Class rdf:about="https://w3id.org/hacid/onto/ccso/Vulnerability">
        <rdfs:subClassOf rdf:resource="https://w3id.org/hacid/onto/top-level/Situation"/>
        <rdfs:comment xml:lang="en">The susceptibility of an asset to damage or disruption from a specific hazard, considering factors like exposure, sensitivity, and adaptive capacity.</rdfs:comment>
        <rdfs:isDefinedBy rdf:resource="https://w3id.org/hacid/onto/ccso"/>
        <rdfs:label xml:lang="en">Vulnerability</rdfs:label>
    </owl:Class>
    


    <!-- https://w3id.org/hacid/onto/ccso/VulnerabilityType -->

    <owl:Class rdf:about="https://w3id.org/hacid/onto/ccso/VulnerabilityType">
        <rdfs:subClassOf rdf:resource="https://w3id.org/hacid/onto/top-level/Concept"/>
        <rdfs:subClassOf>
            <owl:Restriction>
                <owl:onProperty rdf:resource="https://w3id.org/hacid/onto/top-level/classifies"/>
                <owl:allValuesFrom rdf:resource="https://w3id.org/hacid/onto/ccso/Vulnerability"/>
            </owl:Restriction>
        </rdfs:subClassOf>
        <rdfs:isDefinedBy rdf:resource="https://w3id.org/hacid/onto/ccso"/>
        <rdfs:label xml:lang="en">Vulnerability Type</rdfs:label>
    </owl:Class>
    


    <!-- https://w3id.org/hacid/onto/data#Dataset -->

    <owl:Class rdf:about="https://w3id.org/hacid/onto/data#Dataset"/>
    


    <!-- https://w3id.org/hacid/onto/data/DataGeneratingProcess -->

    <owl:Class rdf:about="https://w3id.org/hacid/onto/data/DataGeneratingProcess"/>
    


    <!-- https://w3id.org/hacid/onto/top-level#Object -->

    <owl:Class rdf:about="https://w3id.org/hacid/onto/top-level#Object"/>
    


    <!-- https://w3id.org/hacid/onto/top-level/TimeEntity -->

    <owl:Class rdf:about="https://w3id.org/hacid/onto/top-level/TimeEntity"/>
    


    <!-- 
    ///////////////////////////////////////////////////////////////////////////////////////
    //
    // Individuals
    //
    ///////////////////////////////////////////////////////////////////////////////////////
     -->

    


    <!-- https://w3id.org/hacid/data/cs/scenarios/RCP/RCP1.9 -->

    <owl:NamedIndividual rdf:about="https://w3id.org/hacid/data/cs/scenarios/RCP/RCP1.9">
        <rdf:type rdf:resource="https://w3id.org/hacid/onto/ccso/GreenhouseGasConcentrationPathway"/>
        <top:acronym xml:lang="en">RCP 1.9</top:acronym>
        <rdfs:comment xml:lang="en">RCP 1.9 is a pathway that limits global warming to below 1.5 °C, the aspirational goal of the Paris Agreement.</rdfs:comment>
        <rdfs:isDefinedBy rdf:resource="https://w3id.org/hacid/onto/ccso"/>
        <rdfs:label xml:lang="en">Representative Concentration Pathway 1.9</rdfs:label>
    </owl:NamedIndividual>
    


    <!-- https://w3id.org/hacid/data/cs/scenarios/RCP/RCP2.6 -->

    <owl:NamedIndividual rdf:about="https://w3id.org/hacid/data/cs/scenarios/RCP/RCP2.6">
        <rdf:type rdf:resource="https://w3id.org/hacid/onto/ccso/GreenhouseGasConcentrationPathway"/>
        <top:acronym xml:lang="en">RCP 2.6</top:acronym>
        <rdfs:comment xml:lang="en">RCP 2.6 is a &quot;very stringent&quot; pathway. According to the IPCC, RCP 2.6 requires that carbon dioxide (CO2) emissions start declining by 2020 and go to zero by 2100. It also requires that methane emissions (CH4) go to approximately half the CH4 levels of 2020, and that sulphur dioxide (SO2) emissions decline to approximately 10% of those of 1980–1990. Like all the other RCPs, RCP 2.6 requires negative CO2 emissions (such as CO2 absorption by trees). For RCP 2.6, those negative emissions would be on average 2 Gigatons of CO2 per year (GtCO2/yr). RCP 2.6 is likely to keep global temperature rise below 2 °C by 2100.</rdfs:comment>
        <rdfs:isDefinedBy rdf:resource="https://w3id.org/hacid/onto/ccso"/>
        <rdfs:label xml:lang="en">Representative Concentration Pathway 2.6</rdfs:label>
    </owl:NamedIndividual>
    


    <!-- https://w3id.org/hacid/data/cs/scenarios/RCP/RCP3.4 -->

    <owl:NamedIndividual rdf:about="https://w3id.org/hacid/data/cs/scenarios/RCP/RCP3.4">
        <rdf:type rdf:resource="https://w3id.org/hacid/onto/ccso/GreenhouseGasConcentrationPathway"/>
        <top:acronym xml:lang="en">RCP 3.4</top:acronym>
        <rdfs:comment xml:lang="en">RCP 3.4 represents an intermediate pathway between the &quot;very stringent&quot; RCP2.6 and less stringent mitigation efforts associated with RCP4.5. As well as just providing another option a variant of RCP3.4 includes considerable removal of greenhouse gases from the atmosphere. A 2021 paper suggests that the most plausible projections of cumulative CO2 emissions (having a 0.1% or 0.3% tolerance with historical accuracy) tend to suggest that RCP 3.4 (3.4 W/m^2, 2.0–2.4 degrees Celsius warming by 2100 according to study) is the most plausible pathway.</rdfs:comment>
        <rdfs:isDefinedBy rdf:resource="https://w3id.org/hacid/onto/ccso"/>
        <rdfs:label xml:lang="en">Representative Concentration Pathway 3.4</rdfs:label>
    </owl:NamedIndividual>
    


    <!-- https://w3id.org/hacid/data/cs/scenarios/RCP/RCP4.5 -->

    <owl:NamedIndividual rdf:about="https://w3id.org/hacid/data/cs/scenarios/RCP/RCP4.5">
        <rdf:type rdf:resource="https://w3id.org/hacid/onto/ccso/GreenhouseGasConcentrationPathway"/>
        <top:acronym xml:lang="en">RCP 4.5</top:acronym>
        <rdfs:comment xml:lang="en">RCP 4.5 is described by the IPCC as an intermediate scenario. Emissions in RCP 4.5 peak around 2040, then decline. According to the IPCC, RCP 4.5 requires that carbon dioxide (CO2) emissions start declining by approximately 2045 to reach roughly half of the levels of 2050 by 2100. It also requires that methane emissions (CH4) stop increasing by 2050 and decline somewhat to about 75% of the CH4 levels of 2040, and that sulphur dioxide (SO2) emissions decline to approximately 20% of those of 1980–1990. Like all the other RCPs, RCP 4.5 requires negative CO2 emissions (such as CO2 absorption by trees). For RCP 4.5, those negative emissions would be 2 Gigatons of CO2 per year (GtCO2/yr). RCP 4.5 is more likely than not to result in global temperature rise between 2 °C and 3 °C, by 2100 with a mean sea level rise 35% higher than that of RCP 2.6. Many plant and animal species will be unable to adapt to the effects of RCP 4.5 and higher RCPs.</rdfs:comment>
        <rdfs:isDefinedBy rdf:resource="https://w3id.org/hacid/onto/ccso"/>
        <rdfs:label xml:lang="en">Representative Concentration Pathway 4.5</rdfs:label>
    </owl:NamedIndividual>
    


    <!-- https://w3id.org/hacid/data/cs/scenarios/RCP/RCP6 -->

    <owl:NamedIndividual rdf:about="https://w3id.org/hacid/data/cs/scenarios/RCP/RCP6">
        <rdf:type rdf:resource="https://w3id.org/hacid/onto/ccso/GreenhouseGasConcentrationPathway"/>
        <top:acronym xml:lang="en">RCP 6</top:acronym>
        <rdfs:comment xml:lang="en">In RCP 6, emissions peak around 2080, then decline. The RCP 6.0 scenario uses a high greenhouse gas emission rate and is a stabilisation scenario where total radiative forcing is stabilised after 2100 by employment of a range of technologies and strategies for reducing greenhouse gas emissions. 6.0 W/m2 refers to the radiative forcing reached by 2100 Projections for temperature according to RCP 6.0 include continuous global warming through 2100 where CO2 levels rise to 670 ppm by 2100 making the global temperature rise by about 3–4 °C by 2100.</rdfs:comment>
        <rdfs:isDefinedBy rdf:resource="https://w3id.org/hacid/onto/ccso"/>
        <rdfs:label xml:lang="en">Representative Concentration Pathway 6</rdfs:label>
    </owl:NamedIndividual>
    


    <!-- https://w3id.org/hacid/data/cs/scenarios/RCP/RCP7 -->

    <owl:NamedIndividual rdf:about="https://w3id.org/hacid/data/cs/scenarios/RCP/RCP7">
        <rdf:type rdf:resource="https://w3id.org/hacid/onto/ccso/GreenhouseGasConcentrationPathway"/>
        <top:acronym xml:lang="en">RCP 7</top:acronym>
        <rdfs:comment xml:lang="en">RCP7 is a baseline outcome rather than a mitigation target.</rdfs:comment>
        <rdfs:isDefinedBy rdf:resource="https://w3id.org/hacid/onto/ccso"/>
        <rdfs:label xml:lang="en">Representative Concentration Pathway 7</rdfs:label>
    </owl:NamedIndividual>
    


    <!-- https://w3id.org/hacid/data/cs/scenarios/RCP/RCP8.5 -->

    <owl:NamedIndividual rdf:about="https://w3id.org/hacid/data/cs/scenarios/RCP/RCP8.5">
        <top:acronym xml:lang="en">RCP 8.5</top:acronym>
        <rdfs:comment xml:lang="en">In RCP 8.5 emissions continue to rise throughout the 21st century. RCP8.5, generally taken as the basis for worst-case climate change scenarios, was based on what proved to be overestimation of projected coal outputs. It is still used for predicting mid-century (and earlier) emissions based on current and stated policies.</rdfs:comment>
        <rdfs:isDefinedBy rdf:resource="https://w3id.org/hacid/onto/ccso"/>
        <rdfs:label xml:lang="en">Representative Concentration Pathway 8.5</rdfs:label>
    </owl:NamedIndividual>
    


    <!-- https://w3id.org/hacid/data/cs/scenarios/SSP/SSP1 -->

    <owl:NamedIndividual rdf:about="https://w3id.org/hacid/data/cs/scenarios/SSP/SSP1">
        <rdf:type rdf:resource="https://w3id.org/hacid/onto/ccso/SharedSocioeconomicPathway"/>
        <top:acronym xml:lang="en">SS1</top:acronym>
        <terms:title xml:lang="en">SS1: Sustainability (&quot;Taking the Green Road&quot;)</terms:title>
        <rdfs:comment xml:lang="en">The world shifts gradually, but pervasively, toward a more sustainable path, emphasizing more inclusive development that respects predicted environmental boundaries. Management of the global commons slowly improves, educational and health investments accelerate the demographic transition, and the emphasis on economic growth shifts toward a broader emphasis on human well-being. Driven by an increasing commitment to achieving development goals, inequality is reduced both across and within countries. Consumption is oriented toward low material growth and lower resource and energy intensity.</rdfs:comment>
        <rdfs:isDefinedBy rdf:resource="https://w3id.org/hacid/onto/ccso"/>
        <rdfs:label xml:lang="en">Shared Socioeconomic Pathways 1</rdfs:label>
    </owl:NamedIndividual>
    


    <!-- https://w3id.org/hacid/data/cs/scenarios/SSP/SSP2 -->

    <owl:NamedIndividual rdf:about="https://w3id.org/hacid/data/cs/scenarios/SSP/SSP2">
        <rdf:type rdf:resource="https://w3id.org/hacid/onto/ccso/SharedSocioeconomicPathway"/>
        <top:acronym xml:lang="en">SSP 2</top:acronym>
        <terms:title xml:lang="en">SSP2: Middle of the road</terms:title>
        <rdfs:comment xml:lang="en">The world follows a path in which social, economic, and technological trends do not shift markedly from historical patterns. Development and income growth proceeds unevenly, with some countries making relatively good progress while others fall short of expectations. Global and national institutions work toward but make slow progress in achieving sustainable development goals. Environmental systems experience degradation, although there are some improvements and overall the intensity of resource and energy use declines. Global population growth is moderate and levels off in the second half of the century. Income inequality persists or improves only slowly and challenges to reducing vulnerability to societal and environmental changes remain.</rdfs:comment>
        <rdfs:isDefinedBy rdf:resource="https://w3id.org/hacid/onto/ccso"/>
        <rdfs:label xml:lang="en">Shared Socioeconomic Pathways 2</rdfs:label>
    </owl:NamedIndividual>
    


    <!-- https://w3id.org/hacid/data/cs/scenarios/SSP/SSP3 -->

    <owl:NamedIndividual rdf:about="https://w3id.org/hacid/data/cs/scenarios/SSP/SSP3">
        <rdf:type rdf:resource="https://w3id.org/hacid/onto/ccso/SharedSocioeconomicPathway"/>
        <top:acronym xml:lang="en">SSP 3</top:acronym>
        <terms:title xml:lang="en">SSP3: Regional rivalry (A Rocky Road)</terms:title>
        <rdfs:comment xml:lang="en">A resurgent nationalism, concerns about competitiveness and security, and regional conflicts push countries to increasingly focus on domestic or, at most, regional issues. Policies shift over time to become increasingly oriented toward national and regional security issues. Countries focus on achieving energy and food security goals within their own regions at the expense of broader-based development. Investments in education and technological development decline. Economic development is slow, consumption is material-intensive, and inequalities persist or worsen over time. Population growth is low in industrialized and high in developing countries. A low international priority for addressing environmental concerns leads to strong environmental degradation in some regions.</rdfs:comment>
        <rdfs:isDefinedBy rdf:resource="https://w3id.org/hacid/onto/ccso"/>
        <rdfs:label xml:lang="en">Shared Socioeconomic Pathways 3</rdfs:label>
    </owl:NamedIndividual>
    


    <!-- https://w3id.org/hacid/data/cs/scenarios/SSP/SSP4 -->

    <owl:NamedIndividual rdf:about="https://w3id.org/hacid/data/cs/scenarios/SSP/SSP4">
        <rdf:type rdf:resource="https://w3id.org/hacid/onto/ccso/SharedSocioeconomicPathway"/>
        <top:acronym xml:lang="en">SSP 4</top:acronym>
        <terms:title xml:lang="en">SSP4: Inequality (A Road Divided)</terms:title>
        <rdfs:comment xml:lang="en">Highly unequal investments in human capital, combined with increasing disparities in economic opportunity and political power, lead to increasing inequalities and stratification both across and within countries. Over time, a gap widens between an internationally-connected society that contributes to knowledge- and capital-intensive sectors of the global economy, and a fragmented collection of lower-income, poorly educated societies that work in a labor intensive, low-tech economy. Social cohesion degrades and conflict and unrest become increasingly common. Technology development is high in the high-tech economy and sectors. The globally connected energy sector diversifies, with investments in both carbon-intensive fuels like coal and unconventional oil, but also low-carbon energy sources. Environmental policies focus on local issues around middle and high income areas.</rdfs:comment>
        <rdfs:isDefinedBy rdf:resource="https://w3id.org/hacid/onto/ccso"/>
        <rdfs:label xml:lang="en">Shared Socioeconomic Pathways 4</rdfs:label>
    </owl:NamedIndividual>
    


    <!-- https://w3id.org/hacid/data/cs/scenarios/SSP/SSP5 -->

    <owl:NamedIndividual rdf:about="https://w3id.org/hacid/data/cs/scenarios/SSP/SSP5">
        <rdf:type rdf:resource="https://w3id.org/hacid/onto/ccso/SharedSocioeconomicPathway"/>
        <top:acronym xml:lang="en">SSP 5</top:acronym>
        <terms:title xml:lang="en">SSP5: Fossil-Fueled Development (Taking the Highway)</terms:title>
        <rdfs:comment xml:lang="en">This world places increasing faith in competitive markets, innovation and participatory societies to produce rapid technological progress and development of human capital as the path to sustainable development. Global markets are increasingly integrated. There are also strong investments in health, education, and institutions to enhance human and social capital. At the same time, the push for economic and social development is coupled with the exploitation of abundant fossil fuel resources and the adoption of resource and energy intensive lifestyles around the world. All these factors lead to rapid growth of the global economy, while global population peaks and declines in the 21st century. Local environmental problems like air pollution are successfully managed. There is faith in the ability to effectively manage social and ecological systems, including by geo-engineering if necessary.</rdfs:comment>
        <rdfs:isDefinedBy rdf:resource="https://w3id.org/hacid/onto/ccso"/>
        <rdfs:label xml:lang="en">Shared Socioeconomic Pathways 5</rdfs:label>
    </owl:NamedIndividual>
</rdf:RDF>



<!-- Generated by the OWL API (version 4.5.26.2023-07-17T20:34:13Z) https://github.com/owlcs/owlapi -->

